General terminology and notation.

\begin{code}

{-# OPTIONS --without-K --exact-split --safe --no-sized-types --no-guardedness --auto-inline #-}

module Notation.General where

open import MLTT.Pi
open import MLTT.Sigma
open import MLTT.Universes
open import MLTT.Id
open import MLTT.Negation public

Type  = Set
Type₁ = Set₁

reflexive : {X : 𝓤 ̇ } → (X → X → 𝓥 ̇ ) → 𝓤 ⊔ 𝓥 ̇
reflexive R = ∀ x → R x x

symmetric : {X : 𝓤 ̇ } → (X → X → 𝓥 ̇ ) → 𝓤 ⊔ 𝓥 ̇
symmetric R = ∀ x y → R x y → R y x

antisymmetric : {X : 𝓤 ̇ } → (X → X → 𝓥 ̇ ) → 𝓤 ⊔ 𝓥 ̇
antisymmetric R = ∀ x y → R x y → R y x → x ＝ y

transitive : {X : 𝓤 ̇ } → (X → X → 𝓥 ̇ ) → 𝓤 ⊔ 𝓥 ̇
transitive R = ∀ x y z → R x y → R y z → R x z

idempotent-map : {X : 𝓥 ̇ } → (f : X → X) → 𝓥 ̇
idempotent-map f = ∀ x → f (f x) ＝ f x

involutive : {X : 𝓥 ̇ } → (f : X → X) → 𝓥 ̇
involutive f = ∀ x → f (f x) ＝ x

left-neutral : {X : 𝓤 ̇ } → X → (X → X → X) → 𝓤 ̇
left-neutral e _·_ = ∀ x → e · x ＝ x

right-neutral : {X : 𝓤 ̇ } → X → (X → X → X) → 𝓤 ̇
right-neutral e _·_ = ∀ x → x · e ＝ x

associative : {X : 𝓤 ̇ } → (X → X → X) → 𝓤 ̇
associative _·_ = ∀ x y z → (x · y) · z ＝ x · (y · z)

commutative : {X : 𝓤 ̇ } → (X → X → X) → 𝓤 ̇
commutative _·_ = ∀ x y → (x · y) ＝ (y · x)

left-cancellable : {X : 𝓤 ̇ } {Y : 𝓥 ̇ } → (X → Y) → 𝓤 ⊔ 𝓥 ̇
left-cancellable f = ∀ {x x'} → f x ＝ f x' → x ＝ x'

left-cancellable' : {X : 𝓤 ̇ } {Y : 𝓥 ̇ } → (X → Y) → 𝓤 ⊔ 𝓥 ̇
left-cancellable' f = ∀ x x' → f x ＝ f x' → x ＝ x'

right-cancellable : {X : 𝓤 ̇ } {Y : 𝓥 ̇ } → (X → Y) → 𝓤ω
right-cancellable f = {𝓦 : Universe} {Z : 𝓦 ̇ } (g h : codomain f → Z)
                    → g ∘ f ∼ h ∘ f
                    → g ∼ h

_⇔_ : 𝓤 ̇ → 𝓥 ̇ → 𝓤 ⊔ 𝓥 ̇
A ⇔ B = (A → B) × (B → A)

lr-implication : {X : 𝓤 ̇ } {Y : 𝓥 ̇ } → (X ⇔ Y) → (X → Y)
lr-implication = pr₁

rl-implication : {X : 𝓤 ̇ } {Y : 𝓥 ̇ } → (X ⇔ Y) → (Y → X)
rl-implication = pr₂

⇔-sym : {X : 𝓤' ̇  } {Y : 𝓥' ̇  } → X ⇔ Y → Y ⇔ X
⇔-sym (f , g) = (g , f)

⇔-trans : {X : 𝓤' ̇  } {Y : 𝓥' ̇  } {Z : 𝓦' ̇  }
        → X ⇔ Y → Y ⇔ Z → X ⇔ Z
⇔-trans (f , g) (h , k) = (h ∘ f , g ∘ k)

⇔-refl : {X : 𝓤' ̇  } → X ⇔ X
⇔-refl = (id , id)

\end{code}

This is to avoid naming implicit arguments:

\begin{code}

type-of : {X : 𝓤 ̇ } → X → 𝓤 ̇
type-of {𝓤} {X} x = X

\end{code}

We use the following to indicate the type of a subterm (where "∶"
(typed "\:" in emacs) is not the same as ":"):

\begin{code}

-id : (X : 𝓤 ̇ ) → X → X
-id X x = x

syntax -id X x = x ∶ X

\end{code}

This is used for efficiency as a substitute for lazy "let" (or "where"):

\begin{code}

case_of_ : {A : 𝓤 ̇ } {B : A → 𝓥 ̇ } → (a : A) → ((a : A) → B a) → B a
case x of f = f x

Case_of_ : {A : 𝓤 ̇ } {B : A → 𝓥 ̇ } → (a : A) → ((x : A) → a ＝ x → B a) → B a
Case x of f = f x refl

{-# NOINLINE case_of_ #-}

\end{code}

Notation to try to make proofs readable:

\begin{code}

need_which-is-given-by_ : (A : 𝓤 ̇ ) → A → A
need A which-is-given-by a = a

have_by_ : (A : 𝓤 ̇ ) → A → A
have A by a = a

have_so_ : {A : 𝓤 ̇ } {B : 𝓥 ̇ } → A → B → B
have a so b = b

have_so-use_ : {A : 𝓤 ̇ } {B : 𝓥 ̇ } → A → B → B
have a so-use b = b

have_and_ : {A : 𝓤 ̇ } {B : 𝓥 ̇ } → A → B → B
have a and b = b

apply_to_ : {A : 𝓤 ̇ } {B : 𝓥 ̇ } → (A → B) → A → B
apply f to a = f a

have_so-apply_ : {A : 𝓤 ̇ } {B : 𝓥 ̇ } → A → (A → B) → B
have a so-apply f = f a

assume-then : (A : 𝓤 ̇ ) {B : A → 𝓥 ̇ } → ((a : A) → B a) → (a : A) → B a
assume-then A f x = f x

syntax assume-then A (λ x → b) = assume x ∶ A then b

assume-and : (A : 𝓤 ̇ ) {B : A → 𝓥 ̇ } → ((a : A) → B a) → (a : A) → B a
assume-and A f x = f x

syntax assume-and A (λ x → b) = assume x ∶ A and b

mapsto : {A : 𝓤 ̇ } {B : A → 𝓥 ̇ } → ((a : A) → B a) → (a : A) → B a
mapsto f = f

syntax mapsto (λ x → b) = x ↦ b

infixr 10 mapsto

Mapsto : (A : 𝓤 ̇ ) {B : A → 𝓥 ̇ } → ((a : A) → B a) → (a : A) → B a
Mapsto A f = f

syntax Mapsto A (λ x → b) = x ꞉ A ↦ b

infixr 10 Mapsto

\end{code}

Get rid of this:

\begin{code}

Σ! : {X : 𝓤 ̇ } (A : X → 𝓥 ̇ ) → 𝓤 ⊔ 𝓥 ̇
Σ! {𝓤} {𝓥} {X} A = (Σ x ꞉ X , A x) × ((x x' : X) → A x → A x' → x ＝ x')

Sigma! : (X : 𝓤 ̇ ) (A : X → 𝓥 ̇ ) → 𝓤 ⊔ 𝓥 ̇
Sigma! X A = Σ! A

syntax Sigma! A (λ x → b) = Σ! x ꞉ A , b

infixr -1 Sigma!

\end{code}

Note: Σ! is to be avoided, in favour of the contractibility of Σ,
following univalent mathematics.

Fixities:

\begin{code}

infixl -1 -id
infix -1 _⇔_

\end{code}
