Martin Escardo 1st May 2020.

This is ported from the Midlands Graduate School 2019 lecture notes

 https://www.cs.bham.ac.uk/~mhe/HoTT-UF.in-Agda-Lecture-Notes/HoTT-UF-Agda.html
 https://github.com/martinescardo/HoTT-UF.Agda-Lecture-Notes

\begin{code}

{-# OPTIONS --without-K --exact-split --safe --no-sized-types --no-guardedness --auto-inline #-}

module MGS.Basic-UF where

open import MGS.MLTT public

is-center : (X : 𝓤 ̇ ) → X → 𝓤 ̇
is-center X c = (x : X) → c ＝ x

is-singleton : 𝓤 ̇ → 𝓤 ̇
is-singleton X = Σ c ꞉ X , is-center X c

𝟙-is-singleton : is-singleton 𝟙
𝟙-is-singleton = ⋆ , 𝟙-induction (λ x → ⋆ ＝ x) (refl ⋆)

center : (X : 𝓤 ̇ ) → is-singleton X → X
center X (c , φ) = c

centrality : (X : 𝓤 ̇ ) (i : is-singleton X) (x : X) → center X i ＝ x
centrality X (c , φ) = φ

is-subsingleton : 𝓤 ̇ → 𝓤 ̇
is-subsingleton X = (x y : X) → x ＝ y

𝟘-is-subsingleton : is-subsingleton 𝟘
𝟘-is-subsingleton x y = !𝟘 (x ＝ y) x

singletons-are-subsingletons : (X : 𝓤 ̇ ) → is-singleton X → is-subsingleton X
singletons-are-subsingletons X (c , φ) x y = x ＝⟨ (φ x)⁻¹ ⟩
                                             c ＝⟨ φ y ⟩
                                             y ∎

𝟙-is-subsingleton : is-subsingleton 𝟙
𝟙-is-subsingleton = singletons-are-subsingletons 𝟙 𝟙-is-singleton

pointed-subsingletons-are-singletons : (X : 𝓤 ̇ )
                                     → X → is-subsingleton X → is-singleton X

pointed-subsingletons-are-singletons X x s = (x , s x)

singleton-iff-pointed-and-subsingleton : {X : 𝓤 ̇ }
                                       → is-singleton X ⇔ (X × is-subsingleton X)

singleton-iff-pointed-and-subsingleton {𝓤} {X} = (a , b)
 where
  a : is-singleton X → X × is-subsingleton X
  a s = center X s , singletons-are-subsingletons X s

  b : X × is-subsingleton X → is-singleton X
  b (x , t) = pointed-subsingletons-are-singletons X x t

is-prop is-truth-value : 𝓤 ̇ → 𝓤 ̇
is-prop        = is-subsingleton
is-truth-value = is-subsingleton

is-set : 𝓤 ̇ → 𝓤 ̇
is-set X = (x y : X) → is-subsingleton (x ＝ y)

EM EM' : ∀ 𝓤 → 𝓤 ⁺ ̇
EM  𝓤 = (X : 𝓤 ̇ ) → is-subsingleton X → X + ¬ X
EM' 𝓤 = (X : 𝓤 ̇ ) → is-subsingleton X → is-singleton X + is-empty X

EM-gives-EM' : EM 𝓤 → EM' 𝓤
EM-gives-EM' em X s = γ (em X s)
 where
  γ : X + ¬ X → is-singleton X + is-empty X
  γ (inl x) = inl (pointed-subsingletons-are-singletons X x s)
  γ (inr x) = inr x

EM'-gives-EM : EM' 𝓤 → EM 𝓤
EM'-gives-EM em' X s = γ (em' X s)
 where
  γ : is-singleton X + is-empty X → X + ¬ X
  γ (inl i) = inl (center X i)
  γ (inr x) = inr x

no-unicorns : ¬ (Σ X ꞉ 𝓤 ̇ , is-subsingleton X × ¬ (is-singleton X) × ¬ (is-empty X))
no-unicorns (X , i , f , g) = c
 where
  e : is-empty X
  e x = f (pointed-subsingletons-are-singletons X x i)

  c : 𝟘
  c = g e

module magmas where

 Magma : (𝓤 : Universe) → 𝓤 ⁺ ̇
 Magma 𝓤 = Σ X ꞉ 𝓤 ̇ , is-set X × (X → X → X)

 ⟨_⟩ : Magma 𝓤 → 𝓤 ̇
 ⟨ X , i , _·_ ⟩ = X

 magma-is-set : (M : Magma 𝓤) → is-set ⟨ M ⟩
 magma-is-set (X , i , _·_) = i

 magma-operation : (M : Magma 𝓤) → ⟨ M ⟩ → ⟨ M ⟩ → ⟨ M ⟩
 magma-operation (X , i , _·_) = _·_

 syntax magma-operation M x y = x ·⟨ M ⟩ y

 is-magma-hom : (M N : Magma 𝓤) → (⟨ M ⟩ → ⟨ N ⟩) → 𝓤 ̇
 is-magma-hom M N f = (x y : ⟨ M ⟩) → f (x ·⟨ M ⟩ y) ＝ f x ·⟨ N ⟩ f y

 id-is-magma-hom : (M : Magma 𝓤) → is-magma-hom M M (𝑖𝑑 ⟨ M ⟩)
 id-is-magma-hom M = λ (x y : ⟨ M ⟩) → refl (x ·⟨ M ⟩ y)

 is-magma-iso : (M N : Magma 𝓤) → (⟨ M ⟩ → ⟨ N ⟩) → 𝓤 ̇
 is-magma-iso M N f = is-magma-hom M N f
                    × (Σ g ꞉ (⟨ N ⟩ → ⟨ M ⟩), is-magma-hom N M g
                                            × (g ∘ f ∼ 𝑖𝑑 ⟨ M ⟩)
                                            × (f ∘ g ∼ 𝑖𝑑 ⟨ N ⟩))

 id-is-magma-iso : (M : Magma 𝓤) → is-magma-iso M M (𝑖𝑑 ⟨ M ⟩)
 id-is-magma-iso M = id-is-magma-hom M ,
                     𝑖𝑑 ⟨ M ⟩ ,
                     id-is-magma-hom M ,
                     refl ,
                     refl

 Id→iso : {M N : Magma 𝓤} → M ＝ N → ⟨ M ⟩ → ⟨ N ⟩
 Id→iso p = transport ⟨_⟩ p

 Id→iso-is-iso : {M N : Magma 𝓤} (p : M ＝ N) → is-magma-iso M N (Id→iso p)
 Id→iso-is-iso (refl M) = id-is-magma-iso M

 _≅ₘ_ : Magma 𝓤 → Magma 𝓤 → 𝓤 ̇
 M ≅ₘ N = Σ f ꞉ (⟨ M ⟩ → ⟨ N ⟩), is-magma-iso M N f

 magma-Id→iso : {M N : Magma 𝓤} → M ＝ N → M ≅ₘ N
 magma-Id→iso p = (Id→iso p , Id→iso-is-iso p)

 ∞-Magma : (𝓤 : Universe) → 𝓤 ⁺ ̇
 ∞-Magma 𝓤 = Σ X ꞉ 𝓤 ̇ , (X → X → X)

module monoids where

 left-neutral : {X : 𝓤 ̇ } → X → (X → X → X) → 𝓤 ̇
 left-neutral e _·_ = ∀ x → e · x ＝ x

 right-neutral : {X : 𝓤 ̇ } → X → (X → X → X) → 𝓤 ̇
 right-neutral e _·_ = ∀ x → x · e ＝ x

 associative : {X : 𝓤 ̇ } → (X → X → X) → 𝓤 ̇
 associative _·_ = ∀ x y z → (x · y) · z ＝ x · (y · z)

 Monoid : (𝓤 : Universe) → 𝓤 ⁺ ̇
 Monoid 𝓤 = Σ X ꞉ 𝓤  ̇ , is-set X
                      × (Σ · ꞉ (X → X → X) , (Σ e ꞉ X , (left-neutral e ·)
                                                      × (right-neutral e ·)
                                                      × (associative ·)))

refl-left : {X : 𝓤 ̇ } {x y : X} {p : x ＝ y} → refl x ∙ p ＝ p
refl-left {𝓤} {X} {x} {x} {refl x} = refl (refl x)

refl-right : {X : 𝓤 ̇ } {x y : X} {p : x ＝ y} → p ∙ refl y ＝ p
refl-right {𝓤} {X} {x} {y} {p} = refl p

∙assoc : {X : 𝓤 ̇ } {x y z t : X} (p : x ＝ y) (q : y ＝ z) (r : z ＝ t)
       → (p ∙ q) ∙ r ＝ p ∙ (q ∙ r)

∙assoc p q (refl z) = refl (p ∙ q)

⁻¹-left∙ : {X : 𝓤 ̇ } {x y : X} (p : x ＝ y)
         → p ⁻¹ ∙ p ＝ refl y

⁻¹-left∙ (refl x) = refl (refl x)

⁻¹-right∙ : {X : 𝓤 ̇ } {x y : X} (p : x ＝ y)
          → p ∙ p ⁻¹ ＝ refl x

⁻¹-right∙ (refl x) = refl (refl x)

⁻¹-involutive : {X : 𝓤 ̇ } {x y : X} (p : x ＝ y)
              → (p ⁻¹)⁻¹ ＝ p

⁻¹-involutive (refl x) = refl (refl x)

ap-refl : {X : 𝓤 ̇ } {Y : 𝓥 ̇ } (f : X → Y) (x : X)
        → ap f (refl x) ＝ refl (f x)

ap-refl f x = refl (refl (f x))

ap-∙ : {X : 𝓤 ̇ } {Y : 𝓥 ̇ } (f : X → Y) {x y z : X} (p : x ＝ y) (q : y ＝ z)
     → ap f (p ∙ q) ＝ ap f p ∙ ap f q

ap-∙ f p (refl y) = refl (ap f p)

ap⁻¹ : {X : 𝓤 ̇ } {Y : 𝓥 ̇ } (f : X → Y) {x y : X} (p : x ＝ y)
     → (ap f p)⁻¹ ＝ ap f (p ⁻¹)

ap⁻¹ f (refl x) = refl (refl (f x))

ap-id : {X : 𝓤 ̇ } {x y : X} (p : x ＝ y)
      → ap id p ＝ p

ap-id (refl x) = refl (refl x)

ap-∘ : {X : 𝓤 ̇ } {Y : 𝓥 ̇ } {Z : 𝓦 ̇ }
       (f : X → Y) (g : Y → Z) {x y : X} (p : x ＝ y)
     → ap (g ∘ f) p ＝ (ap g ∘ ap f) p

ap-∘ f g (refl x) = refl (refl (g (f x)))

transport∙ : {X : 𝓤 ̇ } (A : X → 𝓥 ̇ ) {x y z : X} (p : x ＝ y) (q : y ＝ z)
           → transport A (p ∙ q) ＝ transport A q ∘ transport A p

transport∙ A p (refl y) = refl (transport A p)

Nat : {X : 𝓤 ̇ } → (X → 𝓥 ̇ ) → (X → 𝓦 ̇ ) → 𝓤 ⊔ 𝓥 ⊔ 𝓦 ̇
Nat A B = (x : domain A) → A x → B x

Nats-are-natural : {X : 𝓤 ̇ } (A : X → 𝓥 ̇ ) (B : X → 𝓦 ̇ ) (τ : Nat A B)
                 → {x y : X} (p : x ＝ y)
                 → τ y ∘ transport A p ＝ transport B p ∘ τ x

Nats-are-natural A B τ (refl x) = refl (τ x)

NatΣ : {X : 𝓤 ̇ } {A : X → 𝓥 ̇ } {B : X → 𝓦 ̇ } → Nat A B → Σ A → Σ B
NatΣ τ (x , a) = (x , τ x a)

transport-ap : {X : 𝓤 ̇ } {Y : 𝓥 ̇ } (A : Y → 𝓦 ̇ )
               (f : X → Y) {x x' : X} (p : x ＝ x') (a : A (f x))
             → transport (A ∘ f) p a ＝ transport A (ap f p) a

transport-ap A f (refl x) a = refl a

apd : {X : 𝓤 ̇ } {A : X → 𝓥 ̇ } (f : (x : X) → A x) {x y : X}
      (p : x ＝ y) → transport A p (f x) ＝ f y

apd f (refl x) = refl (f x)

to-Σ-＝ : {X : 𝓤 ̇ } {A : X → 𝓥 ̇ } {σ τ : Σ A}
       → (Σ p ꞉ pr₁ σ ＝ pr₁ τ , transport A p (pr₂ σ) ＝ pr₂ τ)
       → σ ＝ τ

to-Σ-＝ (refl x , refl a) = refl (x , a)

from-Σ-＝ : {X : 𝓤 ̇ } {A : X → 𝓥 ̇ } {σ τ : Σ A}
         → σ ＝ τ
         → Σ p ꞉ pr₁ σ ＝ pr₁ τ , transport A p (pr₂ σ) ＝ pr₂ τ

from-Σ-＝ (refl (x , a)) = (refl x , refl a)

to-Σ-＝' : {X : 𝓤 ̇ } {A : X → 𝓥 ̇ } {x : X} {a a' : A x}
        → a ＝ a' → Id (Σ A) (x , a) (x , a')

to-Σ-＝' {𝓤} {𝓥} {X} {A} {x} = ap (λ - → (x , -))

transport-× : {X : 𝓤 ̇ } (A : X → 𝓥 ̇ ) (B : X → 𝓦 ̇ )
                {x y : X} (p : x ＝ y) {c : A x × B x}

            → transport (λ x → A x × B x) p c
            ＝ (transport A p (pr₁ c) , transport B p (pr₂ c))

transport-× A B (refl _) = refl _

transportd : {X : 𝓤 ̇ } (A : X → 𝓥 ̇ ) (B : (x : X) → A x → 𝓦 ̇ )
             {x : X} (a : A x) ((a' , b) : Σ a ꞉ A x , B x a) {y : X} (p : x ＝ y)
           → B x a' → B y (transport A p a')

transportd A B a σ (refl y) = id

transport-Σ : {X : 𝓤 ̇ } (A : X → 𝓥 ̇ ) (B : (x : X) → A x → 𝓦 ̇ )
              {x : X} (y : X) (p : x ＝ y) (a : A x) {(a' , b) : Σ a ꞉ A x , B x a}

            → transport (λ x → Σ y ꞉ A x , B x y) p (a' , b)
            ＝ transport A p a' , transportd A B a (a' , b) p b

transport-Σ A B {x} x (refl x) a {σ} = refl σ

\end{code}
