Martin Escardo 2011.

\begin{code}

{-# OPTIONS --without-K --exact-split --safe --no-sized-types --no-guardedness --auto-inline #-}

open import UF.FunExt

module Naturals.Sequence (fe : FunExt) where

open import MLTT.Spartan hiding (_+_)
open import UF.Base
open import UF.Retracts
open import Naturals.Addition

_∶∶_ : {X : ℕ → 𝓤 ̇ } → X 0 → ((n : ℕ) → X (succ n)) → ((n : ℕ) → X n)
(x ∶∶ α) 0 = x
(x ∶∶ α) (succ n) = α n

head : {X : ℕ → 𝓤 ̇ } → ((n : ℕ) → X n) → X 0
head α = α 0

tail : {X : ℕ → 𝓤 ̇ } → ((n : ℕ) → X n) → ((n : ℕ) → X (succ n))
tail α n = α (succ n)

head-tail-eta : {X : ℕ → 𝓤 ̇ } {α : (n : ℕ) → X n} → (head α ∶∶ tail α) ＝ α
head-tail-eta {𝓤} {X} = dfunext (fe 𝓤₀ 𝓤) lemma
 where
  lemma : {α : (n : ℕ) → X n} → (i : ℕ) → (head α ∶∶ tail α) i ＝ α i
  lemma 0 = refl
  lemma (succ i) = refl

private cons : {X : ℕ → 𝓤 ̇ } → X 0 × ((n : ℕ) → X (succ n)) → ((n : ℕ) → X n)
cons (x , α) = x ∶∶ α

cons-has-section' : {X : ℕ → 𝓤 ̇ } → has-section' (cons {𝓤} {X})
cons-has-section' α = (head α , tail α) , head-tail-eta

\end{code}

(In fact it is an equivalence, but I won't bother, until this is
needed.)

\begin{code}

itail : {X : ℕ → 𝓤 ̇ } → (n : ℕ) → ((i : ℕ) → X i) → ((i : ℕ) → X (i + n))
itail n α i = α (i + n)

\end{code}

Added 16th July 2018. Corecursion on sequences ℕ → A.

                    p = (h,t)
             X ------------------> A × X
             |                       |
             |                       |
          f  |                       | A × f
             |                       |
             |                       |
             v                       v
         (ℕ → A) ---------------> A × (ℕ → A)
                  P = (head, tail)


  head (f x) = h x
  tail (f x) = f (t x)

Or equivalentaily

  f x = cons (h x) (f (t x))

\begin{code}

module _ {𝓤 𝓥 : Universe}
         {A : 𝓤 ̇ }
         {X : 𝓥 ̇ }
         (h : X → A)
         (t : X → X)
       where

 private
  f : X → (ℕ → A)
  f x zero = h x
  f x (succ n) = f (t x) n

 seq-corec = f

 seq-corec-head : head ∘ f ∼ h
 seq-corec-head x = refl

 seq-corec-tail : tail ∘ f ∼ f ∘ t
 seq-corec-tail x = dfunext (fe 𝓤₀ 𝓤) (λ n → refl)

 seq-final : Σ! f ꞉ (X → (ℕ → A)), (head ∘ f ∼ h) × (tail ∘ f ∼ f ∘ t)
 seq-final = (seq-corec , seq-corec-head , seq-corec-tail) , c
  where
   c : (f f' : X → ℕ → A) →
         (head ∘ f ∼ h) × (tail ∘ f ∼ f ∘ t) →
         (head ∘ f' ∼ h) × (tail ∘ f' ∼ f' ∘ t) → f ＝ f'
   c f f' (a , b) (c , d) = dfunext (fe 𝓥 𝓤) (λ x → dfunext (fe 𝓤₀ 𝓤) (r x))
    where
     r : (x : X) (n : ℕ) → f x n ＝ f' x n
     r x zero = a x ∙ (c x)⁻¹
     r x (succ n) = f x (succ n) ＝⟨ ap (λ - → - n) (b x) ⟩
                    f (t x) n    ＝⟨ r (t x) n ⟩
                    f' (t x) n   ＝⟨ ( ap (λ - → - n) (d x)) ⁻¹ ⟩
                    f' x (succ n) ∎

 \end{code}

Added 11th September 2018.

\begin{code}

seq-bisimulation : {A : 𝓤 ̇ } → ((ℕ → A) → (ℕ → A) → 𝓥 ̇ ) → 𝓤 ⊔ 𝓥 ̇
seq-bisimulation {𝓤} {𝓥} {A} R = (α β : ℕ → A) → R α β
                                                 → (head α ＝ head β)
                                                 × R (tail α) (tail β)

seq-coinduction : {A : 𝓤 ̇ } (R : (ℕ → A) → (ℕ → A) → 𝓥 ̇ )
                → seq-bisimulation R → (α β : ℕ → A) → R α β → α ＝ β
seq-coinduction {𝓤} {𝓥} {A} R b α β r = dfunext (fe 𝓤₀ 𝓤) (h α β r)
 where
  h : (α β : ℕ → A) → R α β → α ∼ β
  h α β r zero = pr₁ (b α β r)
  h α β r (succ n) = h (tail α) (tail β) (pr₂ (b α β r)) n

\end{code}
