Martin Escardo 2011.

(Totally separated types moved to the module TotallySeparated January
2018, and extended.)

\begin{code}

{-# OPTIONS --safe --without-K --exact-split #-}

module TypeTopology.DiscreteAndSeparated where

open import MLTT.Spartan

open import MLTT.Plus-Properties
open import MLTT.Two-Properties
open import Naturals.Properties
open import NotionsOfDecidability.Complemented
open import NotionsOfDecidability.Decidable
open import UF.Base
open import UF.Equiv
open import UF.FunExt
open import UF.Retracts
open import UF.Subsingletons renaming (⊤Ω to ⊤ ; ⊥Ω to ⊥)
open import UF.Subsingletons-FunExt

is-isolated : {X : 𝓤 ̇ } → X → 𝓤 ̇
is-isolated x = ∀ y → is-decidable (x ＝ y)

is-perfect : 𝓤 ̇ → 𝓤 ̇
is-perfect X = is-empty (Σ x ꞉ X , is-isolated x)

is-isolated' : {X : 𝓤 ̇ } → X → 𝓤 ̇
is-isolated' x = ∀ y → is-decidable (y ＝ x)

is-decidable-eq-sym : {X : 𝓤 ̇ } (x y : X)
                    → is-decidable (x ＝ y)
                    → is-decidable (y ＝ x)
is-decidable-eq-sym x y = cases
                           (λ (p : x ＝ y) → inl (p ⁻¹))
                           (λ (n : ¬ (x ＝ y)) → inr (λ (q : y ＝ x) → n (q ⁻¹)))

is-isolated'-gives-is-isolated : {X : 𝓤 ̇ } (x : X) → is-isolated' x → is-isolated x
is-isolated'-gives-is-isolated x i' y = is-decidable-eq-sym y x (i' y)

is-isolated-gives-is-isolated' : {X : 𝓤 ̇ } (x : X) → is-isolated x → is-isolated' x
is-isolated-gives-is-isolated' x i y = is-decidable-eq-sym x y (i y)

is-discrete : 𝓤 ̇ → 𝓤 ̇
is-discrete X = (x : X) → is-isolated x

\end{code}

Standard examples:

\begin{code}

props-are-discrete : {P : 𝓤 ̇ } → is-prop P → is-discrete P
props-are-discrete i x y = inl (i x y)

𝟘-is-discrete : is-discrete (𝟘 {𝓤})
𝟘-is-discrete = props-are-discrete 𝟘-is-prop

𝟙-is-discrete : is-discrete (𝟙 {𝓤})
𝟙-is-discrete = props-are-discrete 𝟙-is-prop

𝟚-is-discrete : is-discrete 𝟚
𝟚-is-discrete ₀ ₀ = inl refl
𝟚-is-discrete ₀ ₁ = inr (λ (p : ₀ ＝ ₁) → 𝟘-elim (zero-is-not-one p))
𝟚-is-discrete ₁ ₀ = inr (λ (p : ₁ ＝ ₀) → 𝟘-elim (zero-is-not-one (p ⁻¹)))
𝟚-is-discrete ₁ ₁ = inl refl

ℕ-is-discrete : is-discrete ℕ
ℕ-is-discrete 0 0 = inl refl
ℕ-is-discrete 0 (succ n) = inr (λ (p : zero ＝ succ n) → positive-not-zero n (p ⁻¹))
ℕ-is-discrete (succ m) 0 = inr (λ (p : succ m ＝ zero) → positive-not-zero m p)
ℕ-is-discrete (succ m) (succ n) =  step (ℕ-is-discrete m n)
  where
   step : (m ＝ n) + (m ≠ n) → (succ m ＝ succ n) + (succ m ≠ succ n)
   step (inl r) = inl (ap succ r)
   step (inr f) = inr (λ s → f (succ-lc s))

inl-is-isolated : {X : 𝓤 ̇ } {Y : 𝓥 ̇ } (x : X)
                → is-isolated x
                → is-isolated (inl x)
inl-is-isolated {𝓤} {𝓥} {X} {Y} x i = γ
 where
  γ : (z : X + Y) → is-decidable (inl x ＝ z)
  γ (inl x') = Cases (i x')
                (λ (p : x ＝ x') → inl (ap inl p))
                (λ (n : ¬ (x ＝ x')) → inr (contrapositive inl-lc n))
  γ (inr y)  = inr +disjoint

inr-is-isolated : {X : 𝓤 ̇ } {Y : 𝓥 ̇ } (y : Y)
                → is-isolated y
                → is-isolated (inr y)
inr-is-isolated {𝓤} {𝓥} {X} {Y} y i = γ
 where
  γ : (z : X + Y) → is-decidable (inr y ＝ z)
  γ (inl x)  = inr +disjoint'
  γ (inr y') = Cases (i y')
                (λ (p : y ＝ y') → inl (ap inr p))
                (λ (n : ¬ (y ＝ y')) → inr (contrapositive inr-lc n))

+-is-discrete : {X : 𝓤 ̇ } {Y : 𝓥 ̇ }
              → is-discrete X
              → is-discrete Y
              → is-discrete (X + Y)
+-is-discrete d e (inl x) = inl-is-isolated x (d x)
+-is-discrete d e (inr y) = inr-is-isolated y (e y)

\end{code}

The closure of discrete types under Σ is proved in the module
UF.Miscelanea (as this requires to first prove that discrete types
are sets).

General properties:

\begin{code}

discrete-types-are-cotransitive : {X : 𝓤 ̇ }
                                → is-discrete X
                                → {x y z : X}
                                → x ≠ y
                                → (x ≠ z) + (z ≠ y)
discrete-types-are-cotransitive d {x} {y} {z} φ = f (d x z)
 where
  f : (x ＝ z) + (x ≠ z) → (x ≠ z) + (z ≠ y)
  f (inl r) = inr (λ s → φ (r ∙ s))
  f (inr γ) = inl γ

retract-is-discrete : {X : 𝓤 ̇ } {Y : 𝓥 ̇ }
                    → retract Y of X → is-discrete X → is-discrete Y
retract-is-discrete (f , (s , φ)) d y y' = g (d (s y) (s y'))
 where
  g : is-decidable (s y ＝ s y') → is-decidable (y ＝ y')
  g (inl p) = inl ((φ y) ⁻¹ ∙ ap f p ∙ φ y')
  g (inr u) = inr (contrapositive (ap s) u)

𝟚-retract-of-non-trivial-type-with-isolated-point : {X : 𝓤 ̇ } {x₀ x₁ : X} → x₀ ≠ x₁
                                                  → is-isolated x₀ → retract 𝟚 of X
𝟚-retract-of-non-trivial-type-with-isolated-point {𝓤} {X} {x₀} {x₁} ne d = r , (s , rs)
 where
  r : X → 𝟚
  r = pr₁ (characteristic-function d)
  φ : (x : X) → (r x ＝ ₀ → x₀ ＝ x) × (r x ＝ ₁ → ¬ (x₀ ＝ x))
  φ = pr₂ (characteristic-function d)
  s : 𝟚 → X
  s ₀ = x₀
  s ₁ = x₁
  rs : (n : 𝟚) → r (s n) ＝ n
  rs ₀ = different-from-₁-equal-₀ (λ p → pr₂ (φ x₀) p refl)
  rs ₁ = different-from-₀-equal-₁ λ p → 𝟘-elim (ne (pr₁ (φ x₁) p))

𝟚-retract-of-discrete : {X : 𝓤 ̇ } {x₀ x₁ : X} → x₀ ≠ x₁ → is-discrete X → retract 𝟚 of X
𝟚-retract-of-discrete {𝓤} {X} {x₀} {x₁} ne d = 𝟚-retract-of-non-trivial-type-with-isolated-point ne (d x₀)

\end{code}

¬¬-Separated types form an exponential ideal, assuming
extensionality. More generally:

\begin{code}

is-¬¬-separated : 𝓤 ̇ → 𝓤 ̇
is-¬¬-separated X = (x y : X) → ¬¬-stable (x ＝ y)

Π-is-¬¬-separated : funext 𝓤 𝓥
                  → {X : 𝓤 ̇ } {Y : X → 𝓥 ̇ }
                  → ((x : X) → is-¬¬-separated (Y x))
                  → is-¬¬-separated (Π Y)
Π-is-¬¬-separated fe s f g h = dfunext fe lemma₂
 where
  lemma₀ : f ＝ g → ∀ x → f x ＝ g x
  lemma₀ r x = ap (λ - → - x) r

  lemma₁ : ∀ x → ¬¬ (f x ＝ g x)
  lemma₁ = double-negation-unshift (¬¬-functor lemma₀ h)

  lemma₂ : ∀ x → f x ＝ g x
  lemma₂ x =  s x (f x) (g x) (lemma₁ x)

discrete-is-¬¬-separated : {X : 𝓤 ̇ } → is-discrete X → is-¬¬-separated X
discrete-is-¬¬-separated d x y = ¬¬-elim (d x y)

𝟚-is-¬¬-separated : is-¬¬-separated 𝟚
𝟚-is-¬¬-separated = discrete-is-¬¬-separated 𝟚-is-discrete

subtype-is-¬¬-separated : {X : 𝓤 ̇ } {Y : 𝓥 ̇ } (m : X → Y)
                                     → left-cancellable m
                                     → is-¬¬-separated Y
                                     → is-¬¬-separated X
subtype-is-¬¬-separated {𝓤} {𝓥} {X} m i s x x' e = i (s (m x) (m x') (¬¬-functor (ap m) e))

\end{code}

The following is an apartness relation when Y is ¬¬-separated, but we
define it without this assumption. (Are all types ¬¬-separated? See
below.)

\begin{code}

infix 21 _♯_

_♯_ : {X : 𝓤 ̇ } → {Y : X → 𝓥 ̇ } → (f g : (x : X) → Y x) → 𝓤 ⊔ 𝓥 ̇
f ♯ g = Σ x ꞉ domain f , f x ≠ g x


apart-is-different : {X : 𝓤 ̇ } {Y : X → 𝓥 ̇ }
                   → {f g : (x : X) → Y x} → f ♯ g → f ≠ g
apart-is-different (x , φ) r = φ (ap (λ - → - x) r)


apart-is-symmetric : {X : 𝓤 ̇ } → {Y : X → 𝓥 ̇ }
                   → {f g : (x : X) → Y x} → f ♯ g → g ♯ f
apart-is-symmetric (x , φ)  = (x , (φ ∘ _⁻¹))

apart-is-cotransitive : {X : 𝓤 ̇ } → {Y : X → 𝓥 ̇ }
                     → ((x : X) → is-discrete (Y x))
                     → (f g h : (x : X) → Y x)
                     → f ♯ g → f ♯ h  +  h ♯ g
apart-is-cotransitive d f g h (x , φ)  = lemma₁ (lemma₀ φ)
 where
  lemma₀ : f x ≠ g x → (f x ≠ h x)  +  (h x ≠ g x)
  lemma₀ = discrete-types-are-cotransitive (d x)

  lemma₁ : (f x ≠ h x) + (h x ≠ g x) → f ♯ h  +  h ♯ g
  lemma₁ (inl γ) = inl (x , γ)
  lemma₁ (inr δ) = inr (x , δ)

\end{code}

We now consider two cases which render the apartness relation ♯ tight,
assuming extensionality:

\begin{code}

tight : {X : 𝓤 ̇ }
      → funext 𝓤 𝓥
      → {Y : X → 𝓥 ̇ }
      → ((x : X) → is-¬¬-separated (Y x))
      → (f g : (x : X) → Y x)
      → ¬ (f ♯ g) → f ＝ g
tight fe s f g h = dfunext fe lemma₁
 where
  lemma₀ : ∀ x → ¬¬ (f x ＝ g x)
  lemma₀ = not-Σ-implies-Π-not h

  lemma₁ : ∀ x → f x ＝ g x
  lemma₁ x = (s x (f x) (g x)) (lemma₀ x)

tight' : {X : 𝓤 ̇ }
       → funext 𝓤 𝓥
       → {Y : X → 𝓥 ̇ }
       → ((x : X) → is-discrete (Y x)) → (f g : (x : X) → Y x) → ¬ (f ♯ g) → f ＝ g
tight' fe d = tight fe (λ x → discrete-is-¬¬-separated (d x))

\end{code}

What about sums? The special case they reduce to binary products is
easy:

\begin{code}

binary-product-is-¬¬-separated : {X : 𝓤 ̇ } {Y : 𝓥 ̇ }
                               → is-¬¬-separated X
                               → is-¬¬-separated Y
                               → is-¬¬-separated (X × Y)
binary-product-is-¬¬-separated s t (x , y) (x' , y') φ =
 lemma (lemma₀ φ) (lemma₁ φ)
 where
  lemma₀ : ¬¬ ((x , y) ＝ (x' , y')) → x ＝ x'
  lemma₀ = (s x x') ∘ ¬¬-functor (ap pr₁)
  lemma₁ : ¬¬ ((x , y) ＝ (x' , y')) → y ＝ y'
  lemma₁ = (t y y') ∘ ¬¬-functor (ap pr₂)
  lemma : x ＝ x' → y ＝ y' → (x , y) ＝ (x' , y')
  lemma = ap₂ (_,_)

\end{code}

This proof doesn't work for general dependent sums, because, among
other things, (ap pr₁) doesn't make sense in that case.  A different
special case is also easy:

\begin{code}

binary-sum-is-¬¬-separated : {X : 𝓤 ̇ } {Y : 𝓥 ̇ }
                           → is-¬¬-separated X
                           → is-¬¬-separated Y
                           → is-¬¬-separated (X + Y)
binary-sum-is-¬¬-separated {𝓤} {𝓥} {X} {Y} s t (inl x) (inl x') = lemma
 where
  claim : inl x ＝ inl x' → x ＝ x'
  claim = ap p
   where
    p : X + Y → X
    p (inl u) = u
    p (inr v) = x

  lemma : ¬¬ (inl x ＝ inl x') → inl x ＝ inl x'
  lemma = ap inl ∘ s x x' ∘ ¬¬-functor claim

binary-sum-is-¬¬-separated s t (inl x) (inr y) =  λ φ → 𝟘-elim (φ +disjoint )
binary-sum-is-¬¬-separated s t (inr y) (inl x)  = λ φ → 𝟘-elim (φ (+disjoint ∘ _⁻¹))
binary-sum-is-¬¬-separated {𝓤} {𝓥} {X} {Y} s t (inr y) (inr y') = lemma
 where
  claim : inr y ＝ inr y' → y ＝ y'
  claim = ap q
   where
    q : X + Y → Y
    q (inl u) = y
    q (inr v) = v

  lemma : ¬¬ (inr y ＝ inr y') → inr y ＝ inr y'
  lemma = (ap inr) ∘ (t y y') ∘ ¬¬-functor claim

⊥-⊤-density' : funext 𝓤 𝓤
             → propext 𝓤
             → ∀ {𝓥} {X : 𝓥 ̇ }
             → is-¬¬-separated X
             → (f : Ω 𝓤 → X) → f ⊥ ＝ f ⊤
             → wconstant f
⊥-⊤-density' fe pe s f r p q = g p ∙ (g q)⁻¹
  where
    a : ∀ p → ¬¬ (f p ＝ f ⊤)
    a p t = no-truth-values-other-than-⊥-or-⊤ fe pe (p , (b , c))
      where
        b : p ≠ ⊥
        b u = t (ap f u ∙ r)

        c : p ≠ ⊤
        c u = t (ap f u)

    g : ∀ p → f p ＝ f ⊤
    g p = s (f p) (f ⊤) (a p)

\end{code}

Added 19th March 2021.

\begin{code}

equality-of-¬¬stable-propositions' : propext 𝓤
                                   → (P Q : 𝓤 ̇ )
                                   → is-prop P
                                   → is-prop Q
                                   → ¬¬-stable P
                                   → ¬¬-stable Q
                                   → ¬¬-stable (P ＝ Q)
equality-of-¬¬stable-propositions' pe P Q i j f g a = V
 where
  I : ¬¬ (P → Q)
  I = ¬¬-functor (transport id) a

  II : P → Q
  II = →-is-¬¬-stable g I

  III : ¬¬ (Q → P)
  III = ¬¬-functor (transport id ∘ _⁻¹) a

  IV : Q → P
  IV = →-is-¬¬-stable f III

  V : P ＝ Q
  V = pe i j II IV

equality-of-¬¬stable-propositions : funext 𝓤 𝓤
                                  → propext 𝓤
                                  → (p q : Ω 𝓤)
                                  → ¬¬-stable (p holds)
                                  → ¬¬-stable (q holds)
                                  → ¬¬-stable (p ＝ q)
equality-of-¬¬stable-propositions fe pe p q f g a = γ
 where
  δ : p holds ＝ q holds
  δ = equality-of-¬¬stable-propositions'
       pe (p holds) (q holds) (holds-is-prop p) (holds-is-prop q)
       f g (¬¬-functor (ap _holds) a)

  γ : p ＝ q
  γ = to-subtype-＝ (λ _ → being-prop-is-prop fe) δ

⊥-⊤-Density : funext 𝓤 𝓤
            → propext 𝓤
            → {X : 𝓥 ̇ }
              (f : Ω 𝓤 → X)
            → is-¬¬-separated X
            → f ⊥ ＝ f ⊤
            → (p : Ω 𝓤) → f p ＝ f ⊤
⊥-⊤-Density fe pe f s r p = s (f p) (f ⊤) a
 where
  a : ¬¬ (f p ＝ f ⊤)
  a u = no-truth-values-other-than-⊥-or-⊤ fe pe (p , b , c)
   where
    b : p ≠ ⊥
    b v = u (ap f v ∙ r)

    c : p ≠ ⊤
    c w = u (ap f w)

⊥-⊤-density : funext 𝓤 𝓤
            → propext 𝓤
            → (f : Ω 𝓤 → 𝟚)
            → f ⊥ ＝ ₁
            → f ⊤ ＝ ₁
            → (p : Ω 𝓤) → f p ＝ ₁
⊥-⊤-density fe pe f r s p = ⊥-⊤-Density fe pe f 𝟚-is-¬¬-separated (r ∙ s ⁻¹) p ∙ s

\end{code}

21 March 2018

\begin{code}

qinvs-preserve-isolatedness : {X : 𝓤 ̇ } {Y : 𝓥 ̇ } (f : X → Y) → qinv f
                            → (x : X) → is-isolated x → is-isolated (f x)
qinvs-preserve-isolatedness {𝓤} {𝓥} {X} {Y} f (g , ε , η) x i y = h (i (g y))
 where
  h : is-decidable (x ＝ g y) → is-decidable (f x ＝ y)
  h (inl p) = inl (ap f p ∙ η y)
  h (inr u) = inr (contrapositive (λ (q : f x ＝ y) → (ε x)⁻¹ ∙ ap g q) u)

equivs-preserve-isolatedness : {X : 𝓤 ̇ } {Y : 𝓥 ̇ } (f : X → Y) → is-equiv f
                             → (x : X) → is-isolated x → is-isolated (f x)
equivs-preserve-isolatedness f e = qinvs-preserve-isolatedness f (equivs-are-qinvs f e)

new-point-is-isolated : {X : 𝓤 ̇ } → is-isolated {𝓤 ⊔ 𝓥} {X + 𝟙 {𝓥}} (inr ⋆)
new-point-is-isolated {𝓤} {𝓥} {X} = h
 where
  h :  (y : X + 𝟙) → is-decidable (inr ⋆ ＝ y)
  h (inl x) = inr +disjoint'
  h (inr ⋆) = inl refl

\end{code}

Back to old stuff:

\begin{code}

＝-indicator :  (m : ℕ) → Σ p ꞉ (ℕ → 𝟚) , ((n : ℕ) → (p n ＝ ₀ → m ≠ n) × (p n ＝ ₁ → m ＝ n))
＝-indicator m = co-characteristic-function (ℕ-is-discrete m)

χ＝ : ℕ → ℕ → 𝟚
χ＝ m = pr₁ (＝-indicator m)

χ＝-spec : (m n : ℕ) → (χ＝ m n ＝ ₀ → m ≠ n) × (χ＝ m n ＝ ₁ → m ＝ n)
χ＝-spec m = pr₂ (＝-indicator m)

_＝[ℕ]_ : ℕ → ℕ → 𝓤₀ ̇
m ＝[ℕ] n = (χ＝ m n) ＝ ₁

infix  30 _＝[ℕ]_

＝-agrees-with-＝[ℕ] : (m n : ℕ) → m ＝ n ⇔ m ＝[ℕ] n
＝-agrees-with-＝[ℕ] m n = (λ r → different-from-₀-equal-₁ (λ s → pr₁ (χ＝-spec m n) s r)) , pr₂ (χ＝-spec m n)

≠-indicator :  (m : ℕ) → Σ p ꞉ (ℕ → 𝟚) , ((n : ℕ) → (p n ＝ ₀ → m ＝ n) × (p n ＝ ₁ → m ≠ n))
≠-indicator m = indicator (ℕ-is-discrete m)

χ≠ : ℕ → ℕ → 𝟚
χ≠ m = pr₁ (≠-indicator m)

χ≠-spec : (m n : ℕ) → (χ≠ m n ＝ ₀ → m ＝ n) × (χ≠ m n ＝ ₁ → m ≠ n)
χ≠-spec m = pr₂ (≠-indicator m)

_≠[ℕ]_ : ℕ → ℕ → 𝓤₀ ̇
m ≠[ℕ] n = (χ≠ m n) ＝ ₁

infix  30 _≠[ℕ]_

≠[ℕ]-agrees-with-≠ : (m n : ℕ) → m ≠[ℕ] n ⇔ m ≠ n
≠[ℕ]-agrees-with-≠ m n = pr₂ (χ≠-spec m n) , (λ d → different-from-₀-equal-₁ (contrapositive (pr₁ (χ≠-spec m n)) d))

\end{code}

Added 14th Feb 2020:

\begin{code}

discrete-exponential-has-decidable-emptiness-of-exponent : {X : 𝓤 ̇ } {Y : 𝓥 ̇ }
                                                         → funext 𝓤 𝓥
                                                         → (Σ y₀ ꞉ Y , Σ y₁ ꞉ Y , y₀ ≠ y₁)
                                                         → is-discrete (X → Y)
                                                         → is-decidable (is-empty X)
discrete-exponential-has-decidable-emptiness-of-exponent {𝓤} {𝓥} {X} {Y} fe (y₀ , y₁ , ne) d = γ
 where
  a : is-decidable ((λ _ → y₀) ＝ (λ _ → y₁))
  a = d (λ _ → y₀) (λ _ → y₁)

  f : is-decidable ((λ _ → y₀) ＝ (λ _ → y₁)) → is-decidable (is-empty X)
  f (inl p) = inl g
   where
    g : is-empty X
    g x = ne q
     where
      q : y₀ ＝ y₁
      q = ap (λ - → - x) p

  f (inr ν) = inr (contrapositive g ν)
   where
    g : is-empty X → (λ _ → y₀) ＝ (λ _ → y₁)
    g ν = dfunext fe (λ x → 𝟘-elim (ν x))

  γ : is-decidable (is-empty X)
  γ = f a

\end{code}

Added by Tom de Jong in January 2022.

Another logical place for these three lemmas would be Negation.lagda, but
(1) the first lemma needs _⇔_ which is defined in Notation.General.lagda, which
    imports Negation.lagda;
(2) the second lemma needs _≃_ which is only defined in UF.Equiv.lagda;
(3) the third lemma needs funext, which is only defined in UF.FunExt.lagda.

\begin{code}

¬¬-stable-⇔ : {X : 𝓤 ̇  } {Y : 𝓥 ̇  }
            → X ⇔ Y
            → ¬¬-stable X
            → ¬¬-stable Y
¬¬-stable-⇔ (f , g) σ h = f (σ (¬¬-functor g h))

¬¬-stable-≃ : {X : 𝓤 ̇  } {Y : 𝓥 ̇  }
            → X ≃ Y
            → ¬¬-stable X
            → ¬¬-stable Y
¬¬-stable-≃ e = ¬¬-stable-⇔ (⌜ e ⌝ , ⌜ e ⌝⁻¹)

being-¬¬-stable-is-prop : {X : 𝓤 ̇  }
                        → funext 𝓤 𝓤
                        → is-prop X → is-prop (¬¬-stable X)
being-¬¬-stable-is-prop fe i = Π-is-prop fe (λ _ → i)

Ω¬¬ : (𝓤 : Universe)  → 𝓤 ⁺ ̇
Ω¬¬ 𝓤 = Σ p ꞉ Ω 𝓤 , ¬¬-stable (p holds)

Ω¬¬-is-¬¬-separated : funext 𝓤 𝓤
                    → propext 𝓤
                    → is-¬¬-separated (Ω¬¬ 𝓤)
Ω¬¬-is-¬¬-separated fe pe (p , s) (q , t) ν = γ
 where
  α : ¬¬ (p ＝ q)
  α = ¬¬-functor (ap pr₁) ν

  δ : p ＝ q
  δ = equality-of-¬¬stable-propositions fe pe p q s t α

  γ : (p , s) ＝ (q , t)
  γ = to-subtype-＝ (λ p → Π-is-prop fe (λ _ → holds-is-prop p)) δ

\end{code}
