```agda

{-# OPTIONS --without-K --exact-split --safe #-}

open import MLTT.Spartan
open import TypeTopology.DiscreteAndSeparated
open import UF.Subsingletons
open import UF.Miscelanea
open import UF.Equiv

module TWA.Thesis.Chapter2.FiniteDiscrete where

open import Naturals.Addition renaming (_+_ to _+â„•_)

is-even : â„• â†’ ğ“¤â‚€ Ì‡
is-even 0 = ğŸ™
is-even 1 = ğŸ˜
is-even (succ (succ n)) = is-even n

â„•â‚‘ : ğ“¤â‚€ Ì‡
â„•â‚‘ = Î£ n ê‰ â„• , is-even n

-- sample-proof : ((n , _) : â„•â‚‘) â†’ Î£ m ê‰ â„• , n +â„• n ï¼ m 
-- Doesn't termination check
{-


sample-proof' : (n : â„•) â†’ is-even n â†’ Î£ m ê‰ â„• , n +â„• n ï¼ m 
sample-proof' 0 â‹†               = 0 , refl
sample-proof' 1 ()
sample-proof' (succ (succ n)) e
 = succ (succ m') , ap (succ âˆ˜ succ) {!e'!}
 where
  IH : Î£ m' ê‰ â„• , ((n +â„• n) ï¼ m')
  IH = sample-proof' n e
  m' = prâ‚ IH
  e' = prâ‚‚ IH

sample-proof : ((n , _) : â„•â‚‘) â†’ Î£ m ê‰ â„• , n +â„• n ï¼ m 
sample-proof (0 , â‹†)  = 0 , refl
sample-proof (1 , ())
sample-proof (succ (succ n) , e)
 = {!!} , {!!}
 where
  IH : Î£ m' ê‰ â„• , ((n +â„• n) ï¼ m')
  IH = sample-proof (n , e)
  m' = prâ‚ IH
  e' = prâ‚‚ IH
-}

ğ”½ : â„• â†’ ğ“¤â‚€  Ì‡
ğ”½ 0 = ğŸ˜
ğ”½ (succ n) = ğŸ™ + ğ”½ n

-- Definition 3.1.6
-- COMMENT: Change to finite-linear-order (see Fin)
finite-discrete : ğ“¤ Ì‡ â†’ ğ“¤  Ì‡
finite-discrete X = Î£ n ê‰ â„• , ğ”½ n â‰ƒ X

-- Lemma 3.1.7
ğ”½-is-discrete : (n : â„•) â†’ is-discrete (ğ”½ n)
ğ”½-is-discrete 0 = ğŸ˜-is-discrete
ğ”½-is-discrete (succ n) = +-is-discrete ğŸ™-is-discrete (ğ”½-is-discrete n)

{- finite-discrete-is-discrete
 : {X : ğ“¤ Ì‡ } â†’ finite-discrete X â†’ is-discrete X
finite-discrete-is-discrete (n , e)
 = equiv-to-discrete e (ğ”½-is-discrete n) -}

-- Extras
ğ”½-is-set : {n : â„•} â†’ is-set (ğ”½ n)
ğ”½-is-set {succ n} = +-is-set ğŸ™ (ğ”½ n) ğŸ™-is-set ğ”½-is-set

finite-is-set : {F : ğ“¤ Ì‡ } â†’ (f : finite-discrete F) â†’ is-set F
finite-is-set (n , f) = equiv-to-set (â‰ƒ-sym f) ğ”½-is-set

ğŸš-finite : finite-discrete ğŸš
ğŸš-finite = 2 , qinveq g (h , Î· , Î¼)
 where
  g : ğ”½ 2 â†’ ğŸš
  g (inl â‹†) = â‚€
  g (inr (inl â‹†)) = â‚
  h : ğŸš â†’ ğ”½ 2
  h â‚€ = inl â‹†
  h â‚ = inr (inl â‹†)
  Î· : h âˆ˜ g âˆ¼ id
  Î· (inl â‹†) = refl
  Î· (inr (inl â‹†)) = refl
  Î¼ : g âˆ˜ h âˆ¼ id
  Î¼ â‚€ = refl
  Î¼ â‚ = refl

```
