\begin{code}

{-# OPTIONS --safe --without-K #-} --

module MLTT.Bool where

open import MLTT.Spartan

data Bool : ğ“¤â‚€ Ì‡ where
 true false : Bool

{-# BUILTIN BOOL  Bool  #-}
{-# BUILTIN FALSE false #-}
{-# BUILTIN TRUE  true  #-}

true-is-not-false : true â‰  false
true-is-not-false ()

if_then_else_ : {X : ğ“¤ Ì‡ } â†’ Bool â†’ X â†’ X â†’ X
if true  then x else y = x
if false then x else y = y

Bool-induction : (A : Bool â†’ ğ“¤ Ì‡ ) â†’ A true â†’ A false â†’ (b : Bool) â†’ A b
Bool-induction A x y true  = x
Bool-induction A x y false = y

Bool-equality-cases : {A : ğ“¤ Ì‡ } (x : Bool) â†’ (x ï¼ true â†’ A) â†’ (x ï¼ false â†’ A) â†’ A
Bool-equality-cases true  f g = f refl
Bool-equality-cases false f g = g refl

not : Bool â†’ Bool
not false = true
not true  = false

_||_ _&&_ : Bool â†’ Bool â†’ Bool

true  || y = true
false || y = y

true  && y = y
false && y = false

true-right-||-absorptive : (x : Bool) â†’ x || true ï¼ true
true-right-||-absorptive true  = refl
true-right-||-absorptive false = refl

||-left-intro : ({x} y : Bool) â†’ x ï¼ true â†’ x || y ï¼ true
||-left-intro {true} y e = refl

||-right-intro : ({x} y : Bool) â†’ y ï¼ true â†’ x || y ï¼ true
||-right-intro {true}  true e = refl
||-right-intro {false} true e = refl

||-gives-+ : {x y : Bool} â†’ x || y ï¼ true â†’ (x ï¼ true) + (y ï¼ true)
||-gives-+ {true}  {y}    _ = inl refl
||-gives-+ {false} {true} _ = inr refl

&&-gives-Ã— : {x y : Bool} â†’ x && y ï¼ true â†’ (x ï¼ true) Ã— (y ï¼ true)
&&-gives-Ã— {true} {true} _ = refl , refl

&&-intro : {x y : Bool} â†’ x ï¼ true â†’ y ï¼ true â†’ x && y ï¼ true
&&-intro {true} {true} refl refl = refl

infixl 10 _||_
infixl 20 _&&_

record Eq {ğ“¤} (X : ğ“¤ Ì‡ ) : ğ“¤ Ì‡  where
  field
    _==_    : X â†’ X â†’ Bool
    ==-refl : (x : X) â†’ (x == x) ï¼ true

open Eq {{...}} public

â„•-== : â„• â†’ â„• â†’ Bool
â„•-== 0        0        = true
â„•-== 0        (succ y) = false
â„•-== (succ x) 0        = false
â„•-== (succ x) (succ y) = â„•-== x y

â„•-refl : (n : â„•) â†’ (â„•-== n n) ï¼ true
â„•-refl 0        = refl
â„•-refl (succ n) = â„•-refl n

instance
 eqâ„• : Eq â„•
 _==_    {{eqâ„•}} = â„•-==
 ==-refl {{eqâ„•}} = â„•-refl


\end{code}
