Taken from the Advanced Functional Programming module lecture notes 2023-24

Provides functions for manipulating isomorphisms

\begin{code}
{-# OPTIONS --without-K --safe #-}

module TGH.AFP2024.iso-utils where

open import MLTT.Spartan renaming (_+_ to _âˆ”_ ; _âˆ™_ to trans)
open import TGH.AFP2024.isomorphisms

open _â‰…_
open is-bijection

id-iso : (A : ğ“¤â‚€ Ì‡) â†’ A â‰… A
id-iso A = record { bijection = f ; bijectivity = f-is-bijection }
 where
  f : A â†’ A
  f = id

  g : A â†’ A
  g = id

  gf : g âˆ˜ f âˆ¼ id
  gf a = refl

  fg : f âˆ˜ g âˆ¼ id
  fg a = refl

  f-is-bijection : is-bijection f
  f-is-bijection = record { inverse = g ; Î· = gf ; Îµ = fg }

â‰…-sym : {X Y : ğ“¤â‚€ Ì‡} â†’ X â‰… Y â†’ Y â‰… X
â‰…-sym (Isomorphism f (Inverse g Î· Îµ)) = Isomorphism g (Inverse f Îµ Î·)

_âˆ˜áµ¢_ : {A B C : ğ“¤â‚€ Ì‡} â†’ B â‰… C â†’ A â‰… B â†’ A â‰… C
Î± âˆ˜áµ¢ Î² = record { bijection = f ; bijectivity = f-is-bijection }
 where
  f : _ â†’ _
  f = bijection Î± âˆ˜ bijection Î²

  g : _ â†’ _
  g = inverse (bijectivity Î²) âˆ˜ inverse (bijectivity Î±)

  gf : g âˆ˜ f âˆ¼ id
  gf a = trans (ap (inverse (bijectivity Î²)) (Î· (bijectivity Î±) (bijection Î² a)))
               (Î· (bijectivity Î²) a)

  fg : f âˆ˜ g âˆ¼ id
  fg c = trans (ap (bijection Î±) (Îµ (bijectivity Î²) (inverse (bijectivity Î±) c)))
               (Îµ (bijectivity Î±) c)

  f-is-bijection : is-bijection f
  f-is-bijection = record { inverse = g ; Î· = gf ; Îµ = fg }

-- Equational reasoning for iso's
_â‰…âŸ¨_âŸ©_ : (X : ğ“¤â‚€ Ì‡) {Y Z : ğ“¤â‚€ Ì‡} â†’ X â‰… Y â†’ Y â‰… Z â†’ X â‰… Z
X â‰…âŸ¨ p âŸ© q = q âˆ˜áµ¢ p

_âˆáµ¢ : (X : ğ“¤â‚€ Ì‡) â†’ X â‰… X
X âˆáµ¢ = id-iso X

infixr  0 _â‰…âŸ¨_âŸ©_
infix   1 _âˆáµ¢

âˆ”-unit-left-iso : (X : ğ“¤â‚€ Ì‡) â†’ X â‰… ğŸ˜ âˆ” X
âˆ”-unit-left-iso X = record { bijection = f ; bijectivity = f-is-bijection }
 where
  f : X â†’ ğŸ˜ âˆ” X
  f x = inr x

  g : ğŸ˜ âˆ” X â†’ X
  g (inr x) = x

  gf : g âˆ˜ f âˆ¼ id
  gf x = refl

  fg : f âˆ˜ g âˆ¼ id
  fg (inr x) = refl

  f-is-bijection : is-bijection f
  f-is-bijection = record { inverse = g ; Î· = gf ; Îµ = fg }
  
âˆ”-pair-iso : {A B C D : ğ“¤â‚€ Ì‡} â†’ A â‰… B â†’ C â‰… D â†’ (A âˆ” C) â‰… (B âˆ” D)
âˆ”-pair-iso {A} {B} {C} {D} Î± Î² = record { bijection = f ; bijectivity = f-is-bijection }
 where
  f : A âˆ” C â†’ B âˆ” D
  f (inl a) = inl (bijection Î± a)
  f (inr c) = inr (bijection Î² c)

  g : B âˆ” D â†’ A âˆ” C
  g (inl b) = inl (inverse (bijectivity Î±) b)
  g (inr d) = inr (inverse (bijectivity Î²) d)

  gf : g âˆ˜ f âˆ¼ id
  gf (inl a) = ap inl (Î· (bijectivity Î±) a)
  gf (inr c) = ap inr (Î· (bijectivity Î²) c)

  fg : f âˆ˜ g âˆ¼ id
  fg (inl b) = ap inl (Îµ (bijectivity Î±) b)
  fg (inr d) = ap inr (Îµ (bijectivity Î²) d)

  f-is-bijection : is-bijection f
  f-is-bijection = record { inverse = g ; Î· = gf ; Îµ = fg }

âˆ”-assoc-iso : (A B C : ğ“¤â‚€ Ì‡) â†’ A âˆ” B âˆ” C â‰… (A âˆ” B) âˆ” C
âˆ”-assoc-iso A B C = record { bijection = f ; bijectivity = f-is-bijection }
 where
  f : A âˆ” B âˆ” C â†’ (A âˆ” B) âˆ” C
  f (inl a) = inl (inl a)
  f (inr (inl b)) = inl (inr b)
  f (inr (inr c)) = inr c

  g : (A âˆ” B) âˆ” C â†’ A âˆ” B âˆ” C
  g (inl (inl a)) = inl a
  g (inl (inr b)) = inr (inl b)
  g (inr c) = inr (inr c)

  gf : g âˆ˜ f âˆ¼ id
  gf (inl a) = refl
  gf (inr (inl b)) = refl
  gf (inr (inr c)) = refl 

  fg : f âˆ˜ g âˆ¼ id
  fg (inl (inl a)) = refl
  fg (inl (inr b)) = refl
  fg (inr c) = refl

  f-is-bijection : is-bijection f
  f-is-bijection = record { inverse = g ; Î· = gf ; Îµ = fg }

âˆ”-left-swap-iso : (A B C : ğ“¤â‚€ Ì‡) â†’ A âˆ” B âˆ” C â‰… B âˆ” A âˆ” C
âˆ”-left-swap-iso A B C = record { bijection = f ; bijectivity = f-is-bijection }
 where
  f : A âˆ” B âˆ” C â†’ B âˆ” A âˆ” C
  f (inl a) = inr (inl a)
  f (inr (inl b)) = inl b
  f (inr (inr c)) = inr (inr c)

  g : B âˆ” A âˆ” C â†’ A âˆ” B âˆ” C
  g (inl b) = inr (inl b)
  g (inr (inl a)) = inl a
  g (inr (inr c)) = inr (inr c)

  gf : g âˆ˜ f âˆ¼ id
  gf (inl a) = refl
  gf (inr (inl b)) = refl
  gf (inr (inr c)) = refl

  fg : f âˆ˜ g âˆ¼ id
  fg (inl b) = refl
  fg (inr (inl a)) = refl
  fg (inr (inr c)) = refl

  f-is-bijection : is-bijection f
  f-is-bijection = record { inverse = g ; Î· = gf ; Îµ = fg }
