{-# OPTIONS --without-K --exact-split --safe #-}

module MLTT-Agda where

open import Universes

variable
 ğ“¤ ğ“¥ ğ“¦ ğ“£ : Universe

data ğŸ™ : ğ“¤â‚€ Ì‡  where
 â‹† : ğŸ™

ğŸ™-induction : (A : ğŸ™ â†’ ğ“¤â€ŠÌ‡ )
            â†’ A â‹† â†’ (x : ğŸ™) â†’ A x
ğŸ™-induction A a â‹† = a

ğŸ™-induction' : (B : ğ“¤â€ŠÌ‡ ) â†’ B â†’ (ğŸ™ â†’ B)
ğŸ™-induction' B b x = ğŸ™-induction (Î» _ â†’ B) b x

!ğŸ™' : (X : ğ“¤â€ŠÌ‡ ) â†’ X â†’ ğŸ™
!ğŸ™' X x = â‹†

!ğŸ™ : {X : ğ“¤â€ŠÌ‡ } â†’ X â†’ ğŸ™
!ğŸ™ x = â‹†

data ğŸ˜ : ğ“¤â‚€â€ŠÌ‡  where

ğŸ˜-induction : (A : ğŸ˜ â†’ ğ“¤ Ì‡ )
            â†’ (x : ğŸ˜) â†’ A x
ğŸ˜-induction A ()

!ğŸ˜ : (A : ğ“¤ Ì‡ ) â†’ ğŸ˜ â†’ A
!ğŸ˜ A a = ğŸ˜-induction (Î» _ â†’ A) a

is-empty : ğ“¤ Ì‡ â†’ ğ“¤ Ì‡
is-empty X = X â†’ ğŸ˜

Â¬ : ğ“¤ Ì‡ â†’ ğ“¤ Ì‡
Â¬ X = X â†’ ğŸ˜

data â„• : ğ“¤â‚€ Ì‡  where
 zero : â„•
 succ : â„• â†’ â„•

{-# BUILTIN NATURAL â„• #-}

â„•-induction : (A : â„• â†’ ğ“¤ Ì‡ )
            â†’ A 0
            â†’ ((n : â„•) â†’ A n â†’ A (succ n))
            â†’ (n : â„•) â†’ A n
â„•-induction A aâ‚€ f = h
 where
  h : (n : â„•) â†’ A n
  h 0        = aâ‚€
  h (succ n) = f n (h n)

â„•-recursion : (X : ğ“¤ Ì‡ )
            â†’ X
            â†’ (â„• â†’ X â†’ X)
            â†’ â„• â†’ X
â„•-recursion X = â„•-induction (Î» _ â†’ X)

â„•-iteration : (X : ğ“¤ Ì‡ )
            â†’ X
            â†’ (X â†’ X)
            â†’ â„• â†’ X
â„•-iteration A a f = â„•-recursion A a (Î» _ a â†’ f a)

module Arithmetic where

  _+_  _Ã—_  : â„• â†’ â„• â†’ â„•

  x + 0      = x
  x + succ y = succ (x + y)

  x Ã— 0      = 0
  x Ã— succ y = x + x Ã— y

  infixl 0 _+_
  infixl 1 _Ã—_

module Arithmetic' where

  _+_  _Ã—_  : â„• â†’ â„• â†’ â„•

  x + y = h y
   where
    h : â„• â†’ â„•
    h = â„•-iteration â„• x succ

  x Ã— y = h y
   where
    h : â„• â†’ â„•
    h = â„•-iteration â„• 0 (x +_)

  infixl 0 _+_
  infixl 1 _Ã—_

module â„•-order where

  _â‰¤_ _â‰¥_ : â„• â†’ â„• â†’ ğ“¤â‚€ Ì‡
  0      â‰¤ y      = ğŸ™
  succ x â‰¤ 0      = ğŸ˜
  succ x â‰¤ succ y = x â‰¤ y

  x â‰¥ y = y â‰¤ x

data _+_ {ğ“¤ ğ“¥} (X : ğ“¤ Ì‡ ) (Y : ğ“¥ Ì‡ ) : ğ“¤ âŠ” ğ“¥ Ì‡  where
 inl : X â†’ X + Y
 inr : Y â†’ X + Y

+-induction : {X : ğ“¤ Ì‡ } {Y : ğ“¥ Ì‡ } (A : X + Y â†’ ğ“¦ Ì‡ )
            â†’ ((x : X) â†’ A(inl x))
            â†’ ((y : Y) â†’ A(inr y))
            â†’ (z : X + Y) â†’ A z
+-induction A f g (inl x) = f x
+-induction A f g (inr y) = g y

ğŸš : ğ“¤â‚€ Ì‡
ğŸš = ğŸ™ + ğŸ™

pattern â‚€ = inl â‹†
pattern â‚ = inr â‹†

ğŸš-induction : (A : ğŸš â†’ ğ“¤ Ì‡ ) â†’ A â‚€ â†’ A â‚ â†’ (n : ğŸš) â†’ A n
ğŸš-induction A aâ‚€ aâ‚ â‚€ = aâ‚€
ğŸš-induction A aâ‚€ aâ‚ â‚ = aâ‚

ğŸš-induction' : (A : ğŸš â†’ ğ“¤ Ì‡ ) â†’ A â‚€ â†’ A â‚ â†’ (n : ğŸš) â†’ A n
ğŸš-induction' A aâ‚€ aâ‚ = +-induction A
                         (ğŸ™-induction (Î» (x : ğŸ™) â†’ A (inl x)) aâ‚€)
                         (ğŸ™-induction (Î» (y : ğŸ™) â†’ A (inr y)) aâ‚)

record Î£ {ğ“¤ ğ“¥} {X : ğ“¤ Ì‡ } (Y : X â†’ ğ“¥ Ì‡ ) : ğ“¤ âŠ” ğ“¥ Ì‡  where
  constructor _,_
  field
   x : X
   y : Y x

prâ‚ : {X : ğ“¤ Ì‡ } {Y : X â†’ ğ“¥ Ì‡ } â†’ Î£ Y â†’ X
prâ‚ (x , y) = x

prâ‚‚ : {X : ğ“¤ Ì‡ } {Y : X â†’ ğ“¥ Ì‡ } â†’ (z : Î£ Y) â†’ Y (prâ‚ z)
prâ‚‚ (x , y) = y

Î£-induction : {X : ğ“¤ Ì‡ } {Y : X â†’ ğ“¥ Ì‡ } {A : Î£ Y â†’ ğ“¦ Ì‡ }
            â†’ ((x : X) (y : Y x) â†’ A(x , y))
            â†’ (z : Î£ Y) â†’ A z
Î£-induction g (x , y) = g x y

curry : {X : ğ“¤ Ì‡ } {Y : X â†’ ğ“¥ Ì‡ } {A : Î£ Y â†’ ğ“¦ Ì‡ }
      â†’ ((z : Î£ Y) â†’ A z)
      â†’ ((x : X) (y : Y x) â†’ A (x , y))
curry f x y = f (x , y)

_Ã—_ : ğ“¤ Ì‡ â†’ ğ“¥ Ì‡ â†’ ğ“¤ âŠ” ğ“¥ Ì‡
X Ã— Y = Î£ \(x : X) â†’ Y

Î  : {X : ğ“¤ Ì‡ } (A : X â†’ ğ“¥ Ì‡ ) â†’ ğ“¤ âŠ” ğ“¥ Ì‡
Î  {ğ“¤} {ğ“¥} {X} A = (x : X) â†’ A x

id : {X : ğ“¤ Ì‡ } â†’ X â†’ X
id x = x

_âˆ˜_ : {X : ğ“¤ Ì‡ } {Y : ğ“¥ Ì‡ } {Z : Y â†’ ğ“¦ Ì‡ }
    â†’ ((y : Y) â†’ Z y)
    â†’ (f : X â†’ Y)
    â†’ (x : X) â†’ Z (f x)
g âˆ˜ f = Î» x â†’ g (f x)

domain : {X : ğ“¤ Ì‡ } {Y : ğ“¥ Ì‡ } â†’ (X â†’ Y) â†’ ğ“¤ Ì‡
domain {ğ“¤} {ğ“¥} {X} {Y} f = X

codomain : {X : ğ“¤ Ì‡ } {Y : ğ“¥ Ì‡ } â†’ (X â†’ Y) â†’ ğ“¥ Ì‡
codomain {ğ“¤} {ğ“¥} {X} {Y} f = Y

type-of : {X : ğ“¤ Ì‡ } â†’ X â†’ ğ“¤ Ì‡
type-of {ğ“¤} {X} x = X

data Id {ğ“¤} (X : ğ“¤ Ì‡ ) : X â†’ X â†’ ğ“¤ Ì‡  where
 refl : (x : X) â†’ Id X x x

_â‰¡_ : {X : ğ“¤ Ì‡ } â†’ X â†’ X â†’ ğ“¤ Ì‡
x â‰¡ y = Id _ x y

J : (X : ğ“¤ Ì‡ ) (A : (x y : X) â†’ x â‰¡ y â†’ ğ“¥ Ì‡ )
  â†’ ((x : X) â†’ A x x (refl x))
  â†’ (x y : X) (p : x â‰¡ y) â†’ A x y p
J X A f x x (refl x) = f x

H : {X : ğ“¤ Ì‡ } (x : X) (B : (y : X) â†’ x â‰¡ y â†’ ğ“¥ Ì‡ )
  â†’ B x (refl x)
  â†’ (y : X) (p : x â‰¡ y) â†’ B y p
H x B b x (refl x) = b

J' : (X : ğ“¤ Ì‡ ) (A : (x y : X) â†’ x â‰¡ y â†’ ğ“¥ Ì‡ )
   â†’ ((x : X) â†’ A x x (refl x))
   â†’ (x y : X) (p : x â‰¡ y) â†’ A x y p
J' X A f x = H x (A x) (f x)

Js-agreement : (X : ğ“¤ Ì‡ ) (A : (x y : X) â†’ x â‰¡ y â†’ ğ“¥ Ì‡ )
               (f : (x : X) â†’ A x x (refl x)) (x y : X) (p : x â‰¡ y)
             â†’ J X A f x y p â‰¡ J' X A f x y p
Js-agreement X A f x x (refl x) = refl (f x)

transport : {X : ğ“¤ Ì‡ } (A : X â†’ ğ“¥ Ì‡ ) {x y : X}
          â†’ x â‰¡ y â†’ A x â†’ A y
transport A (refl x) = id

transportJ : {X : ğ“¤ Ì‡ } (A : X â†’ ğ“¥ Ì‡ ) {x y : X}
           â†’ x â‰¡ y â†’ A x â†’ A y
transportJ {ğ“¤} {ğ“¥} {X} A {x} {y} = J X (Î» x y _ â†’ A x â†’ A y) (Î» x â†’ id) x y

nondep-H : {X : ğ“¤ Ì‡ } (x : X) (A : X â†’ ğ“¥ Ì‡ )
         â†’ A x â†’ (y : X) â†’ x â‰¡ y â†’ A y
nondep-H {ğ“¤} {ğ“¥} {X} x A = H x (Î» y _ â†’ A y)

transportH : {X : ğ“¤ Ì‡ } (A : X â†’ ğ“¥ Ì‡ ) {x y : X}
           â†’ x â‰¡ y â†’ A x â†’ A y
transportH {ğ“¤} {ğ“¥} {X} A {x} {y} p a = nondep-H x A a y p

transports-agreement : {X : ğ“¤ Ì‡ } (A : X â†’ ğ“¥ Ì‡ ) {x y : X} (p : x â‰¡ y)
                     â†’ (transportH A p â‰¡ transportH A p)
                     Ã— (transportJ A p â‰¡ transportH A p)
transports-agreement A (refl x) = refl (transport A (refl x)) ,
                                  refl (transport A (refl x))

lhs : {X : ğ“¤ Ì‡ } {x y : X} â†’ x â‰¡ y â†’ X
lhs {ğ“¤} {X} {x} {y} p = x

rhs : {X : ğ“¤ Ì‡ } {x y : X} â†’ x â‰¡ y â†’ X
rhs {ğ“¤} {X} {x} {y} p = y

_âˆ™_ : {X : ğ“¤ Ì‡ } {x y z : X} â†’ x â‰¡ y â†’ y â‰¡ z â†’ x â‰¡ z
p âˆ™ q = transport (lhs p â‰¡_) q p

_â‰¡âŸ¨_âŸ©_ : {X : ğ“¤ Ì‡ } (x : X) {y z : X} â†’ x â‰¡ y â†’ y â‰¡ z â†’ x â‰¡ z
x â‰¡âŸ¨ p âŸ© q = p âˆ™ q

_âˆ : {X : ğ“¤ Ì‡ } (x : X) â†’ x â‰¡ x
x âˆ = refl x

_â»Â¹ : {X : ğ“¤ Ì‡ } â†’ {x y : X} â†’ x â‰¡ y â†’ y â‰¡ x
p â»Â¹ = transport (_â‰¡ lhs p) p (refl (lhs p))

ap : {X : ğ“¤ Ì‡ } {Y : ğ“¥ Ì‡ } (f : X â†’ Y) {x x' : X} â†’ x â‰¡ x' â†’ f x â‰¡ f x'
ap f p = transport (Î» - â†’ f (lhs p) â‰¡ f -) p (refl (f (lhs p)))

_âˆ¼_ : {X : ğ“¤ Ì‡ } {A : X â†’ ğ“¥ Ì‡ } â†’ ((x : X) â†’ A x) â†’ ((x : X) â†’ A x) â†’ ğ“¤ âŠ” ğ“¥ Ì‡
f âˆ¼ g = âˆ€ x â†’ f x â‰¡ g x

Â¬Â¬ Â¬Â¬Â¬ : ğ“¤ Ì‡ â†’ ğ“¤ Ì‡
Â¬Â¬  A = Â¬(Â¬ A)
Â¬Â¬Â¬ A = Â¬(Â¬Â¬ A)

dni : {A : ğ“¤ Ì‡ } â†’ A â†’ Â¬Â¬ A
dni a u = u a

contrapositive : {A : ğ“¤ Ì‡ } {B : ğ“¤ Ì‡ } â†’ (A â†’ B) â†’ (Â¬ B â†’ Â¬ A)
contrapositive f v a = v (f a)

tno : {A : ğ“¤ Ì‡ } â†’ Â¬Â¬Â¬ A â†’ Â¬ A
tno = contrapositive dni

_â‰¢_ : {X : ğ“¤ Ì‡ } â†’ X â†’ X â†’ ğ“¤ Ì‡
x â‰¢ y = Â¬(x â‰¡ y)

â‰¢-sym : {X : ğ“¤ Ì‡ } {x y : X} â†’ x â‰¢ y â†’ y â‰¢ x
â‰¢-sym {ğ“¤} {X} {x} {y} u = Î» (p : y â‰¡ x) â†’ u (p â»Â¹)

ğŸ™-is-not-ğŸ˜ : Â¬(ğŸ™ â‰¡ ğŸ˜)
ğŸ™-is-not-ğŸ˜ p = f p â‹†
 where
  f : ğŸ™ â‰¡ ğŸ˜ â†’ ğŸ™ â†’ ğŸ˜
  f = transport id

â‚-is-not-â‚€ : Â¬(â‚ â‰¡ â‚€)
â‚-is-not-â‚€ p = ğŸ™-is-not-ğŸ˜ q
 where
  f : ğŸš â†’ ğ“¤â‚€ Ì‡
  f â‚€ = ğŸ˜
  f â‚ = ğŸ™
  q : ğŸ™ â‰¡ ğŸ˜
  q = ap f p

â‚-is-not-â‚€[not-an-MLTT-proof] : Â¬(â‚ â‰¡ â‚€)
â‚-is-not-â‚€[not-an-MLTT-proof] ()

ğŸš-has-decidable-equality : (m n : ğŸš) â†’ (m â‰¡ n) + (m â‰¢ n)
ğŸš-has-decidable-equality â‚€ â‚€ = inl (refl â‚€)
ğŸš-has-decidable-equality â‚€ â‚ = inr (â‰¢-sym â‚-is-not-â‚€)
ğŸš-has-decidable-equality â‚ â‚€ = inr â‚-is-not-â‚€
ğŸš-has-decidable-equality â‚ â‚ = inl (refl â‚)

not-zero-is-one : (n : ğŸš) â†’ n â‰¢ â‚€ â†’ n â‰¡ â‚
not-zero-is-one â‚€ f = !ğŸ˜ (â‚€ â‰¡ â‚) (f (refl â‚€))
not-zero-is-one â‚ f = refl â‚

inl-inr-disjoint-images : {X : ğ“¤ Ì‡ } {Y : ğ“¥ Ì‡ } {x : X} {y : Y} â†’ inl x â‰¢ inr y
inl-inr-disjoint-images {ğ“¤} {ğ“¥} {X} {Y} p = ğŸ™-is-not-ğŸ˜ r
 where
  f : X + Y â†’ ğ“¤â‚€ Ì‡
  f (inl x) = ğŸ™
  f (inr y) = ğŸ˜
  r : ğŸ™ â‰¡ ğŸ˜
  r = ap f p

module twin-primes where

 open Arithmetic renaming (_Ã—_ to _*_ ; _+_ to _âˆ”_)
 open â„•-order

 is-prime : â„• â†’ ğ“¤â‚€ Ì‡
 is-prime n = (n â‰¥ 2) Ã— ((x y : â„•) â†’ x * y â‰¡ n â†’ (x â‰¡ 1) + (x â‰¡ n))

 twin-prime-conjecture : ğ“¤â‚€ Ì‡
 twin-prime-conjecture = (n : â„•) â†’ Î£ \(p : â„•) â†’ (p â‰¥ n) Ã— is-prime p Ã— is-prime (p âˆ” 2)

infix  4  _âˆ¼_
infixr 4 _,_
infixr 2 _Ã—_
infixr 1 _+_
infixl 5 _âˆ˜_
infix  0 _â‰¡_
infixl 2 _âˆ™_
infixr 0 _â‰¡âŸ¨_âŸ©_
infix  1 _âˆ
infix  3  _â»Â¹

