Tom de Jong, Nicolai Kraus, Fredrik Nordvall Forsberg, Chuangjie Xu,
13 November 2023.

\begin{code}

{-# OPTIONS --safe --without-K --no-exact-split #-}

open import UF.Univalence

module Ordinals.Exponentiation
       (ua : Univalence)
       where

open import UF.Base
open import UF.Embeddings hiding (âŒŠ_âŒ‹)
open import UF.Equiv
open import UF.EquivalenceExamples
open import UF.ExcludedMiddle
open import UF.FunExt
open import UF.Sets
open import UF.Subsingletons
open import UF.Subsingletons-FunExt
open import UF.UA-FunExt

private
 fe : FunExt
 fe = Univalence-gives-FunExt ua

 fe' : Fun-Ext
 fe' {ğ“¤} {ğ“¥} = fe ğ“¤ ğ“¥

 pe : PropExt
 pe = Univalence-gives-PropExt ua

open import MLTT.Plus-Properties
open import MLTT.Spartan
open import MLTT.Sigma
-- open import Notation.CanonicalMap
open import Ordinals.Arithmetic fe
open import Ordinals.ArithmeticProperties ua
open import Ordinals.ConvergentSequence ua
open import Ordinals.Equivalence
open import Ordinals.Maps
open import Ordinals.Notions
open import Ordinals.OrdinalOfOrdinals ua
open import Ordinals.Type
open import Ordinals.Underlying

-- our imports
open import MLTT.List


data lex {X : ğ“¤ Ì‡  } (R : X â†’ X â†’ ğ“¥ Ì‡  ) : List X â†’ List X â†’ ğ“¤ âŠ” ğ“¥ Ì‡  where
 []-lex : {y : X}{ys : List X} â†’ lex R [] (y âˆ· ys)
 head-lex : {x y : X}{xs ys : List X} â†’ R x y â†’ lex R (x âˆ· xs) (y âˆ· ys)
 tail-lex : {x y : X}{xs ys : List X} â†’ x ï¼ y â†’ lex R xs ys â†’ lex R (x âˆ· xs) (y âˆ· ys)

lex-for-ordinal : (Î± : Ordinal ğ“¤) â†’ List âŸ¨ Î± âŸ© â†’ List âŸ¨ Î± âŸ© â†’ ğ“¤ Ì‡
lex-for-ordinal Î± = lex (underlying-order Î±)

syntax lex-for-ordinal Î± xs ys = xs â‰ºâŸ¨List Î± âŸ© ys

is-irreflexive : {X : ğ“¤ Ì‡  } (R : X â†’ X â†’ ğ“¥ Ì‡  ) â†’ ğ“¤ âŠ” ğ“¥ Ì‡
is-irreflexive R = âˆ€ x â†’ Â¬ (R x x)

module _ {X : ğ“¤ Ì‡  } (R : X â†’ X â†’ ğ“¥ Ì‡  ) where

 lex-transitive : is-transitive R â†’ is-transitive (lex R)
 lex-transitive tr [] (y âˆ· ys) (z âˆ· zs) []-lex (head-lex q) = []-lex
 lex-transitive tr [] (y âˆ· ys) (z âˆ· zs) []-lex (tail-lex r q) = []-lex
 lex-transitive tr (x âˆ· xs) (y âˆ· ys) (z âˆ· zs) (head-lex p) (head-lex q) = head-lex (tr x y z p q)
 lex-transitive tr (x âˆ· xs) (y âˆ· ys) (.y âˆ· zs) (head-lex p) (tail-lex refl q) = head-lex p
 lex-transitive tr (x âˆ· xs) (.x âˆ· ys) (z âˆ· zs) (tail-lex refl p) (head-lex q) = head-lex q
 lex-transitive tr (x âˆ· xs) (.x âˆ· ys) (.x âˆ· zs) (tail-lex refl p) (tail-lex refl q)
  = tail-lex refl (lex-transitive tr xs ys zs p q)

 []-lex-bot : is-bot (lex R) []
 []-lex-bot xs ()

 data is-decreasing : List X â†’ ğ“¤ âŠ” ğ“¥ Ì‡  where
  []-decr : is-decreasing []
  sing-decr : {x : X} â†’ is-decreasing [ x ]
  many-decr : {x y : X}{xs : List X} â†’ R y x â†’ is-decreasing (y âˆ· xs) â†’ is-decreasing (x âˆ· y âˆ· xs)

 is-decreasing-propositional : ((x y : X) â†’ is-prop (R x y))
                             â†’ (xs : List X) â†’ is-prop (is-decreasing xs)
 is-decreasing-propositional pR [] []-decr []-decr = refl
 is-decreasing-propositional pR (x âˆ· []) sing-decr sing-decr = refl
 is-decreasing-propositional pR (x âˆ· y âˆ· xs) (many-decr p ps) (many-decr q qs) =
  apâ‚‚ many-decr (pR y x p q) (is-decreasing-propositional pR (y âˆ· xs) ps qs)

 is-decreasing-tail : {x : X} {xs : List X} â†’ is-decreasing (x âˆ· xs) â†’ is-decreasing xs
 is-decreasing-tail sing-decr = []-decr
 is-decreasing-tail (many-decr _ d) = d

 is-decreasing-heads : {x y : X} {xs : List X} â†’ is-decreasing (x âˆ· y âˆ· xs) â†’ R y x
 is-decreasing-heads (many-decr p _) = p

 DecreasingList : (ğ“¤ âŠ” ğ“¥) Ì‡
 DecreasingList = Î£ xs ê‰ List X , is-decreasing xs

 lex-decr : DecreasingList â†’ DecreasingList â†’ ğ“¤ âŠ” ğ“¥ Ì‡
 lex-decr (xs , _) (ys , _) = lex R xs ys
\end{code}

\begin{code}
 []-acc-decr : {p : is-decreasing []} â†’ is-accessible lex-decr ([] , p)
 []-acc-decr {[]-decr} = acc (Î» xs q â†’ ğŸ˜-elim ([]-lex-bot _ q))

 lex-decr-acc : is-transitive R
              â†’ (x : X) â†’ is-accessible R x
              â†’ (xs : List X) (Î´ : is-decreasing xs)
              â†’ is-accessible lex-decr (xs , Î´)
              â†’ (Îµ : is-decreasing (x âˆ· xs))
              â†’ is-accessible lex-decr ((x âˆ· xs) , Îµ)
 lex-decr-acc tr =
  transfinite-induction' R P Ï•
    where
     Q : X â†’ DecreasingList â†’ ğ“¤ âŠ” ğ“¥ Ì‡
     Q x (xs , _) = (Îµ' : is-decreasing (x âˆ· xs)) â†’ is-accessible lex-decr ((x âˆ· xs) , Îµ')
     P : X â†’ ğ“¤ âŠ” ğ“¥ Ì‡
     P x = (xs : List X) (Î´ : is-decreasing xs)
         â†’ is-accessible lex-decr (xs , Î´)
         â†’ Q x (xs , Î´)

     Ï• : (x : X) â†’ ((y : X) â†’ R y x â†’ P y) â†’ P x
     Ï• x IH xs Î´ Î² = transfinite-induction' lex-decr (Q x) (Î» (xs , Îµ) â†’ Ï•' xs Îµ) (xs , Î´) Î²
      where
       Ï•' : (xs : List X) â†’ (Îµ : is-decreasing xs)
          â†’ ((ys : DecreasingList) â†’ lex-decr ys (xs , Îµ) â†’ Q x ys)
          â†’ Q x (xs , Îµ)
       Ï•' xs _ IHâ‚‚ Îµ' = acc (Î» (ys , Îµ) â†’ g ys Îµ)
        where
         g : (ys : List X) â†’ (Îµ : is-decreasing ys)
            â†’ lex-decr (ys , Îµ) ((x âˆ· xs) , Îµ')
            â†’ is-accessible lex-decr (ys , Îµ)
         g [] Îµ p = []-acc-decr
         g (y âˆ· []) Îµ (head-lex p) = IH y p [] []-decr []-acc-decr Îµ
         g (y âˆ· z âˆ· ys) Îµ (head-lex p) =
           IH y p (z âˆ· ys) (is-decreasing-tail Îµ)
              (g (z âˆ· ys) (is-decreasing-tail Îµ) (head-lex (tr z y x (is-decreasing-heads Îµ) p)))
              Îµ
         g (.x âˆ· ys) Îµ (tail-lex refl l) = IHâ‚‚ (ys , is-decreasing-tail Îµ) l Îµ

 lex-wellfounded : is-transitive R â†’ is-well-founded R â†’ is-well-founded lex-decr
 lex-wellfounded tr wf (xs , Î´) = lex-wellfounded' wf xs Î´
  where
   lex-wellfounded' : is-well-founded R
                    â†’ (xs : List X) (Î´ : is-decreasing xs)
                    â†’ is-accessible lex-decr (xs , Î´)
   lex-wellfounded' wf [] Î´ = []-acc-decr
   lex-wellfounded' wf (x âˆ· xs) Î´ =
     lex-decr-acc tr
                  x
                  (wf x)
                  xs
                  (is-decreasing-tail Î´)
                  (lex-wellfounded' wf xs (is-decreasing-tail Î´))
                  Î´
\end{code}

\begin{code}

 lex-irreflexive : is-irreflexive R â†’ is-irreflexive (lex R)
 lex-irreflexive ir (x âˆ· xs) (head-lex p) = ir x p
 lex-irreflexive ir (x âˆ· xs) (tail-lex e q) = lex-irreflexive ir xs q

 -- this is not helpful below
 lex-extensional : is-irreflexive R â†’ is-extensional R â†’ is-extensional (lex R)
 lex-extensional ir ext [] [] p q = refl
 lex-extensional ir ext [] (y âˆ· ys) p q = ğŸ˜-elim ([]-lex-bot [] (q [] []-lex))
 lex-extensional ir ext (x âˆ· xs) [] p q = ğŸ˜-elim ([]-lex-bot [] (p [] []-lex))
 lex-extensional ir ext (x âˆ· xs) (y âˆ· ys) p q = apâ‚‚ _âˆ·_ eâ‚€ eâ‚
  where
   pâ‚€ : âˆ€ z â†’ R z x â†’ R z y
   pâ‚€ z zRx with (p (z âˆ· ys) (head-lex zRx))
   pâ‚€ z zRx | head-lex zRy = zRy
   pâ‚€ z zRx | tail-lex _ ysRys = ğŸ˜-elim (lex-irreflexive ir ys ysRys)
   qâ‚€ : âˆ€ z â†’ R z y â†’ R z x
   qâ‚€ z zRy with (q (z âˆ· xs) (head-lex zRy))
   qâ‚€ z zRy | head-lex zRx = zRx
   qâ‚€ z zRy | tail-lex _ xsRxs = ğŸ˜-elim (lex-irreflexive ir xs xsRxs)
   eâ‚€ : x ï¼ y
   eâ‚€ = ext x y pâ‚€ qâ‚€
   pâ‚ : âˆ€ zs â†’ lex R zs xs â†’ lex R zs ys
   pâ‚ zs zsRxs with (p (x âˆ· zs) (tail-lex refl zsRxs))
   pâ‚ zs zsRxs | head-lex xRy = ğŸ˜-elim (ir y (transport (Î» z â†’ R z y) eâ‚€ xRy))
   pâ‚ zs zsRxs | tail-lex _ zsRys = zsRys
   qâ‚ : âˆ€ zs â†’ lex R zs ys â†’ lex R zs xs
   qâ‚ zs zsRys with (q (y âˆ· zs) (tail-lex refl zsRys))
   qâ‚ zs zsRys | head-lex yRx = ğŸ˜-elim (ir y (transport (Î» z â†’ R y z) eâ‚€ yRx))
   qâ‚ zs zsRys | tail-lex _ zsRxs = zsRxs
   eâ‚ : xs ï¼ ys
   eâ‚ = lex-extensional ir ext xs ys pâ‚ qâ‚

\end{code}

\begin{code}

 lex-prop-valued : is-set X â†’ is-prop-valued R â†’ is-irreflexive R â†’ is-prop-valued (lex R)
 lex-prop-valued st pr irR [] (y âˆ· ys) []-lex []-lex = refl
 lex-prop-valued st pr irR (x âˆ· xs) (y âˆ· ys) (head-lex p) (head-lex q) = ap head-lex (pr x y p q)
 lex-prop-valued st pr irR (.y âˆ· xs) (y âˆ· ys) (head-lex p) (tail-lex refl qs) = ğŸ˜-elim (irR y p)
 lex-prop-valued st pr irR (x âˆ· xs) (.x âˆ· ys) (tail-lex refl ps) (head-lex q) = ğŸ˜-elim (irR x q)
 lex-prop-valued st pr irR (x âˆ· xs) (y âˆ· ys) (tail-lex e ps) (tail-lex r qs) =
  apâ‚‚ tail-lex (st e r) (lex-prop-valued st pr irR xs ys ps qs)

\end{code}

\begin{code}


-- can we get away with different universes like this?
module _ (Î± : Ordinal ğ“¤)(Î² : Ordinal ğ“¥) where

 âŸ¨[ğŸ™+_]^_âŸ© : ğ“¤ âŠ” ğ“¥ Ì‡
 âŸ¨[ğŸ™+_]^_âŸ© = Î£ xs ê‰ List âŸ¨ Î² Ã—â‚’ Î± âŸ© , is-decreasing (underlying-order Î±) (map prâ‚‚ xs)

 to-exponential-ï¼ : {xs ys : âŸ¨[ğŸ™+_]^_âŸ©} â†’ prâ‚ xs ï¼ prâ‚ ys â†’ xs ï¼ ys
 to-exponential-ï¼ = to-subtype-ï¼ (Î» xs â†’ is-decreasing-propositional
                                            (underlying-order Î±)
                                            (Prop-valuedness Î±)
                                            (map prâ‚‚ xs))



 underlying-list : âŸ¨[ğŸ™+_]^_âŸ© â†’ List âŸ¨ Î² Ã—â‚’ Î± âŸ©
 underlying-list (xs , _) = xs

 underlying-list-decreasing-base : (xs : âŸ¨[ğŸ™+_]^_âŸ©) â†’ is-decreasing (underlying-order Î±) (map prâ‚‚ (underlying-list xs))
 underlying-list-decreasing-base (xs , p) = p

 underlying-list-decreasing : (xs : âŸ¨[ğŸ™+_]^_âŸ©) â†’ is-decreasing (underlying-order (Î² Ã—â‚’ Î±)) (underlying-list xs)
 underlying-list-decreasing (xs , p) = is-decreasing-prâ‚‚-to-is-decreasing xs p
  where
   is-decreasing-prâ‚‚-to-is-decreasing : (xs : List âŸ¨ Î² Ã—â‚’ Î± âŸ©)
                                      â†’ is-decreasing (underlying-order Î±) (map prâ‚‚ xs)
                                      â†’ is-decreasing (underlying-order (Î² Ã—â‚’ Î±)) xs
   is-decreasing-prâ‚‚-to-is-decreasing [] _ = []-decr
   is-decreasing-prâ‚‚-to-is-decreasing (x âˆ· []) _ = sing-decr
   is-decreasing-prâ‚‚-to-is-decreasing (x âˆ· x' âˆ· xs) (many-decr p ps)
    = many-decr (inl p) (is-decreasing-prâ‚‚-to-is-decreasing (x' âˆ· xs) ps)

 exponential-order : âŸ¨[ğŸ™+_]^_âŸ© â†’ âŸ¨[ğŸ™+_]^_âŸ© â†’ ğ“¤ âŠ” ğ“¥ Ì‡
 exponential-order (xs , _) (ys , _) = xs â‰ºâŸ¨List (Î² Ã—â‚’ Î±) âŸ© ys

 exponential-order-prop-valued : is-prop-valued exponential-order
 exponential-order-prop-valued (xs , _) (ys , _)
   = lex-prop-valued _ (underlying-type-is-set fe (Î² Ã—â‚’ Î±))
                       (Prop-valuedness (Î² Ã—â‚’ Î±))
                       (irrefl (Î² Ã—â‚’ Î±))
                       xs
                       ys

 exponential-order-wellfounded : is-well-founded exponential-order
 exponential-order-wellfounded (xs , Î´) =
  acc-lex-decr-to-acc-exponential xs Î´ (lex-wellfounded (underlying-order (Î² Ã—â‚’ Î±)) (Transitivity (Î² Ã—â‚’ Î±)) (Well-foundedness (Î² Ã—â‚’ Î±)) _)
  where
   acc-lex-decr-to-acc-exponential : (xs : List âŸ¨ Î² Ã—â‚’ Î± âŸ©)
                                   â†’ (Î´ : is-decreasing (underlying-order Î±) (map prâ‚‚ xs))
                                   â†’ is-accessible (lex-decr (underlying-order (Î² Ã—â‚’ Î±))) ((xs , underlying-list-decreasing (xs , Î´)))
                                   â†’ is-accessible exponential-order (xs , Î´)
   acc-lex-decr-to-acc-exponential xs Î´ (acc h) =
    acc Î» (ys , Îµ) ys<xs â†’ acc-lex-decr-to-acc-exponential ys Îµ (h (ys ,  underlying-list-decreasing (ys , Îµ)) ys<xs)

 private
  R = underlying-order (Î² Ã—â‚’ Î±)
  decreasing-prâ‚‚ : List âŸ¨ Î² Ã—â‚’ Î± âŸ© â†’ ğ“¤ Ì‡
  decreasing-prâ‚‚ xs = is-decreasing (underlying-order Î±) (map prâ‚‚ xs)


 -- TODO: CLEAN UP
 -- TODO: Rename
 lemma' : (xs ys : List âŸ¨ Î² Ã—â‚’ Î± âŸ©) (x : âŸ¨ Î² Ã—â‚’ Î± âŸ©)
        â†’ decreasing-prâ‚‚ (x âˆ· xs)
        â†’ decreasing-prâ‚‚ ys
        â†’ lex R ys xs
        â†’ decreasing-prâ‚‚ (x âˆ· ys)
 lemma' (x' âˆ· xs) [] x Î´ Îµ l = sing-decr
 lemma' (x' âˆ· xs) (y âˆ· ys) x (many-decr l Î´) Îµ (head-lex (inl k)) =
  many-decr (Transitivity Î± (prâ‚‚ y) (prâ‚‚ x') (prâ‚‚ x) k l) Îµ
 lemma' ((xâ‚' , _) âˆ· xs) ((yâ‚ , yâ‚‚) âˆ· ys) (xâ‚ , xâ‚‚) Î´ Îµ (head-lex (inr (refl , k))) =
  many-decr (is-decreasing-heads (underlying-order Î±) Î´) Îµ
 lemma' (_ âˆ· xs) (y âˆ· ys) x Î´ Îµ (tail-lex refl l) =
  many-decr (is-decreasing-heads (underlying-order Î±) Î´) Îµ

 -- TODO: Rename
 lemma : (xs ys : List âŸ¨ Î² Ã—â‚’ Î± âŸ©) (x : âŸ¨ Î² Ã—â‚’ Î± âŸ©)
       â†’ decreasing-prâ‚‚ (x âˆ· xs) â†’ decreasing-prâ‚‚ (x âˆ· ys)
       â†’ ((zs : List âŸ¨ Î² Ã—â‚’ Î± âŸ©)
              â†’ decreasing-prâ‚‚ zs
              â†’ lex R zs (x âˆ· xs) â†’ lex R zs (x âˆ· ys)) -- TODO: Use â‰¤
       â†’ ((zs : List âŸ¨ Î² Ã—â‚’ Î± âŸ©)
              â†’ decreasing-prâ‚‚ zs
              â†’ lex R zs xs â†’ lex R zs ys) -- TODO: Use â‰¤
 lemma xs ys x Î´ Îµ h zs Îµ' l = g hâ‚“
  where
   hâ‚“ : lex R (x âˆ· zs) (x âˆ· ys)
   hâ‚“ = h (x âˆ· zs) lem (tail-lex refl l)
    where
     lem : decreasing-prâ‚‚ (x âˆ· zs)
     lem = lemma' xs zs x Î´ Îµ' l
   g : lex R (x âˆ· zs) (x âˆ· ys) â†’ lex R zs ys
   g (head-lex r) = ğŸ˜-elim (irreflexive R x (Well-foundedness (Î² Ã—â‚’ Î±) x) r)
   g (tail-lex _ k) = k


 exponential-order-extensional : is-extensional exponential-order
 exponential-order-extensional (xs , Î´) (ys , Îµ) p q =
  to-exponential-ï¼ (exponential-order-extensional' xs Î´ ys Îµ (Î» zs Îµ' â†’ p (zs , Îµ')) (Î» zs Îµ' â†’ q (zs , Îµ')))
  where
   exponential-order-extensional' : (xs : List âŸ¨ Î² Ã—â‚’ Î± âŸ©)
                                  â†’ (Î´ : decreasing-prâ‚‚ xs)
                                  â†’ (ys : List âŸ¨ Î² Ã—â‚’ Î± âŸ©)
                                  â†’ (Îµ : decreasing-prâ‚‚ ys)
                                  â†’ ((zs : List âŸ¨ Î² Ã—â‚’ Î± âŸ©) â†’ decreasing-prâ‚‚ zs â†’ lex R zs xs â†’ lex R zs ys )
                                  â†’ ((zs : List âŸ¨ Î² Ã—â‚’ Î± âŸ©) â†’ decreasing-prâ‚‚ zs â†’ lex R zs ys â†’ lex R zs xs )
                                  â†’ xs ï¼ ys
   exponential-order-extensional' [] Î´ [] Îµ p q = refl
   exponential-order-extensional' [] Î´ (y âˆ· ys) Îµ p q =
    ğŸ˜-elim ([]-lex-bot _ [] (q [] Î´ []-lex))
   exponential-order-extensional' (x âˆ· xs) Î´ [] Îµ p q =
    ğŸ˜-elim ([]-lex-bot _ [] (p [] Îµ []-lex))
   exponential-order-extensional' (x âˆ· []) Î´ (y âˆ· []) Îµ p q =
     ap [_] (Extensionality (Î² Ã—â‚’ Î±) x y eâ‚ eâ‚‚)
      where
       eâ‚ : âˆ€ z â†’ R z x â†’ R z y
       eâ‚ z r = h p'
        where
         h : lex R [ z ] [ y ] â†’ R z y
         h (head-lex r') = r'
         p' : lex R [ z ] [ y ]
         p' = p [ z ] sing-decr (head-lex r)
       eâ‚‚ : âˆ€ z â†’ R z y â†’ R z x
       eâ‚‚ z r = h q'
        where
         h : lex R [ z ] [ x ] â†’ R z x
         h (head-lex r') = r'
         q' : lex R [ z ] [ x ]
         q' = q [ z ] sing-decr (head-lex r)
   exponential-order-extensional' (x âˆ· []) Î´ (y âˆ· y' âˆ· ys) Îµ p q = V
    where
     I : lex R [ y ] (y âˆ· y' âˆ· ys)
     I = tail-lex refl []-lex
     II : R y x
     II = h q'
      where
       h : lex R [ y ] [ x ] â†’ R y x
       h (head-lex r) = r
       q' : lex R [ y ] [ x ]
       q' = q [ y ] sing-decr I
     III : lex R (y âˆ· y' âˆ· ys) [ x ]
     III = head-lex II
     IV : lex R (y âˆ· y' âˆ· ys) (y âˆ· y' âˆ· ys)
     IV = p (y âˆ· y' âˆ· ys) Îµ III
     V : [ x ] ï¼ y âˆ· y' âˆ· ys
     V = ğŸ˜-elim
          (lex-irreflexive R
            (Î» x â†’ irreflexive R x (Well-foundedness (Î² Ã—â‚’ Î±) x))
           (y âˆ· y' âˆ· ys) IV)
   exponential-order-extensional' (x âˆ· x' âˆ· xs) Î´ (y âˆ· []) Îµ p q = V -- TODO: Factor out
    where
     I : lex R [ x ] (x âˆ· x' âˆ· xs)
     I = tail-lex refl []-lex
     II : R x y
     II = h p'
      where
       h : lex R [ x ] [ y ] â†’ R x y
       h (head-lex r) = r
       p' : lex R [ x ] [ y ]
       p' = p [ x ] sing-decr I
     III : lex R (x âˆ· x' âˆ· xs) [ y ]
     III = head-lex II
     IV : lex R (x âˆ· x' âˆ· xs) (x âˆ· x' âˆ· xs)
     IV = q (x âˆ· x' âˆ· xs) Î´ III
     V : x âˆ· x' âˆ· xs ï¼ [ y ]
     V = ğŸ˜-elim
          (lex-irreflexive R
            (Î» y â†’ irreflexive R y (Well-foundedness (Î² Ã—â‚’ Î±) y))
           (x âˆ· x' âˆ· xs) IV)
   exponential-order-extensional' (x âˆ· x' âˆ· xs) Î´ (y âˆ· y' âˆ· ys) Îµ p q =
    apâ‚‚ _âˆ·_ e
            (exponential-order-extensional'
             (x' âˆ· xs) (is-decreasing-tail (underlying-order Î±) Î´)
             (y' âˆ· ys) (is-decreasing-tail (underlying-order Î±) Îµ)
             (p' e) (q' e))
     where
      e : x ï¼ y
      e = g II II'
       where
        I : lex R [ x ] (x âˆ· x' âˆ· xs)
        I = tail-lex refl []-lex
        II : lex R [ x ] (y âˆ· y' âˆ· ys)
        II = p [ x ] sing-decr I
        I' : lex R [ y ] (y âˆ· y' âˆ· ys)
        I' = tail-lex refl []-lex
        II' : lex R [ y ] (x âˆ· x' âˆ· xs)
        II' = q [ y ] sing-decr I'
        g : lex R [ x ] (y âˆ· y' âˆ· ys)
          â†’ lex R [ y ] (x âˆ· x' âˆ· xs)
          â†’ x ï¼ y
        g (head-lex r) (head-lex r') =
         ğŸ˜-elim (irreflexive R x (Well-foundedness (Î² Ã—â‚’ Î±) x) (Transitivity (Î² Ã—â‚’ Î±) x y x r r'))
        g (head-lex _) (tail-lex eq _) = eq â»Â¹
        g (tail-lex eq _) _ = eq
      p' : (x ï¼ y) â†’ (zs : List âŸ¨ Î² Ã—â‚’ Î± âŸ©)
         â†’ decreasing-prâ‚‚ zs
         â†’ lex R zs (x' âˆ· xs)
         â†’ lex R zs (y' âˆ· ys)
      p' refl = lemma (x' âˆ· xs) (y' âˆ· ys) x Î´ Îµ p
      q' : (x ï¼ y) â†’ (zs : List âŸ¨ Î² Ã—â‚’ Î± âŸ©)
         â†’ decreasing-prâ‚‚ zs
         â†’ lex R zs (y' âˆ· ys)
         â†’ lex R zs (x' âˆ· xs)
      q' refl = lemma (y' âˆ· ys) (x' âˆ· xs) y Îµ Î´ q


 exponential-order-transitive : is-transitive exponential-order
 exponential-order-transitive (xs , _) (ys , _) (zs , _) p q =
  lex-transitive (underlying-order (Î² Ã—â‚’ Î±)) (Transitivity (Î² Ã—â‚’ Î±)) xs ys zs p q

[ğŸ™+_]^_ : Ordinal ğ“¤ â†’ Ordinal ğ“¥ â†’ Ordinal (ğ“¤ âŠ” ğ“¥)
[ğŸ™+ Î± ]^ Î² = âŸ¨[ğŸ™+ Î± ]^ Î² âŸ©
           , exponential-order Î± Î²
           , exponential-order-prop-valued Î± Î²
           , exponential-order-wellfounded Î± Î²
           , exponential-order-extensional Î± Î²
           , exponential-order-transitive Î± Î²

-- End goal: prove it satisfies (0, succ, sup)-spec

exp-0-spec' : (Î± : Ordinal ğ“¤) â†’ ([ğŸ™+ Î± ]^ (ğŸ˜â‚’ {ğ“¥})) â‰ƒâ‚’ ğŸ™â‚’ {ğ“¤ âŠ” ğ“¥}
exp-0-spec' Î± = f , f-monotone , qinvs-are-equivs f f-qinv , g-monotone
 where
  f : âŸ¨ [ğŸ™+ Î± ]^ ğŸ˜â‚’ âŸ© â†’ ğŸ™
  f _ = â‹†
  f-monotone : is-order-preserving ([ğŸ™+ Î± ]^ ğŸ˜â‚’) ğŸ™â‚’ (Î» _ â†’ â‹†)
  f-monotone ([] , Î´) ([] , Îµ) u =
    ğŸ˜-elim
     (irreflexive
      (exponential-order Î± ğŸ˜â‚’)
      ([] , Î´)
      (exponential-order-wellfounded Î± ğŸ˜â‚’ _) u)
  g : ğŸ™ â†’ âŸ¨ [ğŸ™+ Î± ]^ ğŸ˜â‚’ âŸ©
  g _ = [] , []-decr
  g-monotone : is-order-preserving ğŸ™â‚’ ([ğŸ™+ Î± ]^ ğŸ˜â‚’) g
  g-monotone â‹† â‹† u = ğŸ˜-elim u
  f-qinv : qinv f
  f-qinv = g , p , q
   where
    p : (Î» x â†’ [] , []-decr) âˆ¼ id
    p ([] , Î´) = to-exponential-ï¼ Î± ğŸ˜â‚’ refl
    q : (Î» x â†’ â‹†) âˆ¼ id
    q â‹† = refl

exp-0-spec : (Î± : Ordinal ğ“¤) â†’ [ğŸ™+ Î± ]^ (ğŸ˜â‚’ {ğ“¥}) ï¼ ğŸ™â‚’
exp-0-spec {ğ“¤} {ğ“¥} Î± = eqtoidâ‚’ (ua (ğ“¤ âŠ” ğ“¥)) fe' ([ğŸ™+ Î± ]^ ğŸ˜â‚’) ğŸ™â‚’ (exp-0-spec' Î±)

{- We should the more general statement that

     ([ğŸ™+ Î± ]^ (Î² +â‚’ Î³)) â‰ƒâ‚’ (([ğŸ™+ Î± ]^ Î²) Ã—â‚’ ([ğŸ™+ Î±]^ Î³)

   and

     ([ğŸ™+ Î±]^ ğŸ™â‚’) ï¼ ğŸ™â‚’ +â‚’ Î±
-}

exp-succ-spec' : (Î± : Ordinal ğ“¤) (Î² : Ordinal ğ“¥)
               â†’ ([ğŸ™+ Î± ]^ (Î² +â‚’ ğŸ™â‚’)) â‰ƒâ‚’ (([ğŸ™+ Î± ]^ Î²) Ã—â‚’ (ğŸ™â‚’ +â‚’ Î±))
exp-succ-spec' Î± Î² = f , f-monotone , qinvs-are-equivs f f-qinv , g-monotone
 where
  f : âŸ¨ [ğŸ™+ Î± ]^ (Î² +â‚’ ğŸ™â‚’) âŸ© â†’ âŸ¨ ([ğŸ™+ Î± ]^ Î²) Ã—â‚’ (ğŸ™â‚’ +â‚’ Î±) âŸ©
  f ([] , Î´) = (([] , Î´) , inl â‹†)
  f ((inl b , a âˆ· xs) , Î´) = (((b , a) âˆ· xs') , Î´') , (inl â‹†)
   where
    xs' : {!!}
    xs' = {!!}
    Î´' : {!!}
    Î´' = {!!}
  f ((inr â‹† , a âˆ· xs) , Î´) = (xs' , Î´') , inr a
   where
    xs' : {!!}
    xs' = {!!}
    Î´' : {!!}
    Î´' = {!!}
  f-monotone : is-order-preserving ([ğŸ™+ Î± ]^ (Î² +â‚’ ğŸ™â‚’)) (([ğŸ™+ Î± ]^ Î²) Ã—â‚’ (ğŸ™â‚’ +â‚’ Î±)) f
  f-monotone = {!!}
  g : âŸ¨ ([ğŸ™+ Î± ]^ Î²) Ã—â‚’ (ğŸ™â‚’ +â‚’ Î±) âŸ© â†’ âŸ¨ [ğŸ™+ Î± ]^ (Î² +â‚’ ğŸ™â‚’) âŸ©
  g (([] , Î´) , inl â‹†) = [] , []-decr
  g ((((b , a) âˆ· xs) , Î´) , inl â‹†) = (inl b , a âˆ· xs') , Î´'
   where
    xs' : {!!}
    xs' = {!!}
    Î´' : {!!}
    Î´' = {!!}
  g (l , inr a) = ((inr â‹†) , a âˆ· xs') , Î´'
   where
    xs' : {!!}
    xs' = {!!}
    Î´' : {!!}
    Î´' = {!!}
  g-monotone : is-order-preserving (([ğŸ™+ Î± ]^ Î²) Ã—â‚’ (ğŸ™â‚’ +â‚’ Î±)) ([ğŸ™+ Î± ]^ (Î² +â‚’ ğŸ™â‚’)) g
  g-monotone = {!!}
  f-qinv : qinv f
  f-qinv = g , p , q
   where
    p : {!!}
    p = {!!}
    q : {!!}
    q = {!!}

exp-succ-spec : (Î± : Ordinal ğ“¤) (Î² : Ordinal ğ“¥)
              â†’ ([ğŸ™+ Î± ]^ (Î² +â‚’ ğŸ™â‚’)) ï¼ (([ğŸ™+ Î± ]^ Î²) Ã—â‚’ (ğŸ™â‚’ +â‚’ Î±))
exp-succ-spec = {!!}
