Tom de Jong, Nicolai Kraus, Fredrik Nordvall Forsberg, Chuangjie Xu,
23 April 2023.

\begin{code}

{-# OPTIONS --safe --without-K --no-exact-split --lossy-unification #-}

open import UF.Univalence
open import UF.PropTrunc
open import UF.Size

module Ordinals.ExponentiationAlternative
       (ua : Univalence)
       (pt : propositional-truncations-exist)
       (sr : Set-Replacement pt)
       where

open import UF.Base
open import UF.Equiv
open import UF.ExcludedMiddle
open import UF.FunExt
open import UF.Sets
open import UF.Subsingletons
open import UF.Subsingletons-FunExt
open import UF.UA-FunExt
open import UF.ImageAndSurjection pt

private
 fe : FunExt
 fe = Univalence-gives-FunExt ua

 fe' : Fun-Ext
 fe' {ğ“¤} {ğ“¥} = fe ğ“¤ ğ“¥

 pe : PropExt
 pe = Univalence-gives-PropExt ua


open import Naturals.Order

open import MLTT.Plus-Properties
open import MLTT.Spartan
open import MLTT.Sigma
open import MLTT.List

open import Ordinals.Arithmetic fe
open import Ordinals.ArithmeticProperties ua
open import Ordinals.Equivalence
open import Ordinals.Maps
open import Ordinals.Notions
open import Ordinals.OrdinalOfOrdinals ua
open import Ordinals.Type
open import Ordinals.Underlying
open import Ordinals.WellOrderingTaboo
open import Ordinals.OrdinalOfOrdinalsSuprema ua

open import Ordinals.Exponentiation ua pt sr

open PropositionalTruncation pt

open suprema pt sr
\end{code}


We define `exp Î± Î² = sup_{1 + âŸ¨ Î² âŸ©} (inl _ â†¦ ğŸ™â‚’; inr b â†¦ exp Î± (Î² â†“ b) Ã—â‚’ Î±)
by transfinite recursion on Î².

\begin{code}

exp : (Î± : Ordinal ğ“¤) â†’ (Î² : Ordinal ğ“¥) â†’ Ordinal (ğ“¤ âŠ” ğ“¥)
exp {ğ“¤} {ğ“¥} Î± = transfinite-recursion-on-OO
                  (Ordinal (ğ“¤ âŠ” ğ“¥))
                  (Î» Î² ih â†’ sup {I = ğŸ™ {ğ“¤} + âŸ¨ Î² âŸ©}
                                  (cases
                                    (Î» _ â†’ ğŸ™â‚’)
                                    (Î» b â†’ ih b Ã—â‚’ Î±))) -- exp Î± (Î² â†“ b) Ã—â‚’ Î±

exp-behaviour : (Î± : Ordinal ğ“¤) â†’ (Î² : Ordinal ğ“¥) â†’
                exp Î± Î² ï¼ sup {I = ğŸ™ {ğ“¤} + âŸ¨ Î² âŸ©} (cases (Î» _ â†’ ğŸ™â‚’) (Î» b â†’ exp Î± (Î² â†“ b) Ã—â‚’ Î±))
exp-behaviour {ğ“¤} {ğ“¥} Î± Î² = {!transfinite-recursion-on-OO-behaviour (Ordinal (ğ“¤ âŠ” ğ“¥)) ((Î» Î² ih â†’ sup {I = ğŸ™ {ğ“¤} + âŸ¨ Î² âŸ©} (cases (Î» _ â†’ ğŸ™â‚’) (Î» b â†’ ih b Ã—â‚’ Î±)))exp-body Î±) Î²!}

\end{code}

\begin{code}

sup-composition : {B : ğ“¤ Ì‡ }{C : ğ“¤ Ì‡ } â†’ (f : B â†’ C) â†’ (F : C â†’ Ordinal ğ“¤) â†’ sup (F âˆ˜ f) âŠ´ sup F
sup-composition f F = sup-is-lower-bound-of-upper-bounds (F âˆ˜ f) (sup F) (Î» i â†’ sup-is-upper-bound F (f i))

exp-monotone-in-exponent : (Î± : Ordinal ğ“¤) â†’ (Î² Î³ : Ordinal ğ“¥)
                         â†’ Î² âŠ´ Î³ â†’ exp Î± Î² âŠ´ exp Î± Î³
exp-monotone-in-exponent Î± Î² Î³ p = transportâ‚‚â»Â¹ _âŠ´_ (exp-behaviour Î± Î²) (exp-behaviour Î± Î³) (transport (Î» - â†’ sup -  âŠ´ sup F) claim' (sup-composition f F))
  where
    F : ğŸ™ {ğ“¤} + âŸ¨ Î³ âŸ© â†’ Ordinal _
    F  = cases (Î» _ â†’ ğŸ™â‚’) (Î» c â†’ exp Î± (Î³ â†“ c) Ã—â‚’ Î±)

    f : ğŸ™ {ğ“¤} + âŸ¨ Î² âŸ© â†’ ğŸ™ {ğ“¤} + âŸ¨ Î³ âŸ©
    f (inl x) = inl x
    f (inr b) = inr (prâ‚ p b)

    F' : ğŸ™ {ğ“¤} + âŸ¨ Î² âŸ© â†’ Ordinal _
    F' = cases (Î» _ â†’ ğŸ™â‚’) (Î» b â†’ exp Î± (Î² â†“ b) Ã—â‚’ Î±)

    initial-segments-agree : (b : âŸ¨ Î² âŸ©) â†’ Î² â†“ b ï¼ Î³ â†“ (prâ‚ p b)
    initial-segments-agree b = prâ‚‚ (from-â‰¼ (âŠ´-gives-â‰¼ Î² Î³ p) b)

    claim : (i : ğŸ™ {ğ“¤} + âŸ¨ Î² âŸ©) â†’ F (f i) ï¼ F' i
    claim (inl x) = refl
    claim (inr b) = ap (Î» - â†’ exp Î± - Ã—â‚’ Î±) (initial-segments-agree b â»Â¹)

    claim' : F âˆ˜ f ï¼ F'
    claim' = dfunext fe' claim

exp-has-least-element : (Î± : Ordinal ğ“¤) â†’ (Î² : Ordinal ğ“¥) â†’ ğŸ™â‚’ {ğ“¤ âŠ” ğ“¥} âŠ´ exp Î± Î²
exp-has-least-element {ğ“¤} Î± Î² = transportâ»Â¹ (ğŸ™â‚’ âŠ´_) (exp-behaviour Î± Î²) q
  where
    q : ğŸ™â‚’ âŠ´ sup (cases (Î» _ â†’ ğŸ™â‚’) (Î» b â†’ exp Î± (Î² â†“ b) Ã—â‚’ Î±))
    q = sup-is-upper-bound (cases (Î» _ â†’ ğŸ™â‚’) (Î» b â†’ exp Î± (Î² â†“ b) Ã—â‚’ Î±)) (inl â‹†)

exp-satisfies-zero-specification : (Î± : Ordinal ğ“¤) â†’ exp Î± (ğŸ˜â‚’ {ğ“¥}) ï¼ ğŸ™â‚’
exp-satisfies-zero-specification Î± = âŠ´-antisym (exp Î± ğŸ˜â‚’) ğŸ™â‚’ II III
  where
    I : (i : ğŸ™ + ğŸ˜) â†’ cases (Î» _ â†’ ğŸ™â‚’) (Î» b â†’ exp Î± (ğŸ˜â‚’ â†“ b) Ã—â‚’ Î±) i âŠ´ ğŸ™â‚’
    I (inl _) = âŠ´-refl ğŸ™â‚’

    II : exp Î± ğŸ˜â‚’ âŠ´ ğŸ™â‚’
    II = transportâ»Â¹ (_âŠ´ ğŸ™â‚’) (exp-behaviour Î± ğŸ˜â‚’) (sup-is-lower-bound-of-upper-bounds (cases (Î» _ â†’ ğŸ™â‚’) (Î» b â†’ exp Î± (ğŸ˜â‚’ â†“ b) Ã—â‚’ Î±)) ğŸ™â‚’ I)

    III : ğŸ™â‚’ âŠ´ exp Î± ğŸ˜â‚’
    III = exp-has-least-element Î± ğŸ˜â‚’

exp-power-one-is-identity : (Î± : Ordinal ğ“¤) â†’ ğŸ™â‚’ {ğ“¤} âŠ´ Î± â†’ exp Î± (ğŸ™â‚’ {ğ“¤}) ï¼ Î±
exp-power-one-is-identity Î± p = transportâ»Â¹ (Î» - â†’ - ï¼ Î±) (exp-behaviour Î± ğŸ™â‚’)
                                            (âŠ´-antisym _ _ f g)
 where
  I : (ğŸ™â‚’ â†“ â‹†) âŠ´ ğŸ˜â‚’
  I = (Î» x â†’ ğŸ˜-elim (prâ‚‚ x)) , (Î» x â†’ ğŸ˜-elim (prâ‚‚ x)) , (Î» x â†’ ğŸ˜-elim (prâ‚‚ x))

  II : (ğŸ™â‚’ â†“ â‹†) ï¼ ğŸ˜â‚’
  II = âŠ´-antisym _ _ I (ğŸ˜â‚’-least-âŠ´ (ğŸ™â‚’ â†“ â‹†))

  III : exp Î± (ğŸ™â‚’ â†“ â‹†) ï¼ ğŸ™â‚’
  III = transportâ»Â¹ (Î» - â†’ exp Î± - ï¼ ğŸ™â‚’) II (exp-satisfies-zero-specification Î±)

  IV : exp Î± (ğŸ™â‚’ â†“ â‹†) Ã—â‚’ Î± ï¼ Î±
  IV = (ap (_Ã—â‚’ Î±) III âˆ™ ğŸ™â‚’-left-neutral-Ã—â‚’ Î±)

  f : sup (cases (Î» _ â†’ ğŸ™â‚’) (Î» b â†’ exp Î± (ğŸ™â‚’ â†“ b) Ã—â‚’ Î±)) âŠ´ Î±
  f = (sup-is-lower-bound-of-upper-bounds (cases (Î» _ â†’ ğŸ™â‚’) (Î» b â†’ exp Î± (ğŸ™â‚’ â†“ b) Ã—â‚’ Î±)) Î± k)
    where
     k : (i : ğŸ™ + ğŸ™) â†’ cases (Î» _ â†’ ğŸ™â‚’) (Î» b â†’ exp Î± (ğŸ™â‚’ â†“ b) Ã—â‚’ Î±) i âŠ´ Î±
     k (inl _) = p
     k (inr b) = transportâ»Â¹ (_âŠ´ Î±) IV (âŠ´-refl Î±)

  g : Î± âŠ´ sup (cases (Î» _ â†’ ğŸ™â‚’) (Î» b â†’ exp Î± (ğŸ™â‚’ â†“ b) Ã—â‚’ Î±))
  g = transport (_âŠ´ sup (cases (Î» _ â†’ ğŸ™â‚’) (Î» b â†’ exp Î± (ğŸ™â‚’ â†“ b) Ã—â‚’ Î±)))
                IV
                (sup-is-upper-bound (cases (Î» _ â†’ ğŸ™â‚’) (Î» b â†’ exp Î± (ğŸ™â‚’ â†“ b) Ã—â‚’ Î±)) (inr â‹†))


exp-power-two : (Î± : Ordinal ğ“¤) â†’ ğŸ™â‚’ {ğ“¤} âŠ´ Î± â†’ exp Î± (ğŸ™â‚’ +â‚’ ğŸ™â‚’ {ğ“¤}) ï¼ Î± Ã—â‚’ Î±
exp-power-two {ğ“¤} Î± p = transportâ»Â¹ (Î» - â†’ - ï¼ Î± Ã—â‚’ Î±) (exp-behaviour Î± (ğŸ™â‚’ +â‚’ ğŸ™â‚’) âˆ™ ap sup eq')
                                (âŠ´-antisym _ _ (sup-is-lower-bound-of-upper-bounds F (Î± Ã—â‚’ Î±) F-upper-bound) (sup-is-upper-bound F (inr (inr â‹†))))
  where
   F : ğŸ™ + (ğŸ™ + ğŸ™) â†’ Ordinal ğ“¤
   F (inl _) = ğŸ™â‚’
   F (inr (inl _)) = Î±
   F (inr (inr _)) = Î± Ã—â‚’ Î±

   pâ‚‚ : Î± âŠ´ (Î± Ã—â‚’ Î±)
   pâ‚‚ = transport (_âŠ´ (Î± Ã—â‚’ Î±)) (ğŸ™â‚’-right-neutral-Ã—â‚’ Î±) (Ã—â‚’-right-monotone-âŠ´ Î± ğŸ™â‚’ Î± p)

   F-upper-bound : (i : ğŸ™ + (ğŸ™ + ğŸ™)) â†’  F i âŠ´ (Î± Ã—â‚’ Î±)
   F-upper-bound (inl _) = âŠ´-trans _ _ _ p pâ‚‚
   F-upper-bound (inr (inl _)) = pâ‚‚
   F-upper-bound (inr (inr _)) = âŠ´-refl (Î± Ã—â‚’ Î±)

   eq : (i : ğŸ™ + (ğŸ™ + ğŸ™)) â†’ (cases (Î» _ â†’ ğŸ™â‚’) (Î» b â†’ exp Î± ((ğŸ™â‚’ +â‚’ ğŸ™â‚’) â†“ b) Ã—â‚’ Î±)) i ï¼ F i
   eq (inl _) = refl
   eq (inr (inl x)) = IV
    where
      I : ((ğŸ™â‚’ +â‚’ ğŸ™â‚’) â†“ inl â‹†) âŠ´ ğŸ˜â‚’
      I = (Î» { (inl x , p) â†’ p ; (inr x , p) â†’ p}) , (Î» x y â†’ ğŸ˜-elim y) , Î» { (inl x , p) â†’ ğŸ˜-elim p ; (inr x , p) â†’ ğŸ˜-elim p }

      II : ((ğŸ™â‚’ +â‚’ ğŸ™â‚’) â†“ inl â‹†) ï¼ ğŸ˜â‚’
      II = âŠ´-antisym _ _ I (ğŸ˜â‚’-least-âŠ´ ((ğŸ™â‚’ +â‚’ ğŸ™â‚’) â†“ inl â‹†))

      III : exp Î± ((ğŸ™â‚’ +â‚’ ğŸ™â‚’) â†“ inl â‹†) ï¼ ğŸ™â‚’
      III = transportâ»Â¹ (Î» - â†’ exp Î± - ï¼ ğŸ™â‚’) II (exp-satisfies-zero-specification Î±)

      IV : exp Î± ((ğŸ™â‚’ +â‚’ ğŸ™â‚’) â†“ inl â‹†) Ã—â‚’ Î± ï¼ Î±
      IV = (ap (_Ã—â‚’ Î±) III âˆ™ ğŸ™â‚’-left-neutral-Ã—â‚’ Î±)
   eq (inr (inr x)) = III
     where
      I : ((ğŸ™â‚’ +â‚’ ğŸ™â‚’) â†“ inr â‹†) ï¼ ğŸ™â‚’
      I = +â‚’-ğŸ™â‚’-â†“-right ğŸ™â‚’

      II : exp Î± ((ğŸ™â‚’ +â‚’ ğŸ™â‚’) â†“ inr â‹†) ï¼ Î±
      II = ap (exp Î±) I âˆ™ exp-power-one-is-identity Î± p

      III : exp Î± ((ğŸ™â‚’ +â‚’ ğŸ™â‚’) â†“ inr â‹†) Ã—â‚’ Î± ï¼ Î± Ã—â‚’ Î±
      III = ap (_Ã—â‚’ Î±) II

   eq' : (cases (Î» _ â†’ ğŸ™â‚’) (Î» b â†’ exp Î± ((ğŸ™â‚’ +â‚’ ğŸ™â‚’) â†“ b) Ã—â‚’ Î±)) ï¼ F
   eq' = dfunext fe' eq

finite-ord : â„• â†’ Ordinal ğ“¤
finite-ord zero = ğŸ˜â‚’
finite-ord (succ n) = finite-ord n +â‚’ ğŸ™â‚’

finite-ordâ»Â¹ : {n : â„•} â†’ âŸ¨ finite-ord {ğ“¤ = ğ“¤} n âŸ© â†’ â„•
finite-ordâ»Â¹ {n = succ n} (inl x) = finite-ordâ»Â¹ {n = n} x
finite-ordâ»Â¹ {n = succ n} (inr x) = n

finite-ordâ»Â¹-bound : {n : â„•} â†’ (k : âŸ¨ finite-ord {ğ“¤ = ğ“¤} n âŸ©) â†’ finite-ordâ»Â¹ k <â„• n
finite-ordâ»Â¹-bound {n = succ n} (inl k) = â‰¤-trans (finite-ordâ»Â¹ k) (succ (finite-ordâ»Â¹ k)) n (â‰¤-succ (finite-ordâ»Â¹ k)) (finite-ordâ»Â¹-bound {n = n} k)
finite-ordâ»Â¹-bound {n = succ n} (inr _) = <-succ n

finite-ord-â†“ : {n : â„•} â†’ (k : âŸ¨ finite-ord {ğ“¤} n âŸ©) â†’  finite-ord n â†“ k ï¼ finite-ord (finite-ordâ»Â¹ k)
finite-ord-â†“ {n = succ n} (inl k) = +â‚’-â†“-left k â»Â¹ âˆ™ finite-ord-â†“ {n = n} k
finite-ord-â†“ {n = succ n} (inr x) = +â‚’-ğŸ™â‚’-â†“-right (finite-ord n)

finite-exp : Ordinal ğ“¤ â†’ â„• â†’ Ordinal ğ“¤
finite-exp Î± zero = ğŸ™â‚’
finite-exp Î± (succ n) = finite-exp Î± n Ã—â‚’ Î±

finite-exp-swap : (Î± : Ordinal ğ“¤) â†’ (n : â„•) â†’ finite-exp Î± (succ n) ï¼ Î± Ã—â‚’ finite-exp Î± n
finite-exp-swap Î± zero = (ğŸ™â‚’ Ã—â‚’ Î±) ï¼âŸ¨ ğŸ™â‚’-left-neutral-Ã—â‚’ Î± âŸ© Î± ï¼âŸ¨ ğŸ™â‚’-right-neutral-Ã—â‚’ Î± â»Â¹ âŸ© (Î± Ã—â‚’ ğŸ™â‚’) âˆ
finite-exp-swap Î± (succ n) =
  ((finite-exp Î± n Ã—â‚’ Î±) Ã—â‚’ Î±) ï¼âŸ¨ ap (_Ã—â‚’ Î±) (finite-exp-swap Î± n) âŸ©
  ((Î± Ã—â‚’ finite-exp Î± n) Ã—â‚’ Î±) ï¼âŸ¨ Ã—â‚’-assoc Î± (finite-exp Î± n) Î± âŸ©
  ( Î± Ã—â‚’ (finite-exp Î± n Ã—â‚’ Î±)) âˆ

finite-exp-least-element : (Î± : Ordinal ğ“¤) â†’ ğŸ™â‚’ {ğ“¤} âŠ´ Î± â†’ (n : â„•) â†’ ğŸ™â‚’ {ğ“¤} âŠ´ finite-exp Î± n
finite-exp-least-element Î± p zero = âŠ´-refl ğŸ™â‚’
finite-exp-least-element Î± p (succ n) = âŠ´-trans _ _ _ p
                                                      (transportâ‚‚ _âŠ´_
                                                                  (ğŸ™â‚’-right-neutral-Ã—â‚’ Î±)
                                                                  (finite-exp-swap Î± n â»Â¹)
                                                                  (Ã—â‚’-right-monotone-âŠ´ Î± _ _ (finite-exp-least-element Î± p n)))


finite-exp-monotone : (Î± : Ordinal ğ“¤) â†’ ğŸ™â‚’ {ğ“¤} âŠ´ Î± â†’ (n : â„•) â†’ (k : âŸ¨ finite-ord {ğ“¤ = ğ“¤} n âŸ©) â†’ finite-exp Î± (finite-ordâ»Â¹ k) âŠ´ finite-exp Î± n
finite-exp-monotone Î± p (succ n) (inl x) = âŠ´-trans _ _ _ (finite-exp-monotone Î± p n x) (transport (_âŠ´ (finite-exp Î± n Ã—â‚’ Î±)) (ğŸ™â‚’-right-neutral-Ã—â‚’ _) (Ã—â‚’-right-monotone-âŠ´ (finite-exp Î± n) _ _ p))
finite-exp-monotone Î± p (succ n) (inr x) = transport (_âŠ´ (finite-exp Î± n Ã—â‚’ Î±)) (ğŸ™â‚’-right-neutral-Ã—â‚’ _) (Ã—â‚’-right-monotone-âŠ´ (finite-exp Î± n) _ _ p)

finite-exp-finite-ordâ»Â¹-swap : (Î± : Ordinal ğ“¤) â†’ (n : â„•) â†’ (k : âŸ¨ finite-ord {ğ“¤ = ğ“¤} n âŸ©) â†’ finite-exp Î± (finite-ordâ»Â¹ {n = n} k) Ã—â‚’ Î± ï¼ (Î± Ã—â‚’ finite-exp Î± (finite-ordâ»Â¹ {n = n} k))
finite-exp-finite-ordâ»Â¹-swap Î± (succ n) (inl x) = finite-exp-finite-ordâ»Â¹-swap Î± n x
finite-exp-finite-ordâ»Â¹-swap Î± (succ n) (inr x) = finite-exp-swap Î± n


exp-satisfies-succ-specification-for-finite-powers : (Î± : Ordinal ğ“¤) â†’ ğŸ™â‚’ {ğ“¤} âŠ´ Î±
                                                   â†’ (n : â„•) â†’ exp Î± (finite-ord {ğ“¤} n) ï¼ finite-exp Î± n
exp-satisfies-succ-specification-for-finite-powers {ğ“¤} Î± p = course-of-values-induction (Î» n â†’ exp Î± (finite-ord {ğ“¤} n) ï¼ finite-exp Î± n) step
 where
  step : (n : â„•) â†’ (((m : â„•) â†’ m <â„• n â†’ exp Î± (finite-ord {ğ“¤} m) ï¼ finite-exp Î± m)) â†’ exp Î± (finite-ord {ğ“¤} n) ï¼ finite-exp Î± n
  step zero ih = exp-satisfies-zero-specification Î±
  step (succ n) ih = transportâ»Â¹ (Î» - â†’ - ï¼ finite-exp Î± n Ã—â‚’ Î±) (exp-behaviour Î± (finite-ord n +â‚’ ğŸ™â‚’) âˆ™ ap sup eq')
                                 (âŠ´-antisym _ _ (sup-is-lower-bound-of-upper-bounds F _ upper-bound) (sup-is-upper-bound F (inr (inr â‹†))))
   where
    F : ğŸ™ + (âŸ¨ finite-ord n âŸ© + ğŸ™) â†’ Ordinal ğ“¤
    F (inl _) = ğŸ™â‚’
    F (inr (inl k)) = finite-exp Î± (finite-ordâ»Â¹ k) Ã—â‚’ Î±
    F (inr (inr _)) = finite-exp Î± n Ã—â‚’ Î±

    upper-bound : (i : ğŸ™ + (âŸ¨ finite-ord n âŸ© + ğŸ™)) â†’ F i âŠ´ (finite-exp Î± n Ã—â‚’ Î±)
    upper-bound (inl _) = finite-exp-least-element {ğ“¤} Î± p (succ n)
    upper-bound (inr (inl k)) = transportâ‚‚â»Â¹ _âŠ´_ (finite-exp-finite-ordâ»Â¹-swap Î± n k)
                                                 (finite-exp-swap Î± n)
                                                 (Ã—â‚’-right-monotone-âŠ´ Î± _ _ (finite-exp-monotone Î± p n k))
    upper-bound (inr (inr _)) = âŠ´-refl (finite-exp Î± n Ã—â‚’ Î±)

    eq : (i : ğŸ™ + (âŸ¨ finite-ord n âŸ© + ğŸ™)) â†’ (cases (Î» _ â†’ ğŸ™â‚’) (Î» b â†’ exp Î± ((finite-ord n +â‚’ ğŸ™â‚’) â†“ b) Ã—â‚’ Î±)) i ï¼ F i
    eq (inl _) = refl
    eq (inr (inl k)) = ap (_Ã—â‚’ Î±) III
     where
      I : (finite-ord n +â‚’ ğŸ™â‚’) â†“ inl k ï¼ finite-ord (finite-ordâ»Â¹ k)
      I = +â‚’-â†“-left k â»Â¹ âˆ™ finite-ord-â†“ k

      III : exp Î± ((finite-ord n +â‚’ ğŸ™â‚’) â†“ inl k) ï¼ finite-exp Î± (finite-ordâ»Â¹ k)
      III = ap (exp Î±) I âˆ™ ih (finite-ordâ»Â¹ k) (finite-ordâ»Â¹-bound {n = succ n} (inl k))
    eq (inr (inr _)) = ap (Î» z â†’ exp Î± z Ã—â‚’ Î±) (+â‚’-ğŸ™â‚’-â†“-right (finite-ord n)) âˆ™ ap (_Ã—â‚’ Î±) (ih n (<-succ n))

    eq' : (cases (Î» _ â†’ ğŸ™â‚’) (Î» b â†’ exp Î± ((finite-ord n +â‚’ ğŸ™â‚’) â†“ b) Ã—â‚’ Î±)) ï¼ F
    eq' = dfunext fe' eq



{-

   F-upper-bound : (i : ğŸ™ + (ğŸ™ + ğŸ™)) â†’  F i âŠ´ (Î± Ã—â‚’ Î±)
   F-upper-bound (inl _) = âŠ´-trans _ _ _ p pâ‚‚
   F-upper-bound (inr (inl _)) = pâ‚‚
   F-upper-bound (inr (inr _)) = âŠ´-refl (Î± Ã—â‚’ Î±)

   eq : (i : ğŸ™ + (ğŸ™ + ğŸ™)) â†’ (cases (Î» _ â†’ ğŸ™â‚’) (Î» b â†’ exp Î± ((ğŸ™â‚’ +â‚’ ğŸ™â‚’) â†“ b) Ã—â‚’ Î±)) i ï¼ F i
   eq (inl _) = refl
   eq (inr (inl x)) = IV
    where
      I : ((ğŸ™â‚’ +â‚’ ğŸ™â‚’) â†“ inl â‹†) âŠ´ ğŸ˜â‚’
      I = (Î» { (inl x , p) â†’ p ; (inr x , p) â†’ p}) , (Î» x y â†’ ğŸ˜-elim y) , Î» { (inl x , p) â†’ ğŸ˜-elim p ; (inr x , p) â†’ ğŸ˜-elim p }

      II : ((ğŸ™â‚’ +â‚’ ğŸ™â‚’) â†“ inl â‹†) ï¼ ğŸ˜â‚’
      II = âŠ´-antisym _ _ I (ğŸ˜â‚’-least-âŠ´ ((ğŸ™â‚’ +â‚’ ğŸ™â‚’) â†“ inl â‹†))

      III : exp Î± ((ğŸ™â‚’ +â‚’ ğŸ™â‚’) â†“ inl â‹†) ï¼ ğŸ™â‚’
      III = transportâ»Â¹ (Î» - â†’ exp Î± - ï¼ ğŸ™â‚’) II (exp-satisfies-zero-specification Î±)

      IV : exp Î± ((ğŸ™â‚’ +â‚’ ğŸ™â‚’) â†“ inl â‹†) Ã—â‚’ Î± ï¼ Î±
      IV = (ap (_Ã—â‚’ Î±) III âˆ™ ğŸ™â‚’-left-neutral-Ã—â‚’ Î±)
   eq (inr (inr x)) = III
     where
      I : ((ğŸ™â‚’ +â‚’ ğŸ™â‚’) â†“ inr â‹†) ï¼ ğŸ™â‚’
      I = +â‚’-ğŸ™â‚’-â†“-right ğŸ™â‚’

      II : exp Î± ((ğŸ™â‚’ +â‚’ ğŸ™â‚’) â†“ inr â‹†) ï¼ Î±
      II = ap (exp Î±) I âˆ™ exp-power-one-is-identity Î± p

      III : exp Î± ((ğŸ™â‚’ +â‚’ ğŸ™â‚’) â†“ inr â‹†) Ã—â‚’ Î± ï¼ Î± Ã—â‚’ Î±
      III = ap (_Ã—â‚’ Î±) II

   eq' : (cases (Î» _ â†’ ğŸ™â‚’) (Î» b â†’ exp Î± ((ğŸ™â‚’ +â‚’ ğŸ™â‚’) â†“ b) Ã—â‚’ Î±)) ï¼ F
   eq' = dfunext fe' eq
-}
{-
exp-satisfies-succ-specification : (Î± Î² : Ordinal ğ“¤) â†’ ğŸ™â‚’ {ğ“¤} âŠ´ Î±
                                 â†’ exp Î± (Î² +â‚’ ğŸ™â‚’) ï¼ (exp Î± Î²) Ã—â‚’ Î±
exp-satisfies-succ-specification Î± Î² p = transportâ»Â¹ (Î» - â†’ - ï¼ (exp Î± Î²) Ã—â‚’ Î±) (exp-behaviour Î± (Î² +â‚’ ğŸ™â‚’))
                                           (surjective-simulation-gives-equality _ (exp Î± Î² Ã—â‚’ Î±) f f-is-simulation f-is-surjective)
 where
  h : sup (cases (Î» _ â†’ ğŸ™â‚’) (Î» b â†’ exp Î± ((Î² +â‚’ ğŸ™â‚’) â†“ b) Ã—â‚’ Î±)) âŠ´ ((exp Î± Î²) Ã—â‚’ Î±)
  h = (sup-is-lower-bound-of-upper-bounds (cases (Î» _ â†’ ğŸ™â‚’) (Î» b â†’ exp Î± ((Î² +â‚’ ğŸ™â‚’) â†“ b) Ã—â‚’ Î±)) ((exp Î± Î²) Ã—â‚’ Î±) k)
    where
      k : (i : ğŸ™ + prâ‚ (Î² +â‚’ ğŸ™â‚’)) â†’ cases (Î» _ â†’ ğŸ™â‚’) (Î» b â†’ exp Î± ((Î² +â‚’ ğŸ™â‚’) â†“ b) Ã—â‚’ Î±) i âŠ´ (exp Î± Î² Ã—â‚’ Î±)
      k (inl _) = {!!}
      k (inr (inl b)) = {!!}
      k (inr (inr _)) = {!!}

  f : âŸ¨ sup (cases (Î» _ â†’ ğŸ™â‚’) (Î» b â†’ exp Î± ((Î² +â‚’ ğŸ™â‚’) â†“ b) Ã—â‚’ Î±)) âŸ© â†’  âŸ¨ (exp Î± Î²) Ã—â‚’ Î± âŸ©
  f = prâ‚ h

  f-is-simulation : is-simulation _ (exp Î± Î² Ã—â‚’ Î±) f
  f-is-simulation = prâ‚‚ h

  f-is-surjective : is-surjection f
  f-is-surjective = {!!}
-}
{-



(f : Î± â‰¤ Î±') â†’? Î± Ã—â‚’ Î² â‰¤ Î±' Ã—â‚’ Î²

(a , b) â†¦ (f a , b)

Assume (a' , b') < (f a  , b). Need to find (aâ‚€ , bâ‚€) s t (f aâ‚€ , bâ‚€) = (a' , b').



Case b' < b: Take aâ‚€ = ???, bâ‚€ = b'.

Case b' = b, a' < f a


-}

\end{code}
