Andrew Sneap - 27 April 2023

\begin{code}

{-# OPTIONS --without-K --exact-split --safe --no-sized-types --no-guardedness --lossy-unification --auto-inline #-}

open import MLTT.Spartan renaming (_+_ to _âˆ”_)
open import Notation.CanonicalMap
open import Notation.Order
open import Rationals.Abs
open import Rationals.Addition
open import Rationals.Negation
open import Rationals.Order
open import Rationals.Type
open import UF.Base
open import UF.FunExt
open import UF.PropTrunc
open import UF.Subsingletons

module DedekindReals.Functions
  (fe : Fun-Ext)
  (pe : Prop-Ext)
  (pt : propositional-truncations-exist)
 where

open PropositionalTruncation pt

open import DedekindReals.Properties fe pt pe
open import DedekindReals.Type pe pt fe
open import DedekindReals.Extension fe pe pt

\end{code}

To illustrate the use of the extension theorem, the following examples is
provided which lifts the increment function on rationals to a function on reals.

The function which increments by one is clearly uniformly continuous (and this
is proved below). Hence we simply apply the extension thereom and we are done.

\begin{code}

â„š-incr : â„š â†’ â„š
â„š-incr q = q + 1â„š

â„š-incr-uc : â„š-is-uniformly-continuous â„š-incr
â„š-incr-uc (Îµ , 0<Îµ) = (Îµ , 0<Îµ) , Î³
 where
  Î³ : (x xâ‚€ : â„š) â†’ x âˆˆð (Îµ , 0<Îµ) â¦… xâ‚€ â¦† â†’ â„š-incr x âˆˆð (Îµ , 0<Îµ) â¦… â„š-incr xâ‚€ â¦†
  Î³ x xâ‚€ (lâ‚ , lâ‚‚) = Î³â‚ , Î³â‚‚
   where
    I : x + 1â„š < xâ‚€ + Îµ + 1â„š
    I = â„š<-addition-preserves-order x (xâ‚€ + Îµ) 1â„š lâ‚‚

    II : xâ‚€ - Îµ + 1â„š < x + 1â„š
    II = â„š<-addition-preserves-order (xâ‚€ - Îµ) x 1â„š lâ‚

    Î³â‚ : xâ‚€ + 1â„š - Îµ < x + 1â„š
    Î³â‚ = transport (_< x + 1â„š) (â„š+-rearrange xâ‚€ (- Îµ) 1â„š) II

    Î³â‚‚ : x + 1â„š < xâ‚€ + 1â„š + Îµ
    Î³â‚‚ = transport (x + 1â„š <_) (â„š+-rearrange xâ‚€ Îµ 1â„š) I

â„-incr : â„ â†’ â„
â„-incr = extend â„š-incr â„š-incr-uc

â„-incr-agrees-with-â„š-incr : (q : â„š) â†’ â„-incr (Î¹ q) ï¼ Î¹ (â„š-incr q)
â„-incr-agrees-with-â„š-incr q = extend-is-extension q â„š-incr â„š-incr-uc

â„-incr-is-uc : â„-is-uniformly-continuous â„-incr
â„-incr-is-uc = extensions-uc â„š-incr â„š-incr-uc

â„š-neg-is-uc : â„š-is-uniformly-continuous (-_)
â„š-neg-is-uc (Îµ , 0<Îµ) = (Îµ , 0<Îµ) , Î³
 where
  Î³ : (x xâ‚€ : â„š) â†’ x âˆˆð Îµ , 0<Îµ â¦… xâ‚€ â¦† â†’ (- x) âˆˆð Îµ , 0<Îµ â¦… - xâ‚€ â¦†
  Î³ x xâ‚€ (lâ‚ , lâ‚‚) = lâ‚ƒ , lâ‚„
   where
    lâ‚ƒ : (- xâ‚€) - Îµ < - x
    lâ‚ƒ = â„š<-swap-right-add x xâ‚€ Îµ lâ‚‚

    lâ‚„ : - x < (- xâ‚€) + Îµ
    lâ‚„ = â„š<-swap-left-neg xâ‚€ Îµ x lâ‚

â„-_ : â„ â†’ â„
â„-_ = extend -_ â„š-neg-is-uc

â„-neg-agrees-with-â„š : (q : â„š) â†’ â„- (Î¹ q) ï¼ Î¹ (- q)
â„-neg-agrees-with-â„š q = extend-is-extension q -_ â„š-neg-is-uc

â„-neg-is-uc : â„-is-uniformly-continuous â„-_
â„-neg-is-uc = extensions-uc -_ â„š-neg-is-uc

abs-uc : â„š-is-uniformly-continuous abs
abs-uc (Îµ , 0<Îµ) = (Îµ , 0<Îµ) , Î³
 where
  Î³ : (x xâ‚€ : â„š) â†’ x âˆˆð Îµ , 0<Îµ â¦… xâ‚€ â¦† â†’ abs x âˆˆð Îµ , 0<Îµ â¦… abs xâ‚€ â¦†
  Î³ x xâ‚€ (lâ‚ , lâ‚‚) = Î³' (â„š-abs-inverse x) (â„š-abs-inverse xâ‚€)
   where
    I : (- xâ‚€) - Îµ < - x
    I = â„š<-swap-right-add x xâ‚€ Îµ lâ‚‚

    II : - x < (- xâ‚€) + Îµ
    II = â„š<-swap-left-neg xâ‚€ Îµ x lâ‚

    Î³' : (abs x ï¼ x) âˆ” (abs x ï¼ - x)
       â†’ (abs xâ‚€ ï¼ xâ‚€) âˆ” (abs xâ‚€ ï¼ - xâ‚€)
       â†’ abs x âˆˆð Îµ , 0<Îµ â¦… abs xâ‚€ â¦†
    Î³' (inl eâ‚) (inl eâ‚‚) = lâ‚ƒ , lâ‚„
     where
      lâ‚ƒ : abs xâ‚€ - Îµ < abs x
      lâ‚ƒ = transportâ‚‚ (Î» a b â†’ a - Îµ < b) (eâ‚‚ â»Â¹) (eâ‚ â»Â¹) lâ‚

      lâ‚„ : abs x < abs xâ‚€ + Îµ
      lâ‚„ = transportâ‚‚ (Î» a b â†’ b < a + Îµ) (eâ‚‚ â»Â¹) (eâ‚ â»Â¹) lâ‚‚

    Î³' (inl eâ‚) (inr eâ‚‚) = lâ‚ƒ , lâ‚„
     where
      III : abs xâ‚€ - Îµ < - abs x
      III = transportâ‚‚ (Î» a b â†’ a - Îµ < - b) (eâ‚‚ â»Â¹) (eâ‚ â»Â¹) I

      lâ‚ƒ : abs xâ‚€ - Îµ < abs x
      lâ‚ƒ = â„š<-â‰¤-trans (abs xâ‚€ - Îµ) (- abs x) (abs x) III (â„šâ‰¤-abs-neg x)

      IV : abs x < xâ‚€ + Îµ
      IV = transport (_< xâ‚€ + Îµ) (eâ‚ â»Â¹) lâ‚‚

      V : xâ‚€ + Îµ â‰¤ abs xâ‚€ + Îµ
      V = â„šâ‰¤-addition-preserves-order xâ‚€ (abs xâ‚€) Îµ (â„šâ‰¤-abs-all xâ‚€)

      lâ‚„ : abs x <â„š abs xâ‚€ + Îµ
      lâ‚„ = â„š<-â‰¤-trans (abs x) (xâ‚€ + Îµ) (abs xâ‚€ + Îµ) IV V

    Î³' (inr eâ‚) (inl eâ‚‚) = lâ‚ƒ , lâ‚„
     where
      III : abs xâ‚€ - Îµ < x
      III = transport (Î» a â†’ a - Îµ < x) (eâ‚‚ â»Â¹) lâ‚

      lâ‚ƒ : abs xâ‚€ - Îµ < abs x
      lâ‚ƒ = â„š<-â‰¤-trans (abs xâ‚€ - Îµ) x (abs x) III (â„šâ‰¤-abs-all x)

      IV : abs x < (- abs xâ‚€) + Îµ
      IV = transportâ‚‚ (Î» a b â†’ b < (- a) + Îµ) (eâ‚‚ â»Â¹) (eâ‚ â»Â¹) II

      V : (- abs xâ‚€) + Îµ â‰¤ abs xâ‚€ + Îµ
      V = â„šâ‰¤-addition-preserves-order (- abs xâ‚€) (abs xâ‚€) Îµ (â„šâ‰¤-abs-neg xâ‚€)

      lâ‚„ : abs x < abs xâ‚€ + Îµ
      lâ‚„ = â„š<-â‰¤-trans (abs x) ((- abs xâ‚€) + Îµ) (abs xâ‚€ + Îµ) IV V

    Î³' (inr eâ‚) (inr eâ‚‚) = lâ‚ƒ , lâ‚„
     where
      lâ‚ƒ : abs xâ‚€ - Îµ < abs x
      lâ‚ƒ = transportâ‚‚ (Î» a b â†’ a - Îµ < b) (eâ‚‚ â»Â¹) (eâ‚ â»Â¹) I

      lâ‚„ : abs x < abs xâ‚€ + Îµ
      lâ‚„ = transportâ‚‚ (Î» a b â†’ b < a + Îµ) (eâ‚‚ â»Â¹) (eâ‚ â»Â¹) II

â„-abs : â„ â†’ â„
â„-abs = extend abs abs-uc

â„-abs-agrees-with-â„š-abs : (q : â„š) â†’ â„-abs (Î¹ q) ï¼ Î¹ (abs q)
â„-abs-agrees-with-â„š-abs q = extend-is-extension q abs abs-uc

â„-abs-uc : â„-is-uniformly-continuous â„-abs
â„-abs-uc = extensions-uc abs abs-uc

\end{code}
