Lane Biocini, 21 January 2026

The equational theory of PSL2Z. Although sÂ² = 1 and rÂ³ = 1 hold
definitionally (by computation), we provide propositional witnesses
for use in equational reasoning chains. The main result is that
PSL2Z has decidable equality, making it a set (h-level 2).

The decidability proof exploits the mutual inductive structure:
S-edge and R-edge each have decidable equality by structural
recursion, and the disjoint sum PSL2Z = S-edge + R-edge inherits
decidability.

\begin{code}

{-# OPTIONS --safe --without-K --exact-split #-}

module Groups.ModularGroup.Properties where

open import MLTT.Spartan
open import MLTT.Two-Properties
open import MLTT.Plus-Properties using (+disjoint; +functor; inl-lc; inr-lc)
open import MLTT.Unit-Properties using (ğŸ™-is-not-ğŸ˜)
open import UF.Base
open import UF.DiscreteAndSeparated using (is-discrete; discrete-types-are-sets)
open import UF.Sets using (is-set)
open import Groups.ModularGroup.Type
open import Groups.ModularGroup.Base

sÂ² : (x : PSL2Z) â†’ s (s x) ï¼ x
sÂ² (Î· eâ‚€)  = refl
sÂ² (Î· eâ‚)  = refl
sÂ² (sâˆ™ re) = refl
sÂ² (Î¸ re)  = refl

rÂ³ : (x : PSL2Z) â†’ r (r (r x)) ï¼ x
rÂ³ (Î· eâ‚€)            = refl
rÂ³ (Î· eâ‚)            = refl
rÂ³ (sâˆ™ re)           = refl
rÂ³ (râˆ™ eâ‚€)           = refl
rÂ³ (râˆ™ eâ‚)           = refl
rÂ³ (râˆ™ cross re)     = refl
rÂ³ (rÂ²âˆ™ eâ‚€)          = refl
rÂ³ (rÂ²âˆ™ eâ‚)          = refl
rÂ³ (rÂ²âˆ™ cross re)    = refl

rÂ²-r : (x : PSL2Z) â†’ rÂ² (r x) ï¼ x
rÂ²-r = rÂ³

r-rÂ² : (x : PSL2Z) â†’ r (rÂ² x) ï¼ x
r-rÂ² = rÂ³

s-E : s E ï¼ S
s-E = refl

s-S : s S ï¼ E
s-S = refl

r-E : r E ï¼ R
r-E = refl

r-R : r R ï¼ RÂ²
r-R = refl

r-RÂ² : r RÂ² ï¼ E
r-RÂ² = refl

rÂ²-E : rÂ² E ï¼ RÂ²
rÂ²-E = refl

rÂ²-R : rÂ² R ï¼ E
rÂ²-R = refl

rÂ²-RÂ² : rÂ² RÂ² ï¼ R
rÂ²-RÂ² = refl

r-Î· : (se : S-edge) â†’ r (Î· se) ï¼ râˆ™ se
r-Î· eâ‚€         = refl
r-Î· eâ‚         = refl
r-Î· (cross re) = refl

rÂ²-Î· : (se : S-edge) â†’ rÂ² (Î· se) ï¼ rÂ²âˆ™ se
rÂ²-Î· eâ‚€         = refl
rÂ²-Î· eâ‚         = refl
rÂ²-Î· (cross re) = refl

r-Î¸-r+ : (se : S-edge) â†’ r (Î¸ (r+ se)) ï¼ Î¸ (r- se)
r-Î¸-r+ eâ‚€         = refl
r-Î¸-r+ eâ‚         = refl
r-Î¸-r+ (cross re) = refl

r-Î¸-r- : (se : S-edge) â†’ r (Î¸ (r- se)) ï¼ Î· se
r-Î¸-r- eâ‚€         = refl
r-Î¸-r- eâ‚         = refl
r-Î¸-r- (cross re) = refl

rÂ²-Î¸-r+ : (se : S-edge) â†’ rÂ² (Î¸ (r+ se)) ï¼ Î· se
rÂ²-Î¸-r+ se = ap r (r-Î¸-r+ se) âˆ™ r-Î¸-r- se

rÂ²-Î¸-r- : (se : S-edge) â†’ rÂ² (Î¸ (r- se)) ï¼ Î¸ (r+ se)
rÂ²-Î¸-r- se = ap r (r-Î¸-r- se) âˆ™ r-Î· se

sr-Î· : (se : S-edge) â†’ s (r (Î· se)) ï¼ srâˆ™ se
sr-Î· eâ‚€         = refl
sr-Î· eâ‚         = refl
sr-Î· (cross re) = refl

srÂ²-Î· : (se : S-edge) â†’ s (rÂ² (Î· se)) ï¼ srÂ²âˆ™ se
srÂ²-Î· eâ‚€         = refl
srÂ²-Î· eâ‚         = refl
srÂ²-Î· (cross re) = refl

rs-Î¸ : (re : R-edge) â†’ r (s (Î¸ re)) ï¼ rsâˆ™ re
rs-Î¸ (r+ se) = refl
rs-Î¸ (r- se) = refl

rÂ²s-Î¸ : (re : R-edge) â†’ rÂ² (s (Î¸ re)) ï¼ rÂ²sâˆ™ re
rÂ²s-Î¸ (r+ se) = refl
rÂ²s-Î¸ (r- se) = refl

srs-Î¸ : (re : R-edge) â†’ s (r (s (Î¸ re))) ï¼ sâˆ™ r+ cross re
srs-Î¸ (r+ se) = refl
srs-Î¸ (r- se) = refl

srÂ²s-Î¸ : (re : R-edge) â†’ s (rÂ² (s (Î¸ re))) ï¼ sâˆ™ r- cross re
srÂ²s-Î¸ (r+ se) = refl
srÂ²s-Î¸ (r- se) = refl

\end{code}

Cancellation lemmas follow from the order relations. Since sÂ² = 1 and
rÂ³ = 1, the generators are self-inverse (sâ»Â¹ = s, râ»Â¹ = rÂ²) and thus
left-cancellable.

\begin{code}

s-lc : left-cancellable s
s-lc {x} {y} p = sÂ² x â»Â¹ âˆ™ ap s p âˆ™ sÂ² y

r-lc : left-cancellable r
r-lc {x} {y} p = rÂ³ x â»Â¹ âˆ™ ap rÂ² p âˆ™ rÂ³ y

rÂ²-lc : left-cancellable rÂ²
rÂ²-lc = r-lc âˆ˜ r-lc

private
 Î·-helper : PSL2Z â†’ S-edge
 Î·-helper (Î· se) = se
 Î·-helper (Î¸ _) = eâ‚€  -- dummy, but won't be used in valid cases

 Î¸-helper : PSL2Z â†’ R-edge
 Î¸-helper (Î· _) = r+ eâ‚€  -- dummy
 Î¸-helper (Î¸ re) = re

 cross-helper : S-edge â†’ R-edge
 cross-helper (cross re) = re
 cross-helper eâ‚€ = step â‚€ eâ‚€
 cross-helper eâ‚ = step â‚€ eâ‚

 r-helper : R-edge â†’ S-edge
 r-helper (r+ se) = se
 r-helper (r- se) = se

 r-sgn : R-edge â†’ R-sgn
 r-sgn (step d _) = d

\end{code}

The injections Î· and Î¸ are left-cancellable, enabling us to reduce
equality in PSL2Z to equality in the component types.

\begin{code}

Î·-lc : {x y : S-edge} â†’ Id {ğ“¤â‚€} {PSL2Z} (Î· x) (Î· y) â†’ x ï¼ y
Î·-lc refl = refl

Î¸-lc : {x y : R-edge} â†’ Id {ğ“¤â‚€} {PSL2Z} (Î¸ x) (Î¸ y) â†’ x ï¼ y
Î¸-lc refl = refl

S-is-not-E : S â‰  E
S-is-not-E p = ğŸ™-is-not-ğŸ˜ (g (Î·-lc {eâ‚} {eâ‚€} p))
 where
  f : S-edge â†’ ğ“¤â‚€ Ì‡
  f eâ‚€ = ğŸ˜
  f eâ‚ = ğŸ™
  f (cross _) = ğŸ˜

  g : eâ‚ ï¼ eâ‚€ â†’ ğŸ™ ï¼ ğŸ˜
  g = ap f

Î·-is-not-Î¸ : (x : S-edge) (y : R-edge) â†’ Î· x â‰  Î¸ y
Î·-is-not-Î¸ x y p = +disjoint p

Î¸-is-not-Î· : (x : R-edge) (y : S-edge) â†’ Î¸ x â‰  Î· y
Î¸-is-not-Î· x y p = +disjoint (p â»Â¹)

fibers-of-Î·-over-E : (x : S-edge) â†’ is-decidable (Î· x ï¼ E)
fibers-of-Î·-over-E eâ‚€ = inl refl
fibers-of-Î·-over-E eâ‚ = inr S-is-not-E
fibers-of-Î·-over-E (cross x) = inr (Î» p â†’ Î¸-is-not-Î· x eâ‚ (ap s p))

fibers-of-Î·-over-S : (x : S-edge) â†’ is-decidable (Î· x ï¼ S)
fibers-of-Î·-over-S eâ‚€ = inr (Î» p â†’ S-is-not-E (p â»Â¹))
fibers-of-Î·-over-S eâ‚ = inl refl
fibers-of-Î·-over-S (cross x) = inr (Î» p â†’ Î¸-is-not-Î· x eâ‚€ (ap s p))

\end{code}

Decidability of equality is established by mutual recursion on the
graph structure. We decide equality fiber-by-fiber over each
constructor, using the order relations to distinguish r+ from r-.

\begin{code}

fibers-of-Î·-over-cross : (x : S-edge) (y : R-edge)
                       â†’ is-decidable ((inl x) ï¼ inl (cross y))
fibers-of-Î¸-over-r+ : (x : R-edge) (y : S-edge)
                    â†’ is-decidable ((inr x) ï¼ inr (r+ y))
fibers-of-Î¸-over-r- : (x : R-edge) (y : S-edge)
                    â†’ is-decidable ((inr x) ï¼ inr (r- y))

S-edge-is-discrete : is-discrete S-edge
R-edge-is-discrete : is-discrete R-edge

Î·-is-decidable : (x y : S-edge)
               â†’ is-decidable ((inl {ğ“¤â‚€} {ğ“¤â‚€} {S-edge} {R-edge} x) ï¼ inl y)
Î¸-is-decidable : (x y : R-edge)
               â†’ is-decidable ((inr {ğ“¤â‚€} {ğ“¤â‚€} {S-edge} {R-edge} x) ï¼ inr y)

fibers-of-Î·-over-cross eâ‚€ y = inr (Î·-is-not-Î¸ eâ‚ y âˆ˜ ap s)
fibers-of-Î·-over-cross eâ‚ y = inr (Î·-is-not-Î¸ eâ‚€ y âˆ˜ ap s)
fibers-of-Î·-over-cross (cross x) y =
 +functor (ap (Î» re â†’ Î· (cross re)))
          (contrapositive cross-inj)
          (R-edge-is-discrete x y)
 where
  cross-inj : {a b : R-edge} â†’ Î· (cross a) ï¼ Î· (cross b) â†’ a ï¼ b
  cross-inj p = ap (Î¸-helper âˆ˜ s) p

fibers-of-Î¸-over-r+ (r+ x) y =
 +functor (ap (Î» se â†’ Î¸ (r+ se)))
          (contrapositive r+inj)
          (S-edge-is-discrete x y)
 where
  r+inj : {a b : S-edge} â†’ Î¸ (r+ a) ï¼ Î¸ (r+ b) â†’ a ï¼ b
  r+inj {a} {b} p = Î·-lc (rÂ²-Î¸-r+ a â»Â¹ âˆ™ ap rÂ² p âˆ™ rÂ²-Î¸-r+ b)
fibers-of-Î¸-over-r+ (r- x) y = inr lemma
 where
  lemma : Î¸ (r- x) ï¼ Î¸ (r+ y) â†’ ğŸ˜
  lemma p = Î·-is-not-Î¸ x (r- y) (r-Î¸-r- x â»Â¹ âˆ™ ap r p âˆ™ r-Î¸-r+ y)
fibers-of-Î¸-over-r- (r+ x) y = inr lemma
 where
  lemma : Î¸ (r+ x) ï¼ Î¸ (r- y) â†’ ğŸ˜
  lemma p = Î·-is-not-Î¸ x (r+ y) (rÂ²-Î¸-r+ x â»Â¹ âˆ™ ap rÂ² p âˆ™ rÂ²-Î¸-r- y)
fibers-of-Î¸-over-r- (r- x) y =
  +functor (ap (Î» se â†’ Î¸ (r- se)))
           (contrapositive r-inj)
           (S-edge-is-discrete x y)
  where
    r-inj : {a b : S-edge} â†’ Î¸ (r- a) ï¼ Î¸ (r- b) â†’ a ï¼ b
    r-inj {a} {b} p = Î·-lc (r-Î¸-r- a â»Â¹ âˆ™ ap r p âˆ™ r-Î¸-r- b)

S-edge-is-discrete eâ‚€ eâ‚€ = inl refl
S-edge-is-discrete eâ‚€ eâ‚ = inr (Î» p â†’ S-is-not-E (ap inl (p â»Â¹)))
S-edge-is-discrete eâ‚€ (cross y) = inr (Î» p â†’ Î·-is-not-Î¸ eâ‚ y (ap s (ap inl p)))
S-edge-is-discrete eâ‚ eâ‚€ = inr (Î» p â†’ S-is-not-E (ap inl p))
S-edge-is-discrete eâ‚ eâ‚ = inl refl
S-edge-is-discrete eâ‚ (cross y) = inr (Î» p â†’ Î·-is-not-Î¸ eâ‚€ y (ap s (ap inl p)))
S-edge-is-discrete (cross x) eâ‚€ =
  inr (Î» p â†’ Î·-is-not-Î¸ eâ‚ x (ap s (ap inl (p â»Â¹))))
S-edge-is-discrete (cross x) eâ‚ =
  inr (Î» p â†’ Î·-is-not-Î¸ eâ‚€ x (ap s (ap inl (p â»Â¹))))
S-edge-is-discrete (cross x) (cross y) =
  +functor (ap cross) (contrapositive cross-inj) (R-edge-is-discrete x y)
  where
    cross-inj : {a b : R-edge} â†’ cross a ï¼ cross b â†’ a ï¼ b
    cross-inj {a} {b} p = ap cross-helper p

R-edge-is-discrete (r+ x) (r+ y) =
 +functor (ap (Î» se â†’ r+ se)) (contrapositive r+inj) (S-edge-is-discrete x y)
 where
   r+inj : {a b : S-edge} â†’ r+ a ï¼ r+ b â†’ a ï¼ b
   r+inj {a} {b} p = ap r-helper p
R-edge-is-discrete (r+ x) (r- y) = inr (Î» p â†’ zero-is-not-one (ap r-sgn p))
R-edge-is-discrete (r- x) (r+ y) = inr (Î» p â†’ one-is-not-zero (ap r-sgn p))
R-edge-is-discrete (r- x) (r- y) =
 +functor (ap (Î» se â†’ r- se)) (contrapositive r-inj) (S-edge-is-discrete x y)
 where
   r-inj : {a b : S-edge} â†’ r- a ï¼ r- b â†’ a ï¼ b
   r-inj {a} {b} p = ap r-helper p

Î·-is-decidable x eâ‚€ = fibers-of-Î·-over-E x
Î·-is-decidable x eâ‚ = fibers-of-Î·-over-S x
Î·-is-decidable x (cross y) = fibers-of-Î·-over-cross x y

Î¸-is-decidable x (r+ y) = fibers-of-Î¸-over-r+ x y
Î¸-is-decidable x (r- y) = fibers-of-Î¸-over-r- x y

PSL2Z-is-discrete : is-discrete PSL2Z
PSL2Z-is-discrete (Î· x) (Î· y) = Î·-is-decidable x y
PSL2Z-is-discrete (Î· x) (Î¸ y) = inr (Î·-is-not-Î¸ x y)
PSL2Z-is-discrete (Î¸ x) (Î· y) = inr (â‰ -sym (Î·-is-not-Î¸ y x))
PSL2Z-is-discrete (Î¸ x) (Î¸ y) = Î¸-is-decidable x y

PSL2Z-is-set : is-set PSL2Z
PSL2Z-is-set = discrete-types-are-sets PSL2Z-is-discrete

\end{code}

Although we have our main result, why not these as well.

\begin{code}

S-edge-is-set : is-set S-edge
S-edge-is-set = discrete-types-are-sets S-edge-is-discrete

R-edge-is-set : is-set R-edge
R-edge-is-set = discrete-types-are-sets R-edge-is-discrete

\end{code}
