Martin Escardo, 2014.

\begin{code}

{-# OPTIONS --safe --without-K #-}

module Fin.Type where

open import UF.Subsingletons

open import MLTT.Spartan
open import MLTT.Plus-Properties

Fin : â„• â†’ ğ“¤â‚€ Ì‡
Fin 0        = ğŸ˜
Fin (succ n) = Fin n + ğŸ™

\end{code}

We have zero and successor for finite sets, with the following types:

\begin{code}

fzero : {n : â„•} â†’ Fin (succ n)
fzero = inr â‹†

fsucc : {n : â„•} â†’ Fin n â†’ Fin (succ n)
fsucc = inl

suc-lc : {n : â„•} {j k : Fin n} â†’ fsucc j ï¼ fsucc k â†’ j ï¼ k
suc-lc = inl-lc

\end{code}

But it will more convenient to have them as patterns, for the sake of
clarity in definitions by pattern matching:

\begin{code}

pattern ğŸ     = inr â‹†
pattern ğŸ     = inl (inr â‹†)
pattern ğŸ     = inl (inl (inr â‹†))
pattern suc i = inl i

\end{code}

The induction principle for Fin is proved by induction on â„•:

\begin{code}

Fin-induction : (P : (n : â„•) â†’ Fin n â†’ ğ“¤ Ì‡ )
              â†’ ((n : â„•) â†’ P (succ n) ğŸ)
              â†’ ((n : â„•) (i : Fin n) â†’ P n i â†’ P (succ n) (suc i))
              â†’  (n : â„•) (i : Fin n) â†’ P n i

Fin-induction P Î² Ïƒ 0        i       = ğŸ˜-elim i
Fin-induction P Î² Ïƒ (succ n) ğŸ       = Î² n
Fin-induction P Î² Ïƒ (succ n) (suc i) = Ïƒ n i (Fin-induction P Î² Ïƒ n i)

\end{code}
