Martin Escardo, Chuangjie Xu, 2012.

As a simple application of coinduction and corecursion on â„•âˆ, one can
show that the the inclusion map incl : â„•âˆ â†’ â‚‚â„• is part of a
retraction.

This exercise is artificial: a direct construction and proof of the
retraction would be shorter and perhaps clearer. However, it does
illustrate how co-recursion and co-induction can be used.

Recall that a retraction is a pair of maps r : X â†’ Y and s : Y â†’ X
such that r âˆ˜ s : Y â†’ Y is the identity, where r is called the
retraction and s the section. In this case, it follows that
s âˆ˜ r : X â†’ X is idempotent, and s is an injection and r is a
surjection. When such maps exists one says that Y is a retract of X.

The idea of the construction of the retraction is that we "read"
digits from Î± until we find a zero or forever, and count how long
this took.

\begin{code}

{-# OPTIONS --without-K --exact-split --safe --auto-inline #-}

open import UF-FunExt

module CoNaturalsExercise (fe : FunExt) where

open import SpartanMLTT
open import Two-Properties
open import CoNaturals fe
open import GenericConvergentSequence
open import Sequence fe
open import CanonicalMapNotation

â„•âˆ-to-â„•â†’ğŸš-is-a-section : Î£ Ï ê‰ ((â„• â†’ ğŸš) â†’ â„•âˆ) , Ï âˆ˜ Î¹ â‰¡ id
â„•âˆ-to-â„•â†’ğŸš-is-a-section  = Ï , dfunext (fe ğ“¤â‚€ ğ“¤â‚€) lemma
 where
  f-Ï : ğŸš â†’ (â„• â†’ ğŸš) â†’ ğŸ™ + (â„• â†’ ğŸš)
  f-Ï â‚€ Î± = inl â‹†
  f-Ï â‚ Î± = inr Î±

  p-Ï : (â„• â†’ ğŸš) â†’ ğŸ™ + (â„• â†’ ğŸš)
  p-Ï Î± = f-Ï (head Î±) (tail Î±)

  Ï : (â„• â†’ ğŸš) â†’ â„•âˆ
  Ï = â„•âˆ-corec p-Ï

  Ï-spec : PRED âˆ˜ Ï â‰¡ (ğŸ™+ Ï) âˆ˜ p-Ï
  Ï-spec = â„•âˆ-corec-homomorphism p-Ï

  Ï-specâ‚€ : (Î± : â„• â†’ ğŸš) â†’ head Î± â‰¡ â‚€ â†’ Ï Î± â‰¡ Zero
  Ï-specâ‚€ Î± r = coalg-morphism-Zero p-Ï Ï Ï-spec Î± â‹† lemma
   where
    lemma : p-Ï Î± â‰¡ inl â‹†
    lemma = ap (Î» - â†’ f-Ï - (tail Î±)) r

  Ï-specâ‚ : (Î± : â„• â†’ ğŸš) â†’ head Î± â‰¡ â‚ â†’ Ï Î± â‰¡ Succ (Ï (tail Î±))
  Ï-specâ‚ Î± r = coalg-morphism-Succ p-Ï Ï Ï-spec Î± (tail Î±) lemma
   where
    lemma : p-Ï Î± â‰¡ inr (tail Î±)
    lemma = ap (Î» - â†’ f-Ï - (tail Î±)) r

  R : â„•âˆ â†’ â„•âˆ â†’ ğ“¤â‚€ Ì‡
  R u v = Î£ w ê‰ â„•âˆ , (Ï (Î¹ w) â‰¡ u) Ã— (w â‰¡ v)

  r : (u : â„•âˆ) â†’ R (Ï (Î¹ u)) u
  r u = (u , refl , refl)

  R-positivity : (u v : â„•âˆ) â†’ R u v â†’ positivity u â‰¡ positivity v
  R-positivity u v (w , c , d) = ğŸš-equality-cases lemmaâ‚€ lemmaâ‚
   where
    lemmaâ‚€ : positivity w â‰¡ â‚€ â†’ positivity u â‰¡ positivity v
    lemmaâ‚€ r = ap positivity claimâ‚ƒ
     where
      claimâ‚€ : Ï (Î¹ w) â‰¡ Zero
      claimâ‚€ = Ï-specâ‚€ (Î¹ w) r
      claimâ‚ : v â‰¡ Zero
      claimâ‚ = d â»Â¹ âˆ™ is-Zero-equal-Zero (fe ğ“¤â‚€ ğ“¤â‚€) r
      claimâ‚‚ : Ï (Î¹ w) â‰¡ v
      claimâ‚‚ = claimâ‚€ âˆ™ claimâ‚ â»Â¹
      claimâ‚ƒ : u â‰¡ v
      claimâ‚ƒ = c â»Â¹ âˆ™ claimâ‚‚

    lemmaâ‚ : positivity w â‰¡ â‚ â†’ positivity u â‰¡ positivity v
    lemmaâ‚ r = claimâ‚‚ âˆ™ claimâ‚„ â»Â¹
     where
      claimâ‚€ : positivity (Ï (Î¹ w)) â‰¡ â‚
      claimâ‚€ = ap positivity (Ï-specâ‚ (Î¹ w) r)

      claimâ‚ : positivity (Ï (Î¹ w)) â‰¡ positivity u
      claimâ‚ = ap positivity c

      claimâ‚‚ : positivity u â‰¡ â‚
      claimâ‚‚ = claimâ‚ â»Â¹ âˆ™ claimâ‚€
      claimâ‚ƒ : positivity w â‰¡ positivity v
      claimâ‚ƒ = ap positivity d

      claimâ‚„ : positivity v â‰¡ â‚
      claimâ‚„ = claimâ‚ƒ â»Â¹ âˆ™ r

  R-Pred : (u v : â„•âˆ) â†’ R u v â†’ R (Pred u) (Pred v)
  R-Pred u v (w , c , d) = (Pred w , lemmaâ‚€ , lemmaâ‚)
   where
    lemmaâ‚€ : Ï (Î¹ (Pred w)) â‰¡ Pred u
    lemmaâ‚€ = claim âˆ™ claimâ‚€
     where
     claimâ‚€ : Pred (Ï (Î¹ w)) â‰¡ Pred u
     claimâ‚€ = ap Pred c

     claim :  Ï (Î¹ (Pred w)) â‰¡ Pred (Ï (Î¹ w))
     claim = ğŸš-equality-cases claimâ‚ claimâ‚‚
      where
       claimâ‚ : is-Zero w â†’ Ï (Î¹ (Pred w)) â‰¡ Pred (Ï (Î¹ w))
       claimâ‚ r = câ‚ƒ âˆ™ câ‚… â»Â¹
        where
         câ‚€ : w â‰¡ Zero
         câ‚€ = is-Zero-equal-Zero (fe ğ“¤â‚€ ğ“¤â‚€) r
         câ‚ : Pred w â‰¡ Zero
         câ‚ = ap Pred câ‚€

         câ‚‚ : Î¹ (Pred w) 0 â‰¡ â‚€
         câ‚‚ = ap (head âˆ˜ Î¹) câ‚

         câ‚ƒ : Ï (Î¹ (Pred w)) â‰¡ Zero
         câ‚ƒ = Ï-specâ‚€ (Î¹ (Pred w)) câ‚‚

         câ‚„ : Ï (Î¹ w) â‰¡ Zero
         câ‚„ = Ï-specâ‚€ (Î¹ w) r

         câ‚… : Pred (Ï (Î¹ w)) â‰¡ Zero
         câ‚… = ap Pred câ‚„
       claimâ‚‚ : is-positive w â†’ Ï (Î¹ (Pred w)) â‰¡ Pred (Ï (Î¹ w))
       claimâ‚‚ r = câ‚ƒ âˆ™ câ‚ â»Â¹
        where
         câ‚€ : Ï (Î¹ w) â‰¡ Succ (Ï (tail (Î¹ w)))
         câ‚€ = Ï-specâ‚ (Î¹ w) r

         câ‚ : Pred (Ï (Î¹ w)) â‰¡ Ï (tail (Î¹ w))
         câ‚ = ap Pred câ‚€ âˆ™ Pred-Succ

         câ‚ƒ : Ï (Î¹ (Pred w)) â‰¡ Ï (tail (Î¹ w))
         câ‚ƒ = refl

    lemmaâ‚ : Pred w â‰¡ Pred v
    lemmaâ‚ = ap Pred d

  R-bisimulation : â„•âˆ-bisimulation R
  R-bisimulation u v r = (R-positivity u v r , R-Pred u v r)

  lemma : (u : â„•âˆ) â†’ Ï (Î¹ u) â‰¡ u
  lemma u = â„•âˆ-coinduction R R-bisimulation (Ï (Î¹ u)) u (r u)

\end{code}
