Martin Escardo 20-21 December 2012

Development adapted from the module ConvergentSequenceCompact:

Not only is â„•âˆ compact (or searchable), but, moreover, minimal
witnesses can be found.

\begin{code}

{-# OPTIONS --without-K --exact-split --safe --auto-inline #-}

open import UF-FunExt
open import SpartanMLTT

module ConvergentSequenceHasInf (feâ‚€ : funext ğ“¤â‚€ ğ“¤â‚€) where


open import Two-Properties
open import InfProperty
open import GenericConvergentSequence
open import OrderNotation
open import CanonicalMapNotation

â„•âˆ-has-inf : has-inf _â‰¼_
â„•âˆ-has-inf p = a , putative-root-lemma , lower-bound-lemma , uborlb-lemma
 where
  Î± : â„• â†’ ğŸš
  Î± 0       = p (Î¹ 0)
  Î± (succ n) = minğŸš (Î± n) (p (Î¹ (succ n)))

  a : â„•âˆ
  a = (Î± , Î» i â†’ Lemma[minabâ‰¤â‚‚a])

  Daggerâ‚€ : (n : â„•) â†’ a â‰¡ Î¹ n â†’ p (Î¹ n) â‰¡ â‚€
  Daggerâ‚€ 0        r = ap (Î» - â†’ Î¹ - 0) r
  Daggerâ‚€ (succ n) r = p (Î¹ (succ n)) â‰¡âŸ¨ w âŸ©
                       Î± (succ n)     â‰¡âŸ¨ t âŸ©
                       â‚€              âˆ
   where
    s : Î± n â‰¡ â‚
    s = ap (Î» - â†’ Î¹ - n) r âˆ™ Î¹-diagonalâ‚ n

    t = Î± (succ n)              â‰¡âŸ¨ ap (Î» - â†’ Î¹ - (succ n)) r âŸ©
        Î¹ (Î¹ (succ n)) (succ n) â‰¡âŸ¨ Î¹-diagonalâ‚€ n âŸ©
        â‚€                       âˆ

    w : p (Î¹ (succ n)) â‰¡ Î± (succ n)
    w = (ap (Î» - â†’ minğŸš - (p (Î¹ (succ n)))) s)â»Â¹

  Daggerâ‚ : a â‰¡ âˆ â†’ (n : â„•) â†’ p (Î¹ n) â‰¡ â‚
  Daggerâ‚ r 0 = ap (Î» - â†’ Î¹ - 0) r
  Daggerâ‚ r (succ n) = p (Î¹ (succ n)) â‰¡âŸ¨ w âŸ©
                       Î± (succ n)     â‰¡âŸ¨ t âŸ©
                       â‚              âˆ
   where
    s : Î± n â‰¡ â‚
    s = ap (Î» - â†’ Î¹ - n) r

    t : Î± (succ n) â‰¡ â‚
    t = ap (Î» - â†’ Î¹ - (succ n)) r

    w : p (Î¹ (succ n)) â‰¡ Î± (succ n)
    w = (ap (Î» - â†’ minğŸš - (p (Î¹ (succ n)))) s)â»Â¹

  Claimâ‚€ : p a â‰¡ â‚ â†’ (n : â„•) â†’ a â‰¢ Î¹ n
  Claimâ‚€ r n s = equal-â‚-different-from-â‚€ r (Lemma s)
   where
    Lemma : a â‰¡ Î¹ n â†’ p a â‰¡ â‚€
    Lemma t = p a     â‰¡âŸ¨ ap p t âŸ©
              p (Î¹ n) â‰¡âŸ¨ Daggerâ‚€ n t âŸ©
              â‚€       âˆ

  Claimâ‚ : p a â‰¡ â‚ â†’ a â‰¡ âˆ
  Claimâ‚ r = not-finite-is-âˆ feâ‚€ (Claimâ‚€ r)

  Claimâ‚‚ : p a â‰¡ â‚ â†’ (n : â„•) â†’ p (Î¹ n) â‰¡ â‚
  Claimâ‚‚ r = Daggerâ‚ (Claimâ‚ r)

  Claimâ‚ƒ : p a â‰¡ â‚ â†’ p âˆ â‰¡ â‚
  Claimâ‚ƒ r = p âˆ â‰¡âŸ¨ (ap p (Claimâ‚ r))â»Â¹ âŸ©
             p a â‰¡âŸ¨ r âŸ©
             â‚   âˆ

  Lemma : p a â‰¡ â‚ â†’ (v : â„•âˆ) â†’ p v â‰¡ â‚
  Lemma r = â„•âˆ-ğŸš-density feâ‚€ (Claimâ‚‚ r) (Claimâ‚ƒ r)

  putative-root-lemma : (Î£ u ê‰ â„•âˆ , p u â‰¡ â‚€) â†’ p a â‰¡ â‚€
  putative-root-lemma (x , r) = lemma claim
   where
    lemma : Â¬ ((x : â„•âˆ) â†’ p x â‰¡ â‚) â†’ p a â‰¡ â‚€
    lemma = different-from-â‚-equal-â‚€ âˆ˜ (contrapositive Lemma)

    claim : Â¬ ((x : â„•âˆ) â†’ p x â‰¡ â‚)
    claim f = equal-â‚-different-from-â‚€ (f x) r

  lower-bound-lemma : (u : â„•âˆ)â†’ p u â‰¡ â‚€ â†’ a â‰¼ u
  lower-bound-lemma u r 0 s = lemma
    where
     claimâ‚€ : Î¹ u 0 â‰¡ â‚€ â†’ p u â‰¡ Î± 0
     claimâ‚€ t = ap p (is-Zero-equal-Zero feâ‚€ t)

     claimâ‚ : Î¹ u 0 â‰¡ â‚€ â†’ â‚€ â‰¡ â‚
     claimâ‚ t = â‚€   â‰¡âŸ¨ r â»Â¹ âŸ©
                p u â‰¡âŸ¨ claimâ‚€ t âŸ©
                Î± 0 â‰¡âŸ¨ s âŸ©
                â‚   âˆ

     lemma : Î¹ u 0 â‰¡ â‚
     lemma = different-from-â‚€-equal-â‚ (contrapositive claimâ‚ zero-is-not-one)

  lower-bound-lemma u r (succ n) s = lemma
   where
    remark : minğŸš (Î¹ a n) (p (Î¹ (succ n))) â‰¡ â‚
    remark = s

    IH : Î¹ a n â‰¡ â‚ â†’ Î¹ u n â‰¡ â‚
    IH = lower-bound-lemma u r n

    claimâ‚€ : Î¹ u n â‰¡ â‚
    claimâ‚€ = IH (Lemma[minğŸšabâ‰¡â‚â†’aâ‰¡â‚] s)

    claimâ‚ : p (Î¹ (succ n)) â‰¡ â‚
    claimâ‚ = Lemma[minğŸšabâ‰¡â‚â†’bâ‰¡â‚]{(Î¹ a n)} s

    claimâ‚‚ : Î¹ u (succ n) â‰¡ â‚€ â†’ u â‰¡ Î¹ (succ n)
    claimâ‚‚ = Succ-criterion feâ‚€ claimâ‚€

    claimâ‚ƒ : Î¹ u (succ n) â‰¡ â‚€ â†’ p u â‰¡ p (Î¹ (succ n))
    claimâ‚ƒ t = ap p (claimâ‚‚ t)

    claimâ‚„ : Î¹ u (succ n) â‰¡ â‚€ â†’ p u â‰¡ â‚
    claimâ‚„ t = p u            â‰¡âŸ¨ claimâ‚ƒ t âŸ©
               p (Î¹ (succ n)) â‰¡âŸ¨ claimâ‚ âŸ©
               â‚              âˆ

    claimâ‚… : Î¹ u (succ n) â‰¢ â‚€
    claimâ‚… t = equal-â‚-different-from-â‚€ (claimâ‚„ t) r

    lemma : Î¹ u (succ n) â‰¡ â‚
    lemma = different-from-â‚€-equal-â‚ claimâ‚…

  uborlb-lemma : (l : â„•âˆ) â†’ ((x : â„•âˆ) â†’ p x â‰¡ â‚€ â†’ l â‰¼ x) â†’ l â‰¼ a
  uborlb-lemma l lower-bounder = ğŸš-equality-cases lemmaâ‚€ lemmaâ‚
   where
    lemmaâ‚€ : p a â‰¡ â‚€ â†’ l â‰¼ a
    lemmaâ‚€ = lower-bounder a

    lemmaâ‚ : p a â‰¡ â‚ â†’ l â‰¼ a
    lemmaâ‚ r n x = ap (Î» - â†’ Î¹ - n) (Claimâ‚ r)

\end{code}
