Martin Escardo 2011.

(Totally separated types moved to the module TotallySeparated January
2018, and extended.)

\begin{code}

{-# OPTIONS --without-K --exact-split --safe #-}

module DiscreteAndSeparated where

open import UF
open import DecidableAndDetachable

isolated : âˆ€ {U} {X : U Ì‡} â†’ X â†’ U Ì‡
isolated x = âˆ€ y â†’ decidable(x â‰¡ y)

discrete : âˆ€ {U} â†’ U Ì‡ â†’ U Ì‡
discrete X = (x : X) â†’ isolated x

\end{code}

A simple example:

\begin{code}

open import Two

ğŸš-discrete : discrete ğŸš
ğŸš-discrete â‚€ â‚€ = inl refl
ğŸš-discrete â‚€ â‚ = inr(Î» ())
ğŸš-discrete â‚ â‚€ = inr(Î» ())
ğŸš-discrete â‚ â‚ = inl refl

\end{code}

General properties:

\begin{code}

discrete-is-cotransitive : âˆ€ {U} {X : U Ì‡}
                         â†’ discrete X â†’ {x y z : X} â†’ x â‰¢ y â†’  x â‰¢ z  +  z â‰¢ y
discrete-is-cotransitive d {x} {y} {z} Ï† = f(d x z)
 where 
  f : x â‰¡ z  +  x â‰¢ z â†’ x â‰¢ z  +  z â‰¢ y
  f (inl r) = inr (Î» s â†’ Ï†(r âˆ™ s)) 
  f (inr Î³) = inl Î³ 

retract-discrete-discrete : âˆ€ {U} {V} {X : U Ì‡} {Y : V Ì‡}
                         â†’ retract Y of X â†’ discrete X â†’ discrete Y
retract-discrete-discrete (f , (s , Ï†)) d y y' = g (d (s y) (s y'))
 where
  g : decidable (s y â‰¡ s y') â†’ decidable (y â‰¡ y')
  g (inl p) = inl ((Ï† y) â»Â¹ âˆ™ ap f p âˆ™ Ï† y')
  g (inr u) = inr (contrapositive (ap s) u)

ğŸš-retract-of-discrete : âˆ€ {U} {X : U Ì‡} {xâ‚€ xâ‚ : X} â†’ xâ‚€ â‰¢ xâ‚ â†’ discrete X â†’ retract ğŸš of X
ğŸš-retract-of-discrete {U} {X} {xâ‚€} {xâ‚} ne d = r , (s , rs)
 where
  r : X â†’ ğŸš
  r = prâ‚ (characteristic-function (d xâ‚€))
  
  Ï† : (x : X) â†’ (r x â‰¡ â‚€ â†’ xâ‚€ â‰¡ x) Ã— (r x â‰¡ â‚ â†’ Â¬ (xâ‚€ â‰¡ x))
  Ï† = prâ‚‚ (characteristic-function (d xâ‚€))
  
  s : ğŸš â†’ X
  s â‚€ = xâ‚€
  s â‚ = xâ‚
  
  rs : (n : ğŸš) â†’ r (s n) â‰¡ n
  rs â‚€ = Lemma[bâ‰¢â‚â†’bâ‰¡â‚€] (Î» p â†’ prâ‚‚ (Ï† xâ‚€) p refl)
  rs â‚ = Lemma[bâ‰¢â‚€â†’bâ‰¡â‚] Î» p â†’ ğŸ˜-elim (ne (prâ‚ (Ï† xâ‚) p))
  
\end{code}

Separated types form an exponential ideal, assuming
extensionality. More generally:

\begin{code}

separated : âˆ€ {U} â†’ U Ì‡ â†’ U Ì‡
separated X = (x y : X) â†’ Â¬Â¬(x â‰¡ y) â†’ x â‰¡ y

separated-ideal : âˆ€ {U V} â†’ FunExt U V â†’ {X : U Ì‡} {Y : X â†’ V Ì‡}
               â†’ ((x : X) â†’ separated(Y x)) â†’ separated(Î  Y)
separated-ideal fe s f g h = funext fe lemmağŸš
 where 
  lemmaâ‚€ : f â‰¡ g â†’ âˆ€ x â†’ f x â‰¡ g x
  lemmaâ‚€ r x = ap (Î» h â†’ h x) r

  lemmaâ‚ : âˆ€ x â†’ Â¬Â¬(f x â‰¡ g x)
  lemmaâ‚ = DNU(Â¬Â¬-functor lemmaâ‚€ h)

  lemmağŸš : âˆ€ x â†’ f x â‰¡ g x
  lemmağŸš x =  s x (f x) (g x) (lemmaâ‚ x) 

discrete-is-separated : âˆ€ {U} {X : U Ì‡} â†’ discrete X â†’ separated X
discrete-is-separated d x y = Â¬Â¬-elim(d x y)

ğŸš-separated : separated ğŸš
ğŸš-separated = discrete-is-separated ğŸš-discrete

subtype-of-separated-is-separated : âˆ€ {U V} {X : U Ì‡} {Y : V Ì‡} (m : X â†’ Y)
                                  â†’ left-cancellable m â†’ separated Y â†’ separated X
subtype-of-separated-is-separated {U} {V} {X} m i s x x' e = i (s (m x) (m x') (Â¬Â¬-functor (ap m) e))

\end{code}

The following is an apartness relation when Y is separated, but we
define it without this assumption. (Are all types separated? See
below.)

\begin{code}

infix 21 _â™¯_

_â™¯_ : âˆ€ {U V} {X : U Ì‡} â†’ {Y : X â†’ V Ì‡} â†’ (f g : (x : X) â†’ Y x) â†’ U âŠ” V Ì‡
f â™¯ g = Î£ \x â†’ f x â‰¢ g x


apart-is-different : âˆ€ {U V} {X : U Ì‡} {Y : X â†’ V Ì‡}
                   â†’ {f g : (x : X) â†’ Y x} â†’ f â™¯ g â†’ f â‰¢ g
apart-is-different (x , Ï†) r = Ï† (ap (Î» h â†’ h x) r)


apart-is-symmetric : âˆ€ {U V} {X : U Ì‡} â†’ {Y : X â†’ V Ì‡}
                   â†’ {f g : (x : X) â†’ Y x} â†’ f â™¯ g â†’ g â™¯ f
apart-is-symmetric (x , Ï†)  = (x , (Ï† âˆ˜ _â»Â¹)) 

apart-is-cotransitive : âˆ€ {U V} {X : U Ì‡} â†’ {Y : X â†’ V Ì‡}
                     â†’ ((x : X) â†’ discrete(Y x)) 
                     â†’ (f g h : (x : X) â†’ Y x)
                     â†’ f â™¯ g â†’ f â™¯ h  +  h â™¯ g
apart-is-cotransitive d f g h (x , Ï†)  = lemmaâ‚(lemmaâ‚€ Ï†)
 where 
  lemmaâ‚€ : f x â‰¢ g x â†’ f x â‰¢ h x  +  h x â‰¢ g x
  lemmaâ‚€ = discrete-is-cotransitive (d x)

  lemmaâ‚ : f x â‰¢ h x  +  h x â‰¢ g x â†’ f â™¯ h  +  h â™¯ g
  lemmaâ‚ (inl Î³) = inl (x , Î³)
  lemmaâ‚ (inr Î´) = inr (x , Î´)

\end{code}

We now consider two cases which render the apartness relation â™¯ tight,
assuming extensionality:

\begin{code}

tight : âˆ€ {U V} {X : U Ì‡} â†’ FunExt U V â†’ {Y : X â†’ V Ì‡}
      â†’ ((x : X) â†’ separated(Y x))
      â†’ (f g : (x : X) â†’ Y x)
      â†’ Â¬(f â™¯ g) â†’ f â‰¡ g
tight fe s f g h = funext fe lemmaâ‚
 where 
  lemmaâ‚€ : âˆ€ x â†’ Â¬Â¬(f x â‰¡ g x)
  lemmaâ‚€ = not-exists-implies-forall-not h

  lemmaâ‚ : âˆ€ x â†’ f x â‰¡ g x
  lemmaâ‚ x = (s x (f x) (g x)) (lemmaâ‚€ x)


tight' : âˆ€ {U V} {X : U Ì‡} â†’ FunExt U V â†’ {Y : X â†’ V Ì‡}
       â†’ ((x : X) â†’ discrete(Y x)) â†’ (f g : (x : X) â†’ Y x) â†’ Â¬(f â™¯ g) â†’ f â‰¡ g
tight' fe d = tight fe (Î» x â†’ discrete-is-separated(d x)) 

\end{code}

What about sums? The special case they reduce to binary products is
easy:

\begin{code}

binary-product-separated : âˆ€ {U V} {X : U Ì‡} {Y : V Ì‡}
                         â†’ separated X â†’ separated Y â†’ separated(X Ã— Y)
binary-product-separated s t (x , y) (x' , y') Ï† = 
 lemma(lemmaâ‚€ Ï†)(lemmaâ‚ Ï†) 
 where 
  lemmaâ‚€ : Â¬Â¬((x , y) â‰¡ (x' , y')) â†’ x â‰¡ x'
  lemmaâ‚€ = (s x x') âˆ˜ Â¬Â¬-functor(ap prâ‚)

  lemmaâ‚ : Â¬Â¬((x , y) â‰¡ (x' , y')) â†’ y â‰¡ y'
  lemmaâ‚ = (t y y') âˆ˜ Â¬Â¬-functor(ap prâ‚‚)

  lemma : x â‰¡ x' â†’ y â‰¡ y' â†’ (x , y) â‰¡ (x' , y')
  lemma = apâ‚‚ (_,_)  

\end{code}

This proof doesn't work for general dependent sums, because, among
other things, (ap Ï€â‚) doesn't make sense in that case.  A different
special case is also easy:

\begin{code}

binary-sum-separated : âˆ€ {U V} {X : U Ì‡} {Y : V Ì‡}
                     â†’ separated X â†’ separated Y â†’ separated(X + Y)
binary-sum-separated {U} {V} {X} {Y} s t (inl x) (inl x') = lemma 
 where
  claim : inl x â‰¡ inl x' â†’ x â‰¡ x'
  claim = ap p
   where p : X + Y â†’ X
         p(inl u) = u
         p(inr v) = x

  lemma : Â¬Â¬(inl x â‰¡ inl x') â†’ inl x â‰¡ inl x'
  lemma = (ap inl) âˆ˜ (s x x') âˆ˜ Â¬Â¬-functor claim

binary-sum-separated s t (inl x) (inr y) =  Î» Ï† â†’ ğŸ˜-elim(Ï† sum-disjoint )  
binary-sum-separated s t (inr y) (inl x)  = Î» Ï† â†’ ğŸ˜-elim(Ï†(sum-disjoint âˆ˜ _â»Â¹)) 
binary-sum-separated {U} {V} {X} {Y} s t (inr y) (inr y') = lemma 
 where
  claim : inr y â‰¡ inr y' â†’ y â‰¡ y'
  claim = ap q
   where
     q : X + Y â†’ Y
     q(inl u) = y
     q(inr v) = v

  lemma : Â¬Â¬(inr y â‰¡ inr y') â†’ inr y â‰¡ inr y'
  lemma = (ap inr) âˆ˜ (t y y') âˆ˜ Â¬Â¬-functor claim

âŠ¥-âŠ¤-density' : FunExt Uâ‚€ Uâ‚€ â†’ propExt Uâ‚€ â†’ âˆ€ {U} {X : U Ì‡}
              â†’ separated X
              â†’ (f : Prop â†’ X) â†’ f âŠ¥ â‰¡ f âŠ¤ â†’ constant f
âŠ¥-âŠ¤-density' fe pe s f r p q = g p âˆ™ (g q)â»Â¹
  where
    a : âˆ€ p â†’ Â¬Â¬(f p â‰¡ f âŠ¤)
    a p t = no-truth-values-other-than-âŠ¥-or-âŠ¤ fe pe (p , (b , c))
      where
        b : p â‰¢ âŠ¥
        b u = t (ap f u âˆ™ r)
        
        c : p â‰¢ âŠ¤
        c u = t (ap f u)
        
    g : âˆ€ p â†’ f p â‰¡ f âŠ¤
    g p = s (f p) (f âŠ¤) (a p)

\end{code}
