Martin Escardo, 2012

\begin{code}

{-# OPTIONS --without-K --exact-split --safe #-}


open import UF

module EquivalenceExamples where

Curry-Uncurry : (fe : âˆ€ {U V} â†’ FunExt U V)
             â†’ âˆ€ {U V W} {X : U Ì‡} {Y : X â†’ V Ì‡} {Z : (Î£ \(x : X) â†’ Y x) â†’ W Ì‡}
             â†’ Î  Z â‰ƒ Î  \(x : X) â†’ Î  \(y : Y x) â†’ Z(x , y)
Curry-Uncurry fe {U} {V} {W} {X} {Y} {Z} = c , (u , cu) , (u , uc)
   where
    c : (w : Î  Z) â†’ ((x : X) (y : Y x) â†’ Z(x , y))
    c f x y = f (x , y)
    u : ((x : X) (y : Y x) â†’ Z(x , y)) â†’ Î  Z
    u g (x , y) = g x y
    cu : âˆ€ g â†’ c (u g) â‰¡ g
    cu g = funext fe (Î» x â†’ funext fe (Î» y â†’ refl))
    uc : âˆ€ f â†’ u (c f) â‰¡ f
    uc f = funext fe (Î» w â†’ refl)

Î£-assoc : âˆ€ {U V W} â†’ {X : U Ì‡} {Y : X â†’ V Ì‡} {Z : (Î£ \(x : X) â†’ Y x) â†’ W Ì‡}
        â†’ Î£ Z â‰ƒ (Î£ \(x : X) â†’ Î£ \(y : Y x) â†’ Z(x , y))
Î£-assoc {U} {V} {W} {X} {Y} {Z} = c , (u , Î» Ï„ â†’ refl) , (u , Î» Ïƒ â†’ refl) 
   where
    c : Î£ Z â†’ Î£ \x â†’ Î£ \y â†’ Z (x , y)
    c ((x , y) , z) = (x , (y , z))
    u : (Î£ \x â†’ Î£ \y â†’ Z (x , y)) â†’ Î£ Z 
    u (x , (y , z)) = ((x , y) , z)

Î£-â‰ƒ-congruence : âˆ€ {U V} (X : U Ì‡) (Y Y' : X â†’ V Ì‡)
               â†’ ((x : X) â†’ Y x â‰ƒ Y' x) â†’ Î£ Y â‰ƒ Î£ Y'
Î£-â‰ƒ-congruence X Y Y' Ï† = (F , (G , FG) , (H , HF))
   where
    f : (x : X) â†’ Y x â†’ Y' x
    f x = prâ‚(Ï† x)
    g : (x : X) â†’ Y' x â†’ Y x
    g x = prâ‚(prâ‚(prâ‚‚(Ï† x)))
    fg : (x : X) (y' : Y' x) â†’ f x (g x y') â‰¡ y' 
    fg x = prâ‚‚(prâ‚(prâ‚‚(Ï† x)))
    h : (x : X) â†’ Y' x â†’ Y x
    h x = prâ‚(prâ‚‚(prâ‚‚(Ï† x)))
    hf : (x : X) (y : Y x) â†’ h x (f x y) â‰¡ y  
    hf x = prâ‚‚(prâ‚‚(prâ‚‚(Ï† x)))
  
    F : Î£ Y â†’ Î£ Y'
    F (x , y) = x , f x y
    G : Î£ Y' â†’ Î£ Y
    G (x , y') = x , (g x y')
    H : Î£ Y' â†’ Î£ Y
    H (x , y') = x , h x y'
    FG : (w' : Î£ Y') â†’ F(G w') â‰¡ w'
    FG (x , y') = Î£-â‰¡' x _ y' (fg x y')
    HF : (w : Î£ Y) â†’ H(F w) â‰¡ w
    HF (x , y) = Î£-â‰¡' x _ y (hf x y)
  
Î -congruence : (fe : âˆ€ {U V} â†’ FunExt U V)
              â†’ âˆ€ {U V} (X : U Ì‡) (Y Y' : X â†’ V Ì‡)
              â†’ ((x : X) â†’ Y x â‰ƒ Y' x) â†’ Î  Y â‰ƒ Î  Y'
Î -congruence fe X Y Y' Ï† = (F , (G , FG) , (H , HF))
   where
    f : (x : X) â†’ Y x â†’ Y' x
    f x = prâ‚(Ï† x)
    g : (x : X) â†’ Y' x â†’ Y x
    g x =  prâ‚(prâ‚(prâ‚‚(Ï† x)))
    fg : (x : X) (y' : Y' x) â†’ f x (g x y') â‰¡ y' 
    fg x = prâ‚‚(prâ‚(prâ‚‚(Ï† x)))
    h : (x : X) â†’ Y' x â†’ Y x
    h x = prâ‚(prâ‚‚(prâ‚‚(Ï† x)))
    hf : (x : X) (y : Y x) â†’ h x (f x y) â‰¡ y  
    hf x = prâ‚‚(prâ‚‚(prâ‚‚(Ï† x)))
  
    F : ((x : X) â†’ Y x) â†’ ((x : X) â†’ Y' x)
    F = Î» z x â†’ prâ‚ (Ï† x) (z x)
    G : ((x : X) â†’ Y' x) â†’ (x : X) â†’ Y x 
    G u x = g x (u x)
    H : ((x : X) â†’ Y' x) â†’ (x : X) â†’ Y x 
    H u' x = h x (u' x)
  
    FG :  (w' : ((x : X) â†’ Y' x)) â†’ F(G w') â‰¡ w'
    FG w' = funext fe FG' 
     where
      FG' : (x : X) â†’ F(G w') x â‰¡ w' x
      FG' x = fg x (w' x)
  
    HF : (w : ((x : X) â†’ Y x)) â†’ H(F w) â‰¡ w
    HF w = funext fe GF' 
     where
      GF' : (x : X) â†’ H(F w) x â‰¡ w x
      GF' x = hf x (w x)
  
lemma[ğŸ™Ã—Yâ‰ƒY] : âˆ€ {U} {Y : U Ì‡} â†’ ğŸ™ Ã— Y â‰ƒ Y
lemma[ğŸ™Ã—Yâ‰ƒY] {U} {Y} = (f , (g , fg) , (g , gf))
  where 
    f : ğŸ™ Ã— Y â†’ Y
    f (* , y) = y
    g : Y â†’ ğŸ™ Ã— Y 
    g y = (* , y)
    fg : âˆ€ x â†’ f (g x) â‰¡ x 
    fg y = refl 
    gf : âˆ€ z â†’ g (f z) â‰¡ z
    gf (* , y) = refl
  
  
lemma[XÃ—Yâ‰ƒYÃ—X] : âˆ€ {U V} {X : U Ì‡} {Y : V Ì‡} â†’ X Ã— Y â‰ƒ Y Ã— X
lemma[XÃ—Yâ‰ƒYÃ—X] {U} {V} {X} {Y} = (f , (g , fg) , (g , gf))
   where 
    f : X Ã— Y â†’ Y Ã— X
    f (x , y) = (y , x)
    g : Y Ã— X â†’ X Ã— Y
    g (y , x) = (x , y)
    fg : âˆ€ z â†’ f (g z) â‰¡ z 
    fg z = refl 
    gf : âˆ€ t â†’ g (f t) â‰¡ t
    gf t = refl
  
lemma[YÃ—ğŸ™â‰ƒY] : âˆ€ {U} {Y : U Ì‡} â†’ Y Ã— ğŸ™ â‰ƒ Y
lemma[YÃ—ğŸ™â‰ƒY] {U} {Y} = â‰ƒ-trans {U} {U} {U} lemma[XÃ—Yâ‰ƒYÃ—X] lemma[ğŸ™Ã—Yâ‰ƒY] 

lemma[Xâ‰ƒX'â†’Yâ‰ƒY'â†’[XÃ—Y]â‰ƒ[X'Ã—Y']] : âˆ€ {U V W T} {X : U Ì‡} {X' : V Ì‡} {Y : W Ì‡} {Y' : T Ì‡}
                                  â†’ X â‰ƒ X' â†’ Y â‰ƒ Y' â†’ X Ã— Y â‰ƒ X' Ã— Y'
lemma[Xâ‰ƒX'â†’Yâ‰ƒY'â†’[XÃ—Y]â‰ƒ[X'Ã—Y']] {U} {V} {W} {T} {X} {X'} {Y} {Y'} (f , (g , fg) , (h , hf)) (f' , (g' , fg') , (h' , hf'))
   = (f'' , (g'' , fg'') , (h'' , hf''))
   where 
    f'' : X Ã— Y â†’ X' Ã— Y'
    f'' (x , y) = (f x , f' y)
    g'' : X' Ã— Y' â†’ X Ã— Y
    g'' (x' , y') = (g x' , g' y')
    h'' : X' Ã— Y' â†’ X Ã— Y
    h'' (x' , y') = (h x' , h' y')
    fg'' : âˆ€ z' â†’ f'' (g'' z') â‰¡ z' 
    fg''(x' , y') = apâ‚‚ _,_ lemmaâ‚€ lemmaâ‚ 
     where 
      lemmaâ‚€ : f(g x') â‰¡ x'
      lemmaâ‚€ = fg x' 
      lemmaâ‚ : f'(g' y') â‰¡ y'
      lemmaâ‚ = fg' y' 
    hf'' : âˆ€ z â†’ h'' (f'' z) â‰¡ z
    hf''(x' , y') = apâ‚‚ _,_ lemmaâ‚€ lemmaâ‚ 
      where  
       lemmaâ‚€ : h(f x') â‰¡ x'
       lemmaâ‚€ = hf x'
       lemmaâ‚ : h'(f' y') â‰¡ y'
       lemmaâ‚ = hf' y'
       
\end{code}
  
