Martin Escardo 2012.

See my paper "Infinite sets that satisfy the principle of
omniscience" for a discussion of the type â„•âˆ defined here. 
Essentially, â„•âˆ is â„• with an added point âˆ.

(Added December 2017. What we knew for a long time: The â„•âˆ is a
retract of the Cantor type â„• â†’ ğŸš. This required adding a number of
lemmas.)

\begin{code}

{-# OPTIONS --without-K --exact-split --safe #-}

module GenericConvergentSequence where

open import SpartanMLTT renaming (_â‰¤_ to _â‰¤â‚‚_) renaming (â‰¤-anti to â‰¤â‚‚-anti)
open import UF-Base
open import UF-Subsingletons
open import UF-Subsingletons-FunExt
open import UF-FunExt
open import UF-Embedding
open import UF-SetExamples
open import DiscreteAndSeparated
open import NaturalsOrder

funextâ‚€ : Uâ‚ Ì‡
funextâ‚€ = funext Uâ‚€ Uâ‚€

\end{code}

Definition (The generic convergent sequence).
We use u,v to range over â„•âˆ and Î±,Î² to range over â‚‚â„•:

\begin{code}

decreasing : (â„• â†’ ğŸš) â†’ Uâ‚€ Ì‡
decreasing Î± = (i : â„•) â†’ Î±(succ i) â‰¤â‚‚ Î± i 

decreasing-is-prop : funextâ‚€ â†’ (Î± : â„• â†’ ğŸš) â†’ is-prop(decreasing Î±)
decreasing-is-prop fe Î± = is-prop-exponential-ideal fe
                            (Î» i â†’ is-prop-exponential-ideal fe (Î» p â†’ ğŸš-is-set))

â„•âˆ : Uâ‚€ Ì‡
â„•âˆ = Î£ \(Î± : â„• â†’ ğŸš) â†’ decreasing Î±

decreasing-is-prop-old : funextâ‚€ â†’ {Î± : â„• â†’ ğŸš} â†’ is-prop(decreasing Î±)
decreasing-is-prop-old fe {Î±} p q = dfunext fe factâ‚‚
 where
  factâ‚€ : (i : â„•) (f g : Î±(succ i) â‰¡ â‚ â†’ Î± i â‰¡ â‚) â†’ f â‰¡ g
  factâ‚€ i f g = nfunext fe factâ‚
   where
    factâ‚ : (r : Î± (succ i) â‰¡ â‚) â†’ f r â‰¡ g r
    factâ‚ r = ğŸš-is-set (f r) (g r)
  factâ‚‚ : (i : â„•) â†’ p i â‰¡ q i
  factâ‚‚ i = factâ‚€ i (p i) (q i) 

incl : â„•âˆ â†’ (â„• â†’ ğŸš)
incl = prâ‚

incl-lc : funextâ‚€ â†’ left-cancellable incl
incl-lc fe = prâ‚-lc (decreasing-is-prop fe _)  

force-decreasing : (â„• â†’ ğŸš) â†’ (â„• â†’ ğŸš)
force-decreasing Î² 0 = Î² 0
force-decreasing Î² (succ i) = minğŸš (Î²(succ i)) (force-decreasing Î² i)

force-decreasing-is-decreasing : (Î² : â„• â†’ ğŸš) â†’ decreasing(force-decreasing Î²)
force-decreasing-is-decreasing Î² zero     = Lemma[minğŸšabâ‰¡â‚â†’bâ‰¡â‚] {Î² 1} {Î² zero}
force-decreasing-is-decreasing Î² (succ i) = Lemma[minabâ‰¤b] {Î² (succ (succ i))} {force-decreasing Î² (succ i)}

force-decreasing-unchanged : (Î± : â„• â†’ ğŸš) â†’ decreasing Î± â†’ force-decreasing Î± âˆ¼ Î±
force-decreasing-unchanged Î± d zero     = refl
force-decreasing-unchanged Î± d (succ i) = g
  where
    IH : force-decreasing Î± i â‰¡ Î± i
    IH = force-decreasing-unchanged Î± d i
    p : Î± (succ i) â‰¤â‚‚ Î± i
    p = d i
    h : minğŸš (Î± (succ i)) (Î± i) â‰¡ Î± (succ i)
    h = Lemma[aâ‰¤bâ†’minğŸšabâ‰¡a] p
    g' : minğŸš (Î± (succ i)) (force-decreasing Î± i) â‰¡ Î± (succ i)
    g' = transport (Î» b â†’ minğŸš (Î± (succ i)) b â‰¡ Î± (succ i)) (IH â»Â¹) h
    g : force-decreasing Î± (succ i) â‰¡ Î± (succ i)
    g = g'

lcni : (â„•  â†’ ğŸš) â†’ â„•âˆ
lcni Î² = force-decreasing Î² , force-decreasing-is-decreasing Î²

clni-incl : funextâ‚€ â†’ (x : â„•âˆ) â†’ lcni(incl x) â‰¡ x
clni-incl fe (Î± , d) = to-Î£-â‰¡'' (dfunext fe (force-decreasing-unchanged Î± d) , decreasing-is-prop fe Î± _ _)

force-decreasing-is-smaller : (Î² : â„• â†’ ğŸš) (i : â„•) â†’ force-decreasing Î² i â‰¤â‚‚ Î² i
force-decreasing-is-smaller Î² zero     p = p
force-decreasing-is-smaller Î² (succ i) p = Lemma[minğŸšabâ‰¡â‚â†’aâ‰¡â‚] p

force-decreasing-is-not-much-smaller : (Î² : â„• â†’ ğŸš) (n : â„•) â†’ force-decreasing Î² n â‰¡ â‚€ â†’ (Î£ \(m : â„•) â†’ Î² m â‰¡ â‚€)
force-decreasing-is-not-much-smaller Î² zero  p    = zero , p
force-decreasing-is-not-much-smaller Î² (succ n) p = f c
  where
    A = Î£ \(m : â„•) â†’ Î² m â‰¡ â‚€
    c : (Î² (succ n) â‰¡ â‚€) + (force-decreasing Î² n â‰¡ â‚€)
    c = lemma[minğŸšabâ‰¡â‚€] {Î² (succ n)} {force-decreasing Î² n} p
    f : (Î² (succ n) â‰¡ â‚€) + (force-decreasing Î² n â‰¡ â‚€) â†’ A
    f (inl q) = succ n , q
    f (inr r) = force-decreasing-is-not-much-smaller Î² n r

Cantor-separated : funextâ‚€ â†’ separated (â„• â†’ ğŸš)
Cantor-separated fe = separated-ideal fe (Î» _ â†’ ğŸš-is-separated)

â„•âˆ-separated : funextâ‚€ â†’ separated â„•âˆ
â„•âˆ-separated fe = subtype-of-separated-is-separated prâ‚ (incl-lc fe) (Cantor-separated fe)

â„•âˆ-is-set : funextâ‚€ â†’ is-set â„•âˆ
â„•âˆ-is-set fe = separated-is-set fe (â„•âˆ-separated fe)

open import TotallySeparated

â„•âˆ-totally-separated : funextâ‚€ â†’ totally-separated â„•âˆ
â„•âˆ-totally-separated fe {x} {y} Î± = g
 where
  p : â„• â†’ (â„•âˆ â†’ ğŸš)
  p i x = incl x i
  l : incl x â‰¡ incl y
  l = dfunext fe (Î» i â†’ Î± (p i))
  g : x â‰¡ y
  g = incl-lc fe l

Zero : â„•âˆ
Zero = ((Î» i â†’ â‚€) , Î» i â†’ id {Uâ‚€} {â‚€ â‰¡ â‚})

Succ : â„•âˆ â†’ â„•âˆ
Succ (Î± , d) = (Î±' , d')
 where 
  Î±' : â„• â†’ ğŸš
  Î±' 0 = â‚
  Î±'(succ n) = Î± n
  d' : decreasing Î±'
  d' 0 = Î» r â†’ refl
  d' (succ i) = d i

_âŠ‘_ : â„•âˆ â†’ â„• â†’ Uâ‚€ Ì‡
u âŠ‘ n = incl u n â‰¡ â‚€

_âŠ_ : â„• â†’ â„•âˆ â†’ Uâ‚€ Ì‡
n âŠ u = incl u n â‰¡ â‚

not-âŠ-is-âŠ’ : {m : â„•} {u : â„•âˆ} â†’ Â¬(m âŠ u) â†’ u âŠ‘ m
not-âŠ-is-âŠ’ f = Lemma[bâ‰¢â‚â†’bâ‰¡â‚€] f

not-âŠ‘-is-âŠ : {m : â„•} {u : â„•âˆ} â†’ Â¬(u âŠ‘ m) â†’ m âŠ u
not-âŠ‘-is-âŠ f = Lemma[bâ‰¢â‚€â†’bâ‰¡â‚] f

is-Zero : â„•âˆ â†’ Uâ‚€ Ì‡
is-Zero u = u âŠ‘ 0

positive : â„•âˆ â†’ Uâ‚€ Ì‡
positive u = 0 âŠ u

positivity : â„•âˆ â†’ ğŸš
positivity u = incl u 0 

is-Zero-Zero : is-Zero Zero
is-Zero-Zero = refl

Zero-not-Succ : {u : â„•âˆ} â†’ Zero â‰¢ Succ u
Zero-not-Succ {u} r = zero-is-not-one(ap positivity r)

âˆ : â„•âˆ
âˆ = ((Î» i â†’ â‚) , Î» i â†’ id {Uâ‚€} {â‚ â‰¡ â‚})

Succ-âˆ-is-âˆ : funextâ‚€ â†’ Succ âˆ â‰¡ âˆ
Succ-âˆ-is-âˆ fe = incl-lc fe (dfunext fe lemma) 
 where
   lemma : (i : â„•) â†’ incl(Succ âˆ) i â‰¡ incl âˆ i
   lemma 0 = refl
   lemma (succ i) = refl

unique-fixed-point-of-Succ : funextâ‚€ â†’ (u : â„•âˆ) â†’ u â‰¡ Succ u â†’ u â‰¡ âˆ
unique-fixed-point-of-Succ fe u r = incl-lc fe claim
 where
  fact : (i : â„•) â†’ incl u i â‰¡ incl(Succ u) i 
  fact i = ap (Î» w â†’ incl w i) r
  lemma : (i : â„•) â†’ incl u i â‰¡ â‚
  lemma 0 = fact 0
  lemma (succ i) = fact(succ i) âˆ™ lemma i
  claim : incl u â‰¡ incl âˆ
  claim = (dfunext fe lemma)

Pred : â„•âˆ â†’ â„•âˆ
Pred(Î± , d) = (Î± âˆ˜ succ , d âˆ˜ succ)

Pred-Zero-is-Zero : Pred Zero â‰¡ Zero
Pred-Zero-is-Zero = refl 

Pred-Succ-u-is-u : {u : â„•âˆ} â†’ Pred(Succ u) â‰¡ u
Pred-Succ-u-is-u {u} = refl

Pred-âˆ-is-âˆ : Pred âˆ â‰¡ âˆ
Pred-âˆ-is-âˆ = refl

Succ-lc : left-cancellable Succ
Succ-lc = ap Pred

under : â„• â†’ â„•âˆ
under 0 = Zero
under (succ n) = Succ(under n)

_â‰£_ : â„•âˆ â†’ â„• â†’ Uâ‚€ Ì‡
u â‰£ n = u â‰¡ under n

under-lc : left-cancellable under
under-lc {0} {0} r = refl
under-lc {0} {succ n} r = ğŸ˜-elim(Zero-not-Succ r)
under-lc {succ m} {0} r = ğŸ˜-elim(Zero-not-Succ (r â»Â¹))
under-lc {succ m} {succ n} r = ap succ (under-lc {m} {n} (Succ-lc r))

-- This should be proved as a consequence of a more general theorem
-- with essentially the same proof:
under-embedding : funextâ‚€ â†’ is-embedding under
under-embedding fe x (xâ‚€ , râ‚€) (xâ‚ , râ‚) = to-Î£-â‰¡'' (under-lc (râ‚€ âˆ™ râ‚ â»Â¹) , â„•âˆ-is-set fe _ _)

under-lc-refl : (k : â„•) â†’ under-lc refl â‰¡ refl {_} {â„•} {k}
under-lc-refl 0 = refl
under-lc-refl (succ k) = ap (ap succ) (under-lc-refl k)

under-diagonalâ‚€ : (n : â„•) â†’ under n âŠ‘ n
under-diagonalâ‚€ 0 = refl
under-diagonalâ‚€ (succ n) = under-diagonalâ‚€ n

under-diagonalâ‚ : (n : â„•) â†’ n âŠ under(succ n)
under-diagonalâ‚ 0 = refl
under-diagonalâ‚ (succ n) = under-diagonalâ‚ n
 
is-Zero-equal-Zero : funextâ‚€ â†’ {u : â„•âˆ} â†’ is-Zero u â†’ u â‰¡ Zero
is-Zero-equal-Zero fe {u} base = incl-lc fe (dfunext fe lemma)
 where
  lemma : (i : â„•) â†’ incl u i â‰¡ incl Zero i
  lemma 0 = base
  lemma (succ i) = Lemma[[aâ‰¡â‚â†’bâ‰¡â‚]â†’bâ‰¡â‚€â†’aâ‰¡â‚€] (prâ‚‚ u i) (lemma i)

not-Zero-is-Succ : funextâ‚€ â†’ {u : â„•âˆ} â†’ u â‰¢ Zero â†’ u â‰¡ Succ(Pred u)
not-Zero-is-Succ fe {u} f = incl-lc fe (dfunext fe lemma)
 where
  lemma : (i : â„•) â†’ incl u i â‰¡ incl(Succ(Pred u)) i 
  lemma 0 = Lemma[bâ‰¢â‚€â†’bâ‰¡â‚] (f âˆ˜ is-Zero-equal-Zero fe)
  lemma (succ i) = refl

positive-is-not-Zero : {u : â„•âˆ} â†’ positive u â†’ u â‰¢ Zero
positive-is-not-Zero {u} r s = lemma r
 where
  lemma : Â¬(positive u)
  lemma = Lemma[bâ‰¡â‚€â†’bâ‰¢â‚](ap positivity s)

positive-equal-Succ : funextâ‚€ â†’ {u : â„•âˆ} â†’ positive u â†’ u â‰¡ Succ(Pred u)
positive-equal-Succ fe r = not-Zero-is-Succ fe (positive-is-not-Zero r)

Succ-criterion : funextâ‚€ â†’ {u : â„•âˆ} {n : â„•} â†’ n âŠ u â†’ u âŠ‘ succ n â†’ u â‰¡ Succ(under n)
Succ-criterion fe {u} {n} r s = incl-lc fe claim
 where
  lemma : (u : â„•âˆ) (n : â„•) â†’ n âŠ u â†’ u âŠ‘ succ n 
        â†’ (i : â„•) â†’ incl u i â‰¡ incl (Succ(under n)) i
  lemma u 0 r s 0 = r
  lemma u 0 r s (succ i) = lemmaâ‚€ i
     where 
      lemmaâ‚€ : (i : â„•) â†’ u âŠ‘ succ i
      lemmaâ‚€ 0 = s
      lemmaâ‚€ (succ i) = Lemma[[aâ‰¡â‚â†’bâ‰¡â‚]â†’bâ‰¡â‚€â†’aâ‰¡â‚€] (prâ‚‚ u (succ i)) (lemmaâ‚€ i)
  lemma u (succ n) r s 0 = lemmaâ‚ (succ n) r
     where 
      lemmaâ‚ : (n : â„•) â†’ n âŠ u â†’ positive u
      lemmaâ‚ 0 t = t
      lemmaâ‚ (succ n) t = lemmaâ‚ n (prâ‚‚ u n t)
  lemma u (succ n) r s (succ i) = lemma (Pred u) n r s i
  claim : incl u â‰¡ incl (Succ (under n))
  claim = dfunext fe (lemma u n r s)


âˆ-is-not-â„• : (n : â„•) â†’ âˆ â‰¢ under n
âˆ-is-not-â„• n s = zero-is-not-one ((ap (Î» w â†’ incl w n) s âˆ™ under-diagonalâ‚€ n)â»Â¹)

not-â„•-is-âˆ : funextâ‚€ â†’ {u : â„•âˆ} â†’ ((n : â„•) â†’ u â‰¢ under n) â†’ u â‰¡ âˆ
not-â„•-is-âˆ fe {u} f = incl-lc fe (dfunext fe lemma) 
 where
  lemma : (n : â„•) â†’ n âŠ u
  lemma 0 = Lemma[bâ‰¢â‚€â†’bâ‰¡â‚](Î» r â†’ f 0 (is-Zero-equal-Zero fe r)) 
  lemma (succ n) = Lemma[bâ‰¢â‚€â†’bâ‰¡â‚](Î» r â†’ f(succ n)(Succ-criterion fe (lemma n) r)) 

â„•âˆ-density : funextâ‚€ â†’ {p : â„•âˆ â†’ ğŸš} â†’ ((n : â„•) â†’ p(under n) â‰¡ â‚) â†’ p âˆ â‰¡ â‚ â†’ (u : â„•âˆ) â†’ p u â‰¡ â‚
â„•âˆ-density fe {p} f r u = Lemma[bâ‰¢â‚€â†’bâ‰¡â‚] lemma
 where 
  claim : p u â‰¡ â‚€ â†’ (n : â„•) â†’ u â‰¢ under n
  claim g n = contrapositive (Î» s â†’ ap p s âˆ™ f n) (Lemma[bâ‰¡â‚€â†’bâ‰¢â‚] g)

  claim-âˆ : p u â‰¡ â‚€ â†’ u â‰¢ âˆ
  claim-âˆ = (contrapositive (Î» s â†’ ap p s âˆ™ r)) âˆ˜ Lemma[bâ‰¡â‚€â†’bâ‰¢â‚]

  lemma : p u â‰¢ â‚€
  lemma t = claim-âˆ t (not-â„•-is-âˆ fe (claim t)) 

underğŸ™ : â„• + ğŸ™ â†’ â„•âˆ
underğŸ™ = cases under (Î» _ â†’ âˆ)

underğŸ™-embedding : funextâ‚€ â†’ is-embedding underğŸ™
underğŸ™-embedding fe = disjoint-cases-embedding under (Î» _ â†’ âˆ) (under-embedding fe) g d
 where
  g : is-embedding (Î» _ â†’ âˆ)
  g x (* , p) (* , q) = ap (Î» p â†’ * , p) (â„•âˆ-is-set fe p q)
  d : (n : â„•) (y : ğŸ™) â†’ under n â‰¢ âˆ
  d n _ p = âˆ-is-not-â„• n (p â»Â¹)

underğŸ™-dense : funextâ‚€ â†’ Â¬ Î£ \(u : â„•âˆ) â†’ (x : â„• + ğŸ™) â†’ u â‰¢ underğŸ™ x
underğŸ™-dense fe (u , f) = g (not-â„•-is-âˆ fe h)
 where
  g : u â‰¢ âˆ
  g = f (inr *)
  h : (n : â„•) â†’ u â‰¢ under n 
  h n = f (inl n)

\end{code}

There should be a better proof of the following. The idea is simple:
by the above development, u = under 0 if and only if incl u 0 â‰¡ 0, and
u â‰¡ under(n+1) if and only if n âŠ u âŠ‘ n+1.

\begin{code}

finite-isolated : funextâ‚€ â†’ (u : â„•âˆ) (n : â„•) â†’ (u â‰¡ under n) + (u â‰¢ under n)
finite-isolated fe u 0 = two-equality-cases lemmaâ‚€ lemmaâ‚
 where 
  lemmaâ‚€ : is-Zero u â†’ (u â‰¡ Zero) + (u â‰¢ Zero)
  lemmaâ‚€ r = inl(is-Zero-equal-Zero fe r)
  lemmaâ‚ : positive u â†’ (u â‰¡ Zero) + (u â‰¢ Zero)
  lemmaâ‚ r = inr(contrapositive fact (Lemma[bâ‰¡â‚â†’bâ‰¢â‚€] r))
    where fact : u â‰¡ Zero â†’ is-Zero u
          fact r = ap (Î» u â†’ incl u 0) r
finite-isolated fe u (succ n) = two-equality-cases lemmaâ‚€ lemmaâ‚
 where
  lemmaâ‚€ :  u âŠ‘ n â†’ (u â‰¡ under(succ n)) + (u â‰¢ under(succ n))
  lemmaâ‚€ r = inr(contrapositive lemma (Lemma[bâ‰¡â‚€â†’bâ‰¢â‚] r))
   where
    lemma : u â‰¡ under(succ n) â†’ n âŠ u
    lemma r = ap (Î» v â†’ incl v n) r âˆ™ under-diagonalâ‚ n
  lemmaâ‚ :  n âŠ u â†’ (u â‰¡ under(succ n)) + (u â‰¢ under(succ n))
  lemmaâ‚ r = two-equality-cases lemmaâ‚â‚€ lemmaâ‚â‚
   where
    lemmaâ‚â‚€ :  u âŠ‘ succ n â†’ (u â‰¡ under(succ n)) + (u â‰¢ under(succ n))
    lemmaâ‚â‚€ s = inl(Succ-criterion fe r s)
    lemmaâ‚â‚ :  succ n âŠ u â†’ (u â‰¡ under(succ n)) + (u â‰¢ under(succ n))
    lemmaâ‚â‚ s = inr (contrapositive lemma (Lemma[bâ‰¡â‚â†’bâ‰¢â‚€] s))
     where
      lemma : u â‰¡ under(succ n) â†’ u âŠ‘ succ n
      lemma r = ap (Î» v â†’ incl v (succ n)) r âˆ™ under-diagonalâ‚€(succ n)

under-lemma : funextâ‚€ â†’ (u : â„•âˆ) (n : â„•) â†’ u âŠ‘ n â†’ Î£ \(m : â„•) â†’ (m â‰¤ n) Ã— (u â‰¡ under m)
under-lemma fe u zero p     = zero , â‰¤-refl zero , is-Zero-equal-Zero fe p
under-lemma fe u (succ n) p = g (ğŸš-discrete (incl u n) â‚€)
 where
  IH : u âŠ‘ n â†’ Î£ \(m : â„•) â†’ (m â‰¤ n) Ã— (u â‰¡ under m)
  IH = under-lemma fe u n
  g :  decidable(u âŠ‘ n) â†’ Î£ \(m : â„•) â†’ (m â‰¤ succ n) Ã— (u â‰¡ under m)
  g (inl q) = prâ‚(IH q) , â‰¤-trans (prâ‚(IH q)) n (succ n) (prâ‚(prâ‚‚(IH q))) (â‰¤-succ n) , prâ‚‚(prâ‚‚(IH q))
  g (inr Ï†) = succ n , â‰¤-refl n , s
    where
      q : n âŠ u
      q = Lemma[bâ‰¢â‚€â†’bâ‰¡â‚] Ï†
      s : u â‰¡ Succ (under n)
      s = Succ-criterion fe {u} {n} q p

\end{code}

Order on â„•âˆ:

\begin{code}

_â‰¼_ : â„•âˆ â†’ â„•âˆ â†’ Uâ‚€ Ì‡
u â‰¼ v = (n : â„•) â†’ n âŠ u â†’ n âŠ v

âˆ-greatest : (u : â„•âˆ) â†’ u â‰¼ âˆ
âˆ-greatest u = Î» n _ â†’ refl

max : â„•âˆ â†’ â„•âˆ â†’ â„•âˆ
max (Î± , r) (Î² , s) = (Î» i â†’ maxğŸš (Î± i) (Î² i)) , t
 where
  t : decreasing (Î» i â†’ maxğŸš (Î± i) (Î² i))
  t i p = maxğŸš-lemma-converse (Î± i) (Î² i) (f (maxğŸš-lemma(Î±(succ i)) (Î²(succ i)) p))
    where
     f : (Î±(succ i) â‰¡ â‚) + (Î²(succ i) â‰¡ â‚) â†’ (Î± i â‰¡ â‚) + (Î² i â‰¡ â‚)
     f (inl p) = inl (r i p)
     f (inr p) = inr (s i p)

\end{code}

More lemmas about order should be added, but I will do this on demand
as the need arises.

\begin{code}

âˆ-âŠ-maximal : (n : â„•) â†’ n âŠ âˆ
âˆ-âŠ-maximal n = refl

_â‰º_ : â„•âˆ â†’ â„•âˆ â†’ Uâ‚€ Ì‡
u â‰º v = Î£ \(n : â„•) â†’ (u â‰¡ under n) Ã— n âŠ v

â‰º-prop-valued : funextâ‚€ â†’ (u v : â„•âˆ) â†’ is-prop (u â‰º v)
â‰º-prop-valued fe u v (n , r , a) (m , s , b) =
  to-Î£-â‰¡'' (under-lc (r â»Â¹ âˆ™ s) , to-Î£-â‰¡'' (â„•âˆ-is-set fe _ _ , ğŸš-is-set _ _))

âŠ-gives-â‰º : (n : â„•) (u : â„•âˆ) â†’ n âŠ u â†’ under n â‰º u
âŠ-gives-â‰º n u a = n , refl , a

â‰º-gives-âŠ : (n : â„•) (u : â„•âˆ) â†’ under n â‰º u â†’ n âŠ u
â‰º-gives-âŠ n u (m , r , a) = back-transport (Î» k â†’ k âŠ u) (under-lc r) a

âˆ-maximal : (n : â„•) â†’ under n â‰º âˆ
âˆ-maximal n = n , refl , âˆ-âŠ-maximal n

âŠ-reflect : (m n : â„•) â†’  m âŠ under n â†’ m < n
âŠ-reflect zero zero ()
âŠ-reflect zero (succ n) l = zero-minimal n
âŠ-reflect (succ m) zero ()
âŠ-reflect (succ m) (succ n) l = âŠ-reflect m n l

âŠ-back : (u : â„•âˆ) (n : â„•) â†’ succ n âŠ u â†’ n âŠ u
âŠ-back = prâ‚‚

âŠ-trans'' : (u : â„•âˆ) (n : â„•) â†’ (m : â„•) â†’ m â‰¤ n â†’ n âŠ u â†’ m âŠ u
âŠ-trans'' u = regress (Î» n â†’ n âŠ u) (âŠ-back u) 

âŠ-trans' : (u : â„•âˆ) (n : â„•) â†’ (m : â„•) â†’ m < n â†’ n âŠ u â†’ m âŠ u
âŠ-trans' u n m l = âŠ-trans'' u n m (â‰¤-trans m (succ m) n (â‰¤-succ m) l)

âŠ-trans : (m n : â„•) (u : â„•âˆ) â†’ m âŠ under n â†’ n âŠ u â†’ m âŠ u
âŠ-trans m n u a = âŠ-trans' u n m (âŠ-reflect m n a)

â‰º-trans : (u v w : â„•âˆ) â†’ u â‰º v â†’ v â‰º w â†’ u â‰º w
â‰º-trans u v w (m , r , a) (n , s , b) = m , r , âŠ-trans m n w (transport (Î» t â†’ m âŠ t) s a) b

open import Ordinals hiding (_â‰¤_) hiding (â‰¤-refl)

â‰º-well-foundedâ‚‚ : funextâ‚€ â†’ is-well-foundedâ‚‚ _â‰º_
â‰º-well-foundedâ‚‚ fe p Ï† = â„•âˆ-density fe a b
 where
  Î³ : (n : â„•) â†’ ((m : â„•) â†’ m < n â†’ p (under m) â‰¡ â‚) â†’ p (under n) â‰¡ â‚
  Î³ n g = Ï† (under n) h
   where
    h : (u : â„•âˆ) â†’ u â‰º under n â†’ p u â‰¡ â‚
    h u (m , r , l) = back-transport (Î» v â†’ p v â‰¡ â‚) r (g m (âŠ-reflect m n l))
  a : (n : â„•) â†’ p(under n) â‰¡ â‚
  a = course-of-values-induction (Î» n â†’ p(under n) â‰¡ â‚) Î³
  f : (u : â„•âˆ) â†’ u â‰º âˆ â†’ p u â‰¡ â‚
  f u (n , r , l) = back-transport (Î» v â†’ p v â‰¡ â‚) r (a n)
  b : p âˆ â‰¡ â‚
  b = Ï† âˆ f

â‰º-extensional : funextâ‚€ â†’ is-extensional _â‰º_
â‰º-extensional fe u v l m = Î³
 where
  f : (i : â„•) â†’ i âŠ u â†’ i âŠ v
  f i a = â‰º-gives-âŠ i v (l (under i) (âŠ-gives-â‰º i u a))
  g : (i : â„•) â†’ i âŠ v â†’ i âŠ u
  g i a = â‰º-gives-âŠ i u (m (under i) (âŠ-gives-â‰º i v a))
  h : (i : â„•) â†’ incl u i â‰¡ incl v i
  h i = â‰¤â‚‚-anti (f i) (g i)
  Î³ : u â‰¡ v
  Î³ = incl-lc fe (dfunext fe h)

â„•âˆ-ordinalâ‚‚ : funextâ‚€ â†’ is-ordinalâ‚‚ _â‰º_
â„•âˆ-ordinalâ‚‚ fe = (â‰º-well-foundedâ‚‚ fe) , (â‰º-extensional fe) , â‰º-trans

â‰º-cotransitive : funextâ‚€ â†’ cotransitive _â‰º_
â‰º-cotransitive fe u v w (n , r , a) = g (ğŸš-discrete (incl w n) â‚)
 where
  g : decidable(n âŠ w) â†’ (u â‰º w) + (w â‰º v)
  g (inl a) = inl (n , r , a)
  g (inr f) = inr (m , s , âŠ-trans'' v n m l a)
   where
    b : w âŠ‘ n
    b = not-âŠ-is-âŠ’ {n} {w} f
    Ïƒ : Î£ \(m : â„•) â†’ (m â‰¤ n) Ã— (w â‰¡ under m)
    Ïƒ = under-lemma fe w n b
    m : â„•
    m = prâ‚ Ïƒ
    l : m â‰¤ n
    l = prâ‚(prâ‚‚ Ïƒ)
    s : w â‰¡ under m
    s = prâ‚‚(prâ‚‚ Ïƒ)

\end{code}

precedences:

\begin{code}

infix  30 _âŠ_
infix  30 _â‰º_

\end{code}
