Andrew Sneap - 26th November 2021

In this file I define absolute values of integers and some properties of abs, along with positive and negative properties of integers.

\begin{code}

{-# OPTIONS --without-K --exact-split --safe #-}

open import SpartanMLTT renaming (_+_ to _âˆ”_) --TypeTopology

open import DiscreteAndSeparated -- TypeTopology
open import NaturalNumbers-Properties --TypeTopology
open import UF-Miscelanea -- TypeTopology
open import UF-Subsingletons --TypeTopology
open import Unit-Properties -- TypeTopology

open import NaturalsMultiplication renaming (_*_ to _â„•*_)
open import IntegersMultiplication
open import IntegersNegation
open import IntegersAddition
open import IntegersB

module IntegersAbs where

abs : â„¤ â†’ â„•
abs (pos x)     = x
abs (negsucc x) = succ x

absâ„¤ : â„¤ â†’ â„¤
absâ„¤ (pos x)     = pos x
absâ„¤ (negsucc x) = pos (succ x)

pos-lc : {x y : â„•} â†’ pos x â‰¡ pos y â†’ x â‰¡ y
pos-lc = ap abs

negsucc-lc : {x y : â„•} â†’ negsucc x â‰¡ negsucc y â†’ x â‰¡ y
negsucc-lc {x} {y} p = succ-lc (ap abs p)

positive : â„¤ â†’ ğ“¤â‚€ Ì‡
positive (pos x)     = ğŸ™
positive (negsucc x) = ğŸ˜

negative : â„¤ â†’ ğ“¤â‚€ Ì‡
negative (pos x)     = ğŸ˜
negative (negsucc x) = ğŸ™

is-zero : â„¤ â†’ ğ“¤â‚€ Ì‡
is-zero (pos 0)        = ğŸ™
is-zero (pos (succ x)) = ğŸ˜
is-zero (negsucc x)    = ğŸ˜

not-zero : â„¤ â†’ ğ“¤â‚€ Ì‡
not-zero z = Â¬ (is-zero z)

greater-than-zero : â„¤ â†’ ğ“¤â‚€ Ì‡
greater-than-zero (pos 0)        = ğŸ˜
greater-than-zero (pos (succ z)) = ğŸ™
greater-than-zero (negsucc z)    = ğŸ˜

pos-not-negative : {x y : â„•} â†’ pos x â‰¢ negsucc y
pos-not-negative p = ğŸ™-is-not-ğŸ˜ (ap positive p)

neg-not-positive : {x y : â„•} â†’ negsucc x â‰¢ pos y
neg-not-positive p = pos-not-negative (p â»Â¹)

pos-int-not-zero : (x : â„•) â†’ pos (succ x) â‰¢ pos 0
pos-int-not-zero x p = positive-not-zero x (pos-lc p)

neg-int-not-zero : (x : â„•) â†’ negsucc x â‰¢ pos 0
neg-int-not-zero x p = positive-not-zero x (ap abs p)

â„¤-is-discrete : is-discrete â„¤
â„¤-is-discrete (pos x) (pos y) = f (â„•-is-discrete x y)
  where
    f : (x â‰¡ y) âˆ” Â¬ (x â‰¡ y) â†’ (pos x â‰¡ pos y) âˆ” Â¬ (pos x â‰¡ pos y)
    f (inl z) = inl (ap pos z)
    f (inr z) = inr (Î» k â†’ z (pos-lc k))
â„¤-is-discrete (pos x)     (negsucc y) = inr pos-not-negative
â„¤-is-discrete (negsucc x) (pos y)     = inr neg-not-positive
â„¤-is-discrete (negsucc x) (negsucc y) = f (â„•-is-discrete x y)
  where
    f : (x â‰¡ y) âˆ” Â¬ (x â‰¡ y) â†’ decidable (negsucc x â‰¡ negsucc y)
    f (inl z) = inl (ap negsucc z)
    f (inr z) = inr (Î» k â†’ z (negsucc-lc k) )

â„¤-is-set : is-set â„¤
â„¤-is-set = discrete-types-are-sets â„¤-is-discrete

abs-removes-neg-sign : (x : â„¤) â†’ abs x â‰¡ abs (- x)
abs-removes-neg-sign (pos zero)     = refl
abs-removes-neg-sign (pos (succ x)) = refl
abs-removes-neg-sign (negsucc x)    = refl

absâ„¤-removes-neg-sign : (x : â„¤) â†’ absâ„¤ x â‰¡ absâ„¤ (- x)
absâ„¤-removes-neg-sign (pos zero)     = refl
absâ„¤-removes-neg-sign (pos (succ x)) = refl
absâ„¤-removes-neg-sign (negsucc x)    = refl

abs-over-mult : (a b : â„¤) â†’ abs (a * b) â‰¡ abs a â„•* abs b
abs-over-mult (pos x) (pos b) = I
 where
  I : abs (pos x * pos b) â‰¡ abs (pos x) â„•* abs (pos b)
  I = abs (pos x * pos b)        â‰¡âŸ¨ ap abs (pos-multiplication-equiv-to-â„• x b) âŸ©
      abs (pos (x â„•* b))         â‰¡âŸ¨ refl âŸ©
      abs (pos x) â„•* abs (pos b) âˆ
abs-over-mult (pos zero) (negsucc b) = I
 where
  I : abs (pos zero * negsucc b) â‰¡ abs (pos zero) â„•* abs (negsucc b)
  I = abs (pos zero * negsucc b) â‰¡âŸ¨ ap abs (â„¤-zero-left-is-zero (negsucc b)) âŸ©
      abs (pos 0)                â‰¡âŸ¨ zero-left-is-zero (abs (negsucc b)) â»Â¹ âŸ©
      abs (pos zero) â„•* abs (negsucc b) âˆ
abs-over-mult (pos (succ x)) (negsucc b) = I
 where
  I : abs (pos (succ x) * negsucc b) â‰¡ abs (pos (succ x)) â„•* abs (negsucc b)
  I = abs (pos (succ x) * negsucc b)           â‰¡âŸ¨ ap abs (subtraction-dist-over-mult (pos (succ x)) (pos (succ b))) âŸ©
      abs (- ((pos (succ x) * pos (succ b))))  â‰¡âŸ¨ ap (Î» z â†’ (abs (- z))) (pos-multiplication-equiv-to-â„• (succ x) (succ b)) âŸ©
      abs (- pos (succ x â„•* succ b))           â‰¡âŸ¨ abs-removes-neg-sign ( pos (succ x â„•* succ b)) â»Â¹ âŸ©
      abs (pos (succ x â„•* succ b))             â‰¡âŸ¨ refl âŸ©
      succ x â„•* succ b                         â‰¡âŸ¨ refl âŸ©
      abs (pos (succ x)) â„•* abs (negsucc b)    âˆ
abs-over-mult (negsucc x) (pos b) = I
 where
  I : abs (negsucc x * pos b) â‰¡ abs (negsucc x) â„•* abs (pos b)
  I = abs (negsucc x * pos b)        â‰¡âŸ¨ ap abs (subtraction-dist-over-mult' (pos (succ x)) (pos b)) âŸ©
      abs (- pos (succ x) * pos b)   â‰¡âŸ¨ ap (Î» z â†’ abs (- z)) (pos-multiplication-equiv-to-â„• (succ x) b) âŸ©
      abs (- pos (succ x â„•* b))      â‰¡âŸ¨ abs-removes-neg-sign (pos (succ x â„•* b)) â»Â¹ âŸ©
      (succ x) â„•* b                  â‰¡âŸ¨ refl âŸ©
      abs (negsucc x) â„•* abs (pos b) âˆ
abs-over-mult (negsucc x) (negsucc b) = I
 where
  I : abs (negsucc x * negsucc b) â‰¡ abs (negsucc x) â„•* abs (negsucc b)
  I = abs (negsucc x * negsucc b)               â‰¡âŸ¨ ap abs (subtraction-dist-over-mult (negsucc x) (pos (succ b))) âŸ©
      abs (- negsucc x * pos (succ b) )         â‰¡âŸ¨ ap (Î» z â†’ abs (- z)) (subtraction-dist-over-mult' (pos (succ x)) (pos (succ b))) âŸ©
      abs (- (- pos (succ x) * pos (succ b)))   â‰¡âŸ¨ ap abs (minus-minus-is-plus (pos (succ x) * pos (succ b))) âŸ©
      abs (pos (succ x) * pos (succ b))         â‰¡âŸ¨ ap abs (pos-multiplication-equiv-to-â„• (succ x) (succ b)) âŸ©
      (succ x) â„•* (succ b)                      â‰¡âŸ¨ refl âŸ©
      abs (negsucc x) â„•* abs (negsucc b)       âˆ

pos-abs-is-equal : (x : â„•) â†’ absâ„¤ (pos x) â‰¡ pos x
pos-abs-is-equal x = refl

abs-over-mult' : (x y : â„¤) â†’ absâ„¤ (x * y) â‰¡ absâ„¤ x * absâ„¤ y
abs-over-mult' (pos x) (pos y) = I
 where
  I : absâ„¤ (pos x * pos y) â‰¡ absâ„¤ (pos x) * absâ„¤ (pos y)
  I = absâ„¤ (pos x * pos y) â‰¡âŸ¨ ap absâ„¤ (pos-multiplication-equiv-to-â„• x y) âŸ©
      absâ„¤ (pos (x â„•* y))  â‰¡âŸ¨ by-definition âŸ©
      pos (x â„•* y)         â‰¡âŸ¨ pos-multiplication-equiv-to-â„• x y â»Â¹ âŸ©
      pos x * pos y        â‰¡âŸ¨ by-definition âŸ©
      absâ„¤ (pos x) * absâ„¤ (pos y) âˆ
abs-over-mult' (pos x) (negsucc y) = I
 where
  I : absâ„¤ (pos x * negsucc y) â‰¡ absâ„¤ (pos x) * absâ„¤ (negsucc y)
  I = absâ„¤ (pos x * negsucc y)        â‰¡âŸ¨ ap absâ„¤ (subtraction-dist-over-mult (pos x) (pos (succ y))) âŸ©
      absâ„¤ (- pos x * pos (succ y))   â‰¡âŸ¨ ap (Î» z â†’ absâ„¤ (- z)) (pos-multiplication-equiv-to-â„• x (succ y)) âŸ©
      absâ„¤ (- pos (x â„•* succ y))      â‰¡âŸ¨ absâ„¤-removes-neg-sign (pos (x â„•* succ y)) â»Â¹ âŸ©
      absâ„¤ (pos (x â„•* succ y))        â‰¡âŸ¨ by-definition âŸ©
      pos (x â„•* succ y)               â‰¡âŸ¨ pos-multiplication-equiv-to-â„• x (succ y) â»Â¹ âŸ©
      pos x * pos (succ y)            â‰¡âŸ¨ by-definition âŸ©
      absâ„¤ (pos x) * absâ„¤ (negsucc y) âˆ
abs-over-mult' (negsucc x) (pos y) = I
 where
  I : absâ„¤ (negsucc x * pos y) â‰¡ absâ„¤ (negsucc x) * absâ„¤ (pos y)
  I = absâ„¤ (negsucc x * pos y)      â‰¡âŸ¨ ap absâ„¤ (â„¤*-comm (negsucc x) (pos y)) âŸ©
      absâ„¤ (pos y * negsucc x)      â‰¡âŸ¨ ap absâ„¤ (subtraction-dist-over-mult (pos y) (pos (succ x))) âŸ©
      absâ„¤ (- pos y * pos (succ x)) â‰¡âŸ¨ ap (Î» z â†’ absâ„¤ (- z)) (pos-multiplication-equiv-to-â„• y (succ x)) âŸ©
      absâ„¤ (- pos (y â„•* succ x))    â‰¡âŸ¨ absâ„¤-removes-neg-sign (pos (y â„•* succ x)) â»Â¹ âŸ©
      absâ„¤ (pos (y â„•* succ x))      â‰¡âŸ¨ by-definition âŸ©
      pos (y â„•* succ x)             â‰¡âŸ¨ pos-multiplication-equiv-to-â„• y (succ x) â»Â¹ âŸ©
      pos y * pos (succ x)          â‰¡âŸ¨ â„¤*-comm (pos y) (pos (succ x)) âŸ©
      pos (succ x) * pos y          â‰¡âŸ¨ by-definition âŸ© 
      absâ„¤ (negsucc x) * absâ„¤ (pos y) âˆ
abs-over-mult' (negsucc x) (negsucc y) = I
 where
  I : absâ„¤ (negsucc x * negsucc y) â‰¡ absâ„¤ (negsucc x) * absâ„¤ (negsucc y)
  I = absâ„¤ (negsucc x * negsucc y)        â‰¡âŸ¨ ap absâ„¤ (minus-times-minus-is-positive (pos (succ x)) (pos (succ y))) âŸ©
      absâ„¤ (pos (succ x) * pos (succ y))  â‰¡âŸ¨ ap absâ„¤ (pos-multiplication-equiv-to-â„• (succ x) (succ y)) âŸ©
      absâ„¤ (pos (succ x â„•* succ y))       â‰¡âŸ¨ by-definition âŸ©
      pos (succ x â„•* succ y)              â‰¡âŸ¨ pos-multiplication-equiv-to-â„• (succ x) (succ y) â»Â¹ âŸ©
      pos (succ x) * pos (succ y)         â‰¡âŸ¨ by-definition âŸ©
      absâ„¤ (negsucc x) * absâ„¤ (negsucc y) âˆ

succâ„¤-no-fp : (x : â„¤) â†’ Â¬ (x â‰¡ succâ„¤ x)
succâ„¤-no-fp (pos x) e = succ-no-fp x (pos-lc e)
succâ„¤-no-fp (negsucc zero) e = pos-not-negative (e â»Â¹)
succâ„¤-no-fp (negsucc (succ x)) e = succ-no-fp x (negsucc-lc (e â»Â¹))

greater-than-zero-succâ„¤ : (x : â„¤) â†’ greater-than-zero x â†’ greater-than-zero (succâ„¤ x)
greater-than-zero-succâ„¤ (pos 0)        g = ğŸ˜-elim g
greater-than-zero-succâ„¤ (pos (succ x)) g = g
greater-than-zero-succâ„¤ (negsucc x)    g = ğŸ˜-elim g

gtzâ‚€ : (x : â„¤) â†’ (y : â„•) â†’ greater-than-zero x â†’ greater-than-zero (pos y) â†’ greater-than-zero (x + (pos y))
gtzâ‚€ x = induction base step
 where
  base : greater-than-zero x
       â†’ greater-than-zero (pos 0)
       â†’ greater-than-zero (x + pos 0)
  base l r = ğŸ˜-elim r

  step : (k : â„•)
       â†’ (greater-than-zero x â†’ greater-than-zero (pos k) â†’ greater-than-zero (x + pos k))
       â†’ greater-than-zero x
       â†’ greater-than-zero (pos (succ k))
       â†’ greater-than-zero (x + pos (succ k))
  step 0        IH l r = greater-than-zero-succâ„¤ x l
  step (succ k) IH l r = greater-than-zero-succâ„¤ (x + pos (succ k)) (IH l r)

greater-than-zero-trans : (x y : â„¤) â†’ greater-than-zero x â†’ greater-than-zero y â†’ greater-than-zero (x + y)
greater-than-zero-trans x (pos y)         = gtzâ‚€ x y
greater-than-zero-trans x (negsucc y) l r = ğŸ˜-elim r

gtzmtâ‚€ : (x : â„¤) â†’ (y : â„•) â†’ greater-than-zero x â†’ greater-than-zero (pos y) â†’ greater-than-zero (x * pos y)
gtzmtâ‚€ x = induction base step
 where
  base : greater-than-zero x â†’ greater-than-zero (pos 0) â†’ greater-than-zero (x * pos 0)
  base l r = ğŸ˜-elim r

  step : (k : â„•)
       â†’ (greater-than-zero x â†’ greater-than-zero (pos k) â†’ greater-than-zero (x * pos k))
       â†’ greater-than-zero x
       â†’ greater-than-zero (pos (succ k))
       â†’ greater-than-zero (x * pos (succ k))
  step zero IH l r = l
  step (succ k) IH l r = greater-than-zero-trans x (x * pos (succ k)) l (IH l r)

greater-than-zero-mult-trans : (x y : â„¤) â†’ greater-than-zero x â†’ greater-than-zero y â†’ greater-than-zero (x * y)
greater-than-zero-mult-trans x (negsucc y) l r = ğŸ˜-elim r
greater-than-zero-mult-trans x (pos y)     l r = gtzmtâ‚€ x y l r


{-
â„¤-not-equal-to-succ : (x : â„¤) â†’ Â¬ (x â‰¡ succâ„¤ x)
â„¤-not-equal-to-succ = â„¤-induction base stepâ‚ stepâ‚‚
 where
  base : Â¬ (pos 0 â‰¡ succâ„¤ (pos 0))
  base e = pos-int-not-zero 0 (e â»Â¹)
  stepâ‚ : (k : â„¤) â†’ Â¬ (k â‰¡ succâ„¤ k) â†’ Â¬ (succâ„¤ k â‰¡ succâ„¤ (succâ„¤ k))
  stepâ‚ k IH e = IH II
   where
    I : predâ„¤ (succâ„¤ k) â‰¡ predâ„¤ (succâ„¤ (succâ„¤ k))
    I = ap predâ„¤ e
    II : k â‰¡ succâ„¤ k
    II = k                       â‰¡âŸ¨ predsuccâ„¤ k â»Â¹ âŸ©
         predâ„¤ (succâ„¤ k)         â‰¡âŸ¨ I âŸ©
         predâ„¤ (succâ„¤ (succâ„¤ k)) â‰¡âŸ¨ predsuccâ„¤ (succâ„¤ k) âŸ©
         succâ„¤ k âˆ
  stepâ‚‚ : (k : â„¤) â†’ Â¬ (succâ„¤ k â‰¡ succâ„¤ (succâ„¤ k)) â†’ Â¬ (k â‰¡ succâ„¤ k)
  stepâ‚‚ k IH e = IH (ap succâ„¤ e)
-}
