Tom de Jong, 18 September 2020
22 January 2021 reboot

\begin{code}

{-# OPTIONS --without-K --exact-split --safe #-}

open import SpartanMLTT
open import UF-Base

open import UF-Embeddings
open import UF-Equiv
open import UF-EquivalenceExamples
open import UF-FunExt
open import UF-Lower-FunExt
open import UF-Subsingletons
open import UF-Retracts

module Integers where

-- The following two lemmas are dependent adaptations from
-- https://www.cs.bham.ac.uk/~mhe/HoTT-UF-in-Agda-Lecture-Notes/HoTT-UF-Agda.html#â„•-is-nno
-- We should move them to some file on â„•.
â„•-induction-retract : funext ğ“¤â‚€ ğ“¤
                    â†’ (Y : â„• â†’ ğ“¤ Ì‡ ) (yâ‚€ : Y 0) (g : (n : â„•) â†’ Y n â†’ Y (succ n))
                    â†’ (Î£ h ê‰ (Î  Y) , (h 0 â‰¡ yâ‚€) Ã—
                                     ((n : â„•) â†’ h (succ n) â‰¡ g n (h n)))
                    â— (Î£ h ê‰ (Î  Y) , h â‰¡ induction yâ‚€ g)
â„•-induction-retract fe Y yâ‚€ g = Î£-retract _ _ Î³
 where
  Î³ : (h : Î  Y)
    â†’ (h 0 â‰¡ yâ‚€) Ã— ((n : â„•) â†’ h (succ n) â‰¡ g n (h n))
    â— (h â‰¡ induction yâ‚€ g)
  Î³ h =  (h 0 â‰¡ yâ‚€) Ã— ((n : â„•) â†’ h (succ n) â‰¡ g n (h n)) â—âŸ¨ i  âŸ©
         (h âˆ¼ induction yâ‚€ g)                            â—âŸ¨ ii âŸ©
         (h â‰¡ induction yâ‚€ g)                            â—€
   where
    ii = â‰ƒ-gives-â— (â‰ƒ-sym (â‰ƒ-funext fe h (induction yâ‚€ g)))
    i  = r , s , Î·
     where
      r : h âˆ¼ induction yâ‚€ g
        â†’ (h 0 â‰¡ yâ‚€) Ã— ((n : â„•) â†’ h (succ n) â‰¡ g n (h n))
      r H = H 0 , (Î» n â†’ h (succ n)              â‰¡âŸ¨ H (succ n)          âŸ©
                         induction yâ‚€ g (succ n) â‰¡âŸ¨ refl                âŸ©
                         g n (induction yâ‚€ g n)  â‰¡âŸ¨ ap (g n) ((H n) â»Â¹) âŸ©
                         g n (h n)               âˆ)
      s : (h 0 â‰¡ yâ‚€) Ã— ((n : â„•) â†’ h (succ n) â‰¡ g n (h n))
        â†’ h âˆ¼ induction yâ‚€ g
      s (p , K) 0 = p
      s (p , K) (succ n) = h (succ n)              â‰¡âŸ¨ K n                    âŸ©
                           g n (h n)               â‰¡âŸ¨ ap (g n) (s (p , K) n) âŸ©
                           g n (induction yâ‚€ g n)  â‰¡âŸ¨ refl                   âŸ©
                           induction yâ‚€ g (succ n) âˆ
      Î· : r âˆ˜ s âˆ¼ id
      Î· (p , K) =
       r (s (p , K))                                      â‰¡âŸ¨ refl âŸ©
       (p , Î» n â†’ s (p , K) (succ n)
                  âˆ™ (refl âˆ™ ap (g n) ((s (p , K) n) â»Â¹))) â‰¡âŸ¨ Ï†    âŸ©
       (p , K)                                            âˆ
         where
          Ï† = ap (p ,_) (dfunext fe Ïˆ)
           where
            Ïˆ : (n : â„•)
              â†’ s (p , K) (succ n) âˆ™ (refl âˆ™ ap (g n) (s (p , K) n â»Â¹))
              â‰¡ K n
            Ïˆ n = s (p , K) (succ n)
                    âˆ™ (refl âˆ™ ap (g n) (s (p , K) n â»Â¹))   â‰¡âŸ¨ refl âŸ©
                  K n âˆ™ ap (g n) (s (p , K) n)
                    âˆ™ (refl âˆ™ ap (g n) ((s (p , K) n) â»Â¹)) â‰¡âŸ¨ I    âŸ©
                  K n âˆ™ ap (g n) (s (p , K) n)
                    âˆ™ ap (g n) ((s (p , K) n) â»Â¹)          â‰¡âŸ¨ II   âŸ©
                  K n âˆ™ (ap (g n) (s (p , K) n)
                    âˆ™ ap (g n) ((s (p , K) n) â»Â¹))         â‰¡âŸ¨ III  âŸ©
                  K n âˆ™ (ap (g n) (s (p , K) n)
                    âˆ™ (ap (g n) (s (p , K) n)) â»Â¹)         â‰¡âŸ¨ IV   âŸ©
                  K n âˆ™ refl                               â‰¡âŸ¨ refl âŸ©
                  K n                                      âˆ
             where
              I   = ap (K n âˆ™ ap (g n) (s (p , K) n) âˆ™_)
                     (refl-left-neutral {_} {_} {_} {_}
                       {ap (g n) ((s (p , K) n) â»Â¹)})
              II  = âˆ™assoc
                     (K n)
                     (ap (g n) (s (p , K) n))
                     (ap (g n) ((s (p , K) n) â»Â¹))
              III = ap (Î» - â†’ K n âˆ™ (ap (g n) (s (p , K) n) âˆ™ -))
                     ((ap-sym (g n) (s (p , K) n)) â»Â¹)
              IV  = ap (K n âˆ™_)
                     ((right-inverse (ap (g n) (s (p , K) n))) â»Â¹)

â„•-is-nno-dep : funext ğ“¤â‚€ ğ“¤
             â†’ (Y : â„• â†’ ğ“¤ Ì‡ ) (yâ‚€ : Y 0) (g : (n : â„•) â†’ Y n â†’ Y (succ n))
             â†’ âˆƒ! h ê‰ (Î  Y) , ((h 0 â‰¡ yâ‚€) Ã— ((n : â„•) â†’ h (succ n) â‰¡ g n (h n)))
â„•-is-nno-dep {ğ“¤} fe Y yâ‚€ g = Î³
 where
  Î³ : is-singleton
       (Î£ h ê‰ (Î  Y) , (h 0 â‰¡ yâ‚€) Ã— ((n : â„•) â†’ h (succ n) â‰¡ g n (h n)))
  Î³ = retract-of-singleton (â„•-induction-retract fe Y yâ‚€ g)
       (singleton-types'-are-singletons (induction {ğ“¤} {Y} yâ‚€ g))

-- We don't have a use of this (yet)
{-
exercise : funext ğ“¤â‚€ ğ“¤
         â†’ (Y : â„• â†’ ğ“¤ Ì‡ ) (g : (n : â„•) â†’ Y n â†’ Y (succ n))
         â†’ (Î£ h ê‰ (Î  Y) , ((n : â„•) â†’ h (succ n) â‰¡ g n (h n)))
         â‰ƒ Y 0
exercise fe Y g = qinveq Ï€â‚€ (r , Îµ , Î·)
 where
  Ï€â‚€ : (Î£ h ê‰ (Î  Y) , ((n : â„•) â†’ h (succ n) â‰¡ g n (h n))) â†’ Y 0
  Ï€â‚€ (h , p) = h 0
  r : Y 0
    â†’ (Î£ h ê‰ (Î  Y) , ((n : â„•) â†’ h (succ n) â‰¡ g n (h n)))
  r yâ‚€ = h , (Î» n â†’ refl)
   where
    h : Î  Y
    h zero = yâ‚€
    h (succ n) = g n (h n)
  Îµ : r âˆ˜ Ï€â‚€ âˆ¼ id
  Îµ (h , p) = ap u e
   where
    h' : Î  Y
    h' = prâ‚ (r (Ï€â‚€ (h , p)))
    p' : (n : â„•)
       â†’ h' (succ n) â‰¡ g n (h' n)
    p' = prâ‚‚ (r (Ï€â‚€ (h , p)))
    s : Î£ f ê‰ (Î  Y) , ((f 0 â‰¡ h 0) Ã— ((n : â„•) â†’ f (succ n) â‰¡ g n (f n)))
    s = h' , refl , p'
    t : Î£ f ê‰ (Î  Y) , ((f 0 â‰¡ h 0) Ã— ((n : â„•) â†’ f (succ n) â‰¡ g n (f n)))
    t = h , refl , p
    e : s â‰¡ t
    e = singletons-are-props (â„•-is-nno-dep fe Y (h 0) g) s t
    u : (Î£ f ê‰ (Î  Y) , ((f 0 â‰¡ h 0) Ã— ((n : â„•) â†’ f (succ n) â‰¡ g n (f n))))
      â†’ (Î£ f ê‰ (Î  Y) , ((n : â„•) â†’ f (succ n) â‰¡ g n (f n)))
    u (f , _ , q) = f , q
  Î· : Ï€â‚€ âˆ˜ r âˆ¼ id
  Î· yâ‚€ = refl
-}

â„¤ : ğ“¤â‚€ Ì‡
â„¤ = â„• + ğŸ™ + â„•

pattern ğŸ = inr (inl *)
pattern pos i = inr (inr i)
pattern neg i = inl i

â„•-to-â„¤â‚Š : â„• â†’ â„¤
â„•-to-â„¤â‚Š 0        = ğŸ
â„•-to-â„¤â‚Š (succ n) = pos n

â„•-to-â„¤â‚‹ : â„• â†’ â„¤
â„•-to-â„¤â‚‹ 0        = ğŸ
â„•-to-â„¤â‚‹ (succ n) = neg n

â„¤-induction : {ğ“¤ : Universe} (P : â„¤ â†’ ğ“¤ Ì‡ )
            â†’ P ğŸ
            â†’ ((n : â„•) â†’ P (â„•-to-â„¤â‚Š n) â†’ P (â„•-to-â„¤â‚Š (succ n)))
            â†’ ((n : â„•) â†’ P (â„•-to-â„¤â‚‹ n) â†’ P (â„•-to-â„¤â‚‹ (succ n)))
            â†’ (z : â„¤) â†’ P z
â„¤-induction {ğ“¤} P pâ‚€ pâ‚Š pâ‚‹ ğŸ       = pâ‚€
â„¤-induction {ğ“¤} P pâ‚€ pâ‚Š pâ‚‹ (pos i) = h (succ i)
 where
  Pâ‚Š : â„• â†’ ğ“¤ Ì‡
  Pâ‚Š = P âˆ˜ â„•-to-â„¤â‚Š
  h : (n : â„•) â†’ Pâ‚Š n
  h = induction pâ‚€ pâ‚Š
â„¤-induction {ğ“¤} P pâ‚€ pâ‚Š pâ‚‹ (neg i) = h (succ i)
 where
  Pâ‚‹ : â„• â†’ ğ“¤ Ì‡
  Pâ‚‹ = P âˆ˜ â„•-to-â„¤â‚‹
  h : (n : â„•) â†’ Pâ‚‹ n
  h = induction pâ‚€ pâ‚‹

succ-â„¤ : â„¤ â†’ â„¤
succ-â„¤ ğŸ              = pos 0
succ-â„¤ (pos n)        = pos (succ n)
succ-â„¤ (neg 0)        = ğŸ
succ-â„¤ (neg (succ n)) = neg n

-- Theorem 3.13 of "Construction of the Circle in UniMath"
-- by Bezem, Buchholtz, Grayson and Shulman
-- https://arxiv.org/abs/1910.01856
â„¤-symmetric-induction : {ğ“¤ : Universe}
                      â†’ funext ğ“¤â‚€ ğ“¤
                      â†’ (A : â„¤ â†’ ğ“¤ Ì‡ )
                        (f : (z : â„¤) â†’ A z â‰ƒ A (succ-â„¤ z))
                      â†’ (Î£ h ê‰ Î  A , ((z : â„¤) â†’ h (succ-â„¤ z) â‰¡ âŒœ f z âŒ (h z)))
                      â‰ƒ A ğŸ
â„¤-symmetric-induction {ğ“¤} fe A f =
 (Î£ h ê‰ Î  A , Qâ‚ h)                                               â‰ƒâŸ¨ I    âŸ©
 (Î£ h ê‰ (Î  (A âˆ˜ neg) Ã— Î  (A âˆ˜ inr)) , Qâ‚ (gâ‚ h))                  â‰ƒâŸ¨ II   âŸ©
 (Î£ hâ‚™ ê‰ Î  (A âˆ˜ neg) , Î£ háµ£ ê‰ Î  (A âˆ˜ inr) , Qâ‚ (gâ‚ (hâ‚™ , háµ£)))    â‰ƒâŸ¨ III  âŸ©
 (Î£ hâ‚™ ê‰ Î  (A âˆ˜ neg) , Î£ háµ£ ê‰ (Î  (A âˆ˜ âŒœğŸâŒ) Ã— Î  (A âˆ˜ pos)) ,
                         Qâ‚‚ hâ‚™ (gâ‚‚ háµ£))                           â‰ƒâŸ¨ IV   âŸ©
 (Î£ hâ‚™ ê‰ Î  (A âˆ˜ neg) , Î£ hâ‚’ ê‰ Î  (A âˆ˜ âŒœğŸâŒ) ,
                       Î£ hâ‚š ê‰ Î  (A âˆ˜ pos) , Qâ‚‚ hâ‚™ (gâ‚‚ (hâ‚’ , hâ‚š))) â‰ƒâŸ¨ V    âŸ©
 (Î£ hâ‚’ ê‰ Î  (A âˆ˜ âŒœğŸâŒ) , Î£ hâ‚™ ê‰ Î  (A âˆ˜ neg) ,
                       Î£ hâ‚š ê‰ Î  (A âˆ˜ pos) , Qâ‚‚ hâ‚™ (gâ‚‚ (hâ‚’ , hâ‚š))) â‰ƒâŸ¨ VI   âŸ©
 (Î£ hâ‚’ ê‰ Î  (A âˆ˜ âŒœğŸâŒ) , Î£ hâ‚™ ê‰ Î  (A âˆ˜ neg) ,
                       Î£ hâ‚š ê‰ Î  (A âˆ˜ pos) , Qâ‚™' (hâ‚’ *) hâ‚™
                                          Ã— Qâ‚š (hâ‚’ *) hâ‚š)         â‰ƒâŸ¨ VII  âŸ©
 (Î£ hâ‚’ ê‰ Î  (A âˆ˜ âŒœğŸâŒ) , (Î£ hâ‚™ ê‰ Î  (A âˆ˜ neg) , Qâ‚™' (hâ‚’ *) hâ‚™)
                     Ã— (Î£ hâ‚š ê‰ Î  (A âˆ˜ pos) , Qâ‚š (hâ‚’ *) hâ‚š))       â‰ƒâŸ¨ VIII âŸ©
 (Î£ hâ‚’ ê‰ Î  (A âˆ˜ âŒœğŸâŒ) , (Î£ hâ‚™ ê‰ Î  (A âˆ˜ neg) , Qâ‚™' (hâ‚’ *) hâ‚™) Ã— ğŸ™)  â‰ƒâŸ¨ IX   âŸ©
 (Î£ hâ‚’ ê‰ Î  (A âˆ˜ âŒœğŸâŒ) , (Î£ hâ‚™ ê‰ Î  (A âˆ˜ neg) , Qâ‚™' (hâ‚’ *) hâ‚™))      â‰ƒâŸ¨ X    âŸ©
 (Î£ hâ‚’ ê‰ Î  (A âˆ˜ âŒœğŸâŒ) , (Î£ hâ‚™ ê‰ Î  (A âˆ˜ neg) , Qâ‚™ (hâ‚’ *) hâ‚™))       â‰ƒâŸ¨ XI   âŸ©
 (Î£ hâ‚’ ê‰ Î  (A âˆ˜ âŒœğŸâŒ) , ğŸ™)                                         â‰ƒâŸ¨ XII  âŸ©
 Î  (A âˆ˜ âŒœğŸâŒ)                                                      â‰ƒâŸ¨ XIII âŸ©
 A ğŸ                                                              â– 
  where
   âŒœğŸâŒ : ğŸ™ {ğ“¤â‚€} â†’ â„¤
   âŒœğŸâŒ _ = ğŸ
   Qâ‚ : Î  A â†’ ğ“¤ Ì‡
   Qâ‚ h = (z : â„¤) â†’ h (succ-â„¤ z) â‰¡ âŒœ f z âŒ (h z)
   gâ‚ : Î  (A âˆ˜ neg) Ã— Î  (A âˆ˜ inr) â†’ Î  A
   gâ‚ = âŒœ Î Ã—+ fe âŒ
   Qâ‚‚ : Î  (A âˆ˜ neg) â†’ Î  (A âˆ˜ inr) â†’ ğ“¤ Ì‡
   Qâ‚‚ hâ‚™ háµ£ = Qâ‚ (gâ‚ (hâ‚™ , háµ£))
   gâ‚‚ : Î  (A âˆ˜ âŒœğŸâŒ) Ã— Î  (A âˆ˜ pos) â†’ Î  (A âˆ˜ inr)
   gâ‚‚ = âŒœ Î Ã—+ fe âŒ
   Qâ‚š : A ğŸ â†’ Î  (A âˆ˜ pos) â†’ ğ“¤ Ì‡
   Qâ‚š aâ‚’ hâ‚š = (hâ‚š 0 â‰¡ âŒœ f ğŸ âŒ aâ‚’)
            Ã— ((n : â„•) â†’ hâ‚š (succ n) â‰¡ âŒœ f (pos n) âŒ (hâ‚š n))
   Qâ‚™' : A ğŸ â†’ Î  (A âˆ˜ neg) â†’ ğ“¤ Ì‡
   Qâ‚™' aâ‚€ hâ‚™ = (aâ‚€ â‰¡ âŒœ f (neg 0) âŒ (hâ‚™ 0))
             Ã— ((n : â„•) â†’ hâ‚™ n â‰¡ âŒœ f (neg (succ n)) âŒ (hâ‚™ (succ n)))
   Qâ‚™ : A ğŸ â†’ Î  (A âˆ˜ neg) â†’ ğ“¤ Ì‡
   Qâ‚™ aâ‚’ hâ‚™ = (hâ‚™ 0 â‰¡ âŒœ â‰ƒ-sym (f (neg 0)) âŒ aâ‚’)
            Ã— ((n : â„•) â†’ hâ‚™ (succ n) â‰¡ âŒœ â‰ƒ-sym (f (neg (succ n))) âŒ (hâ‚™ n))
   I    =  â‰ƒ-sym (Î£-change-of-variable Qâ‚ gâ‚ (âŒœâŒ-is-equiv (Î Ã—+ fe)))
   II   = Î£-assoc
   III  = Î£-cong
          (Î» hâ‚™ â†’ â‰ƒ-sym (Î£-change-of-variable (Qâ‚‚ hâ‚™) gâ‚‚ (âŒœâŒ-is-equiv (Î Ã—+ fe))))
   IV   = Î£-cong (Î» háµ£ â†’ Î£-assoc)
   V    = Î£-flip
   VI   = Î£-cong (Î» hâ‚’ â†’ Î£-cong (Î» hâ‚™ â†’ Î£-cong (Î» hâ‚š â†’ Î³ hâ‚’ hâ‚™ hâ‚š)))
    where
     Î³ : (hâ‚’ : Î  (A âˆ˜ âŒœğŸâŒ)) (hâ‚™ : Î  (A âˆ˜ neg)) (hâ‚š : Î  (A âˆ˜ pos))
       â†’ Qâ‚‚ hâ‚™ (gâ‚‚ (hâ‚’ , hâ‚š)) â‰ƒ Qâ‚™' (hâ‚’ *) hâ‚™ Ã— Qâ‚š (hâ‚’ *) hâ‚š
     Î³ hâ‚’ hâ‚™ hâ‚š = qinveq Ï† (Ïˆ , Î· , Îµ)
      where
       Ï† : Qâ‚‚ hâ‚™ (gâ‚‚ (hâ‚’ , hâ‚š)) â†’ Qâ‚™' (hâ‚’ *) hâ‚™ Ã— Qâ‚š (hâ‚’ *) hâ‚š
       Ï† q = ((q (neg 0) , q âˆ˜ neg âˆ˜ succ) , (q ğŸ , q âˆ˜ pos))
       Ïˆ : (Qâ‚™' (hâ‚’ *) hâ‚™ Ã— Qâ‚š (hâ‚’ *) hâ‚š) â†’ Qâ‚‚ hâ‚™ (gâ‚‚ (hâ‚’ , hâ‚š))
       Ïˆ ((qâ‚’' , qâ‚™') , (qâ‚’ , qâ‚š)) = c
        where
         c : Qâ‚‚ hâ‚™ (gâ‚‚ (hâ‚’ , hâ‚š))
         c ğŸ              = qâ‚’
         c (pos n)        = qâ‚š n
         c (neg zero)     = qâ‚’'
         c (neg (succ n)) = qâ‚™' n
       Îµ : Ï† âˆ˜ Ïˆ âˆ¼ id
       Îµ q = refl
       Î· : Ïˆ âˆ˜ Ï† âˆ¼ id
       Î· q = dfunext fe c
        where
         c : (z : â„¤) â†’ (Ïˆ (Ï† q)) z â‰¡ q (z)
         c ğŸ              = refl
         c (pos n)        = refl
         c (neg zero)     = refl
         c (neg (succ n)) = refl
   VII  = Î£-cong Î³
    where
     Î³ : (hâ‚’ : Î  (A âˆ˜ âŒœğŸâŒ))
       â†’ (Î£ hâ‚™ ê‰ Î  (A âˆ˜ neg) , Î£ hâ‚š ê‰ Î  (A âˆ˜ pos) , Qâ‚™' (hâ‚’ *) hâ‚™
                                                  Ã— Qâ‚š  (hâ‚’ *) hâ‚š)
       â‰ƒ ((Î£ hâ‚™ ê‰ Î  (A âˆ˜ neg) , Qâ‚™' (hâ‚’ *) hâ‚™)
        Ã— (Î£ hâ‚š ê‰ Î  (A âˆ˜ pos) , Qâ‚š  (hâ‚’ *) hâ‚š))
     Î³ hâ‚’ = qinveq Ï† (Ïˆ , Î· , Îµ)
      where
       Ï† : _
       Ï† (hâ‚™ , hâ‚š , q' , q) = ((hâ‚™ , q') , (hâ‚š , q))
       Ïˆ : _
       Ïˆ ((hâ‚™ , q') , (hâ‚š , q)) = hâ‚™ , hâ‚š , q' , q
       Î· : Ïˆ âˆ˜ Ï† âˆ¼ id
       Î· _ = refl
       Îµ : Ï† âˆ˜ Ïˆ âˆ¼ id
       Îµ _ = refl
   VIII = Î£-cong (Î» hâ‚’ â†’ Î£-cong (Î» _ â†’ singleton-â‰ƒ-ğŸ™ {ğ“¤} {ğ“¤â‚€} (Î³ hâ‚’)))
    where
     Î³ : (hâ‚’ : Î  (A âˆ˜ âŒœğŸâŒ))
       â†’ is-singleton ((Î£ hâ‚š ê‰ Î  (A âˆ˜ pos) , Qâ‚š  (hâ‚’ *) hâ‚š))
     Î³ hâ‚’ = (â„•-is-nno-dep fe (A âˆ˜ pos) aâ‚€ s)
      where
       aâ‚€ : A (pos 0)
       aâ‚€ = âŒœ (f ğŸ) âŒ (hâ‚’ *)
       s : (n : â„•) â†’ A (pos n) â†’ A (pos (succ n))
       s n = âŒœ f (pos n) âŒ
   IX   = Î£-cong (Î» _ â†’ ğŸ™-rneutral)
   X    = Î£-cong (Î» hâ‚’ â†’ Î£-cong (Î» hâ‚™ â†’ Î³ hâ‚’ hâ‚™))
    where
     Î³ : (hâ‚’ : Î  (A âˆ˜ âŒœğŸâŒ)) (hâ‚™ : Î  (A âˆ˜ neg))
       â†’ Qâ‚™' (hâ‚’ *) hâ‚™ â‰ƒ Qâ‚™ (hâ‚’ *) hâ‚™
     Î³ hâ‚’ hâ‚™ = Ã—-cong Î³â‚€ (Î -cong fe fe â„• _ _ Î³â‚™)
      where
       fâ‚€ = âŒœ f (neg 0) âŒ
       fâ‚€â»Â¹ = âŒœ â‰ƒ-sym (f (neg 0)) âŒ
       eâ‚€ : is-equiv fâ‚€
       eâ‚€ = âŒœâŒ-is-equiv (f (neg 0))
       Î³â‚€ : (hâ‚’ * â‰¡ fâ‚€ (hâ‚™ 0))
          â‰ƒ (hâ‚™ 0 â‰¡ fâ‚€â»Â¹ (hâ‚’ *))
       Î³â‚€ = (hâ‚’ * â‰¡ fâ‚€ (hâ‚™ 0))             â‰ƒâŸ¨ Iâ‚€   âŸ©
            (fâ‚€ (hâ‚™ 0) â‰¡ hâ‚’ *)             â‰ƒâŸ¨ IIâ‚€  âŸ©
            (fâ‚€ (hâ‚™ 0) â‰¡ fâ‚€ (fâ‚€â»Â¹ (hâ‚’ *))) â‰ƒâŸ¨ IIIâ‚€ âŸ©
            (hâ‚™ 0 â‰¡ fâ‚€â»Â¹ (hâ‚’ *)) â– 
        where
         Iâ‚€   = â‰¡-flip
         IIâ‚€  = â‰¡-cong-r (fâ‚€ (hâ‚™ 0)) (hâ‚’ *)
                 ((inverses-are-sections fâ‚€ eâ‚€ (hâ‚’ *)) â»Â¹)
         IIIâ‚€ = embedding-criterion-converse fâ‚€
                 (equivs-are-embeddings fâ‚€ eâ‚€)
                 (hâ‚™ 0) (fâ‚€â»Â¹ (hâ‚’ *))
       fâ‚™ : (n : â„•) â†’ A (neg (succ n)) â†’ A (neg n)
       fâ‚™ n = âŒœ f (neg (succ n)) âŒ
       eâ‚™ : (n : â„•) â†’ is-equiv (fâ‚™ n)
       eâ‚™ n = âŒœâŒ-is-equiv (f (neg (succ n)))
       fâ‚™â»Â¹ : (n : â„•) â†’ A (neg n) â†’ A (neg (succ n))
       fâ‚™â»Â¹ n = âŒœ â‰ƒ-sym (f (neg (succ n))) âŒ
       Î³â‚™ : (n : â„•)
          â†’ (hâ‚™ n â‰¡ fâ‚™ n (hâ‚™ (succ n)))
          â‰ƒ (hâ‚™ (succ n) â‰¡ fâ‚™â»Â¹ n (hâ‚™ n))
       Î³â‚™ n = (hâ‚™ n â‰¡ fâ‚™ n (hâ‚™ (succ n)))                 â‰ƒâŸ¨ Iâ‚™ âŸ©
              (fâ‚™ n (hâ‚™ (succ n)) â‰¡ hâ‚™ n)                 â‰ƒâŸ¨ IIâ‚™ âŸ©
              (fâ‚™ n (hâ‚™ (succ n)) â‰¡ fâ‚™ n (fâ‚™â»Â¹ n (hâ‚™ n))) â‰ƒâŸ¨ IIIâ‚™ âŸ©
              (hâ‚™ (succ n) â‰¡ fâ‚™â»Â¹ n (hâ‚™ n))               â– 
        where
         Iâ‚™   = â‰¡-flip
         IIâ‚™  = â‰¡-cong-r (fâ‚™ n (hâ‚™ (succ n))) (hâ‚™ n)
                 ((inverses-are-sections (fâ‚™ n) (eâ‚™ n) (hâ‚™ n)) â»Â¹)
         IIIâ‚™ = embedding-criterion-converse (fâ‚™ n)
                 (equivs-are-embeddings (fâ‚™ n) (eâ‚™ n))
                 (hâ‚™ (succ n)) (fâ‚™â»Â¹ n (hâ‚™ n))
   XI   = Î£-cong (Î» hâ‚’ â†’ singleton-â‰ƒ-ğŸ™ {ğ“¤} {ğ“¤â‚€} (Î³ hâ‚’))
    where
     Î³ : (hâ‚’ : Î  (A âˆ˜ âŒœğŸâŒ))
       â†’ is-singleton ((Î£ hâ‚™ ê‰ Î  (A âˆ˜ neg) , Qâ‚™  (hâ‚’ *) hâ‚™))
     Î³ hâ‚’ = (â„•-is-nno-dep fe (A âˆ˜ neg) aâ‚€ s)
      where
       aâ‚€ : A (neg 0)
       aâ‚€ = âŒœ â‰ƒ-sym (f (neg 0)) âŒ (hâ‚’ *)
       s : (n : â„•) â†’ A (neg n) â†’ A (neg (succ n))
       s n = âŒœ â‰ƒ-sym (f (neg (succ n))) âŒ
   XII  = ğŸ™-rneutral
   XIII = â‰ƒ-sym (ğŸ™â†’ fe)

{-
pred-â„¤ : â„¤ â†’ â„¤
pred-â„¤ ğŸ              = neg 0
pred-â„¤ (pos 0)        = ğŸ
pred-â„¤ (pos (succ n)) = pos n
pred-â„¤ (neg n)        = neg (succ n)

pred-section-of-succ : succ-â„¤ âˆ˜ pred-â„¤ âˆ¼ id
pred-section-of-succ ğŸ              = refl
pred-section-of-succ (pos zero)     = refl
pred-section-of-succ (pos (succ n)) = refl
pred-section-of-succ (neg n)        = refl

pred-retraction-of-succ : pred-â„¤ âˆ˜ succ-â„¤ âˆ¼ id
pred-retraction-of-succ ğŸ              = refl
pred-retraction-of-succ (pos n)        = refl
pred-retraction-of-succ (neg zero)     = refl
pred-retraction-of-succ (neg (succ n)) = refl
-}

\end{code}
