Martin Escardo 1st May 2020.

This is ported from the Midlands Graduate School 2019 lecture notes

 https://www.cs.bham.ac.uk/~mhe/HoTT-UF-in-Agda-Lecture-Notes/HoTT-UF-Agda.html
 https://github.com/martinescardo/HoTT-UF-Agda-Lecture-Notes

\begin{code}

{-# OPTIONS --without-K --exact-split --safe --auto-inline #-}

module MGS-HAE where

open import MGS-Equivalence-Induction public

is-hae : {X : ğ“¤ Ì‡ } {Y : ğ“¥ Ì‡ } â†’ (X â†’ Y) â†’ ğ“¤ âŠ” ğ“¥ Ì‡
is-hae f = Î£ g ê‰ (codomain f â†’ domain f)
         , Î£ Î· ê‰ g âˆ˜ f âˆ¼ id
         , Î£ Îµ ê‰ f âˆ˜ g âˆ¼ id
         , ((x : domain f) â†’ ap f (Î· x) â‰¡ Îµ (f x))

haes-are-invertible : {X : ğ“¤ Ì‡ } {Y : ğ“¥ Ì‡ } (f : X â†’ Y)
                    â†’ is-hae f â†’ invertible f

haes-are-invertible f (g , Î· , Îµ , Ï„) = g , Î· , Îµ

transport-ap-â‰ƒ : {X : ğ“¤ Ì‡ } {Y : ğ“¥ Ì‡ } (f : X â†’ Y)
                 {x x' : X} (a : x' â‰¡ x) (b : f x' â‰¡ f x)
               â†’ (transport (Î» - â†’ f - â‰¡ f x) a b â‰¡ refl (f x)) â‰ƒ (ap f a â‰¡ b)

transport-ap-â‰ƒ f (refl x) b = Î³
 where
  Î³ : (b â‰¡ refl (f x)) â‰ƒ (refl (f x) â‰¡ b)
  Î³ = â»Â¹-â‰ƒ b (refl (f x))

haes-are-equivs : {X : ğ“¤ Ì‡ } {Y : ğ“¥ Ì‡ } (f : X â†’ Y)
                â†’ is-hae f â†’ is-equiv f

haes-are-equivs f (g , Î· , Îµ , Ï„) y = Î³
 where
  c : (Ï† : fiber f y) â†’ (g y , Îµ y) â‰¡ Ï†
  c (x , refl .(f x)) = q
   where
    p : transport (Î» - â†’ f - â‰¡ f x) (Î· x) (Îµ (f x)) â‰¡ refl (f x)
    p = âŒœ â‰ƒ-sym (transport-ap-â‰ƒ f (Î· x) (Îµ (f x))) âŒ (Ï„ x)

    q : (g (f x) , Îµ (f x)) â‰¡ (x , refl (f x))
    q = to-Î£-â‰¡ (Î· x , p)

  Î³ : is-singleton (fiber f y)
  Î³ = (g y , Îµ y) , c

id-is-hae : (X : ğ“¤ Ì‡ ) â†’ is-hae (ğ‘–ğ‘‘ X)
id-is-hae X = ğ‘–ğ‘‘ X , refl , refl , (Î» x â†’ refl (refl x))

ua-equivs-are-haes : is-univalent ğ“¤
                   â†’ {X Y : ğ“¤ Ì‡ } (f : X â†’ Y)
                   â†’ is-equiv f â†’ is-hae f

ua-equivs-are-haes ua {X} {Y} = ğ•-equiv ua (Î» X Y f â†’ is-hae f) id-is-hae X Y

equivs-are-haes : {X : ğ“¤ Ì‡ } {Y : ğ“¥ Ì‡ } (f : X â†’ Y)
                â†’ is-equiv f â†’ is-hae f

equivs-are-haes {ğ“¤} {ğ“¥} {X} {Y} f i = (g , Î· , Îµ , Ï„)
 where
  g : Y â†’ X
  g = inverse f i

  Î· : g âˆ˜ f âˆ¼ id
  Î· = inverses-are-retractions f i

  Îµ : f âˆ˜ g âˆ¼ id
  Îµ = inverses-are-sections f i

  Ï„ : (x : X) â†’ ap f (Î· x) â‰¡ Îµ (f x)
  Ï„ x = Î³
   where
    Ï† : fiber f (f x)
    Ï† = center (fiber f (f x)) (i (f x))

    by-definition-of-g : g (f x) â‰¡ fiber-point Ï†
    by-definition-of-g = refl _

    p : Ï† â‰¡ (x , refl (f x))
    p = centrality (fiber f (f x)) (i (f x)) (x , refl (f x))

    a : g (f x) â‰¡ x
    a = ap fiber-point p

    b : f (g (f x)) â‰¡ f x
    b = fiber-identification Ï†

    by-definition-of-Î· : Î· x â‰¡ a
    by-definition-of-Î· = refl _

    by-definition-of-Îµ : Îµ (f x) â‰¡ b
    by-definition-of-Îµ = refl _

    q = transport (Î» - â†’ f - â‰¡ f x)       a          b         â‰¡âŸ¨ refl _ âŸ©
        transport (Î» - â†’ f - â‰¡ f x)       (ap prâ‚ p) (prâ‚‚ Ï†)   â‰¡âŸ¨ t âŸ©
        transport (Î» - â†’ f (prâ‚ -) â‰¡ f x) p          (prâ‚‚ Ï†)   â‰¡âŸ¨ apd prâ‚‚ p âŸ©
        refl (f x)                                             âˆ
     where
      t = (transport-ap (Î» - â†’ f - â‰¡ f x) prâ‚ p b)â»Â¹

    Î³ : ap f (Î· x) â‰¡ Îµ (f x)
    Î³ = âŒœ transport-ap-â‰ƒ f a b âŒ q

equivs-are-haes' : {X : ğ“¤ Ì‡ } {Y : ğ“¥ Ì‡ } (f : X â†’ Y)
                 â†’ is-equiv f â†’ is-hae f

equivs-are-haes' f e = (inverse f e ,
                        inverses-are-retractions f e ,
                        inverses-are-sections f e ,
                        Ï„)
 where
  Ï„ : âˆ€ x â†’ ap f (inverses-are-retractions f e x) â‰¡ inverses-are-sections f e (f x)
  Ï„ x = âŒœ transport-ap-â‰ƒ f (ap prâ‚ p) (prâ‚‚ Ï†) âŒ q
   where
    Ï† : fiber f (f x)
    Ï† = prâ‚ (e (f x))

    p : Ï† â‰¡ (x , refl (f x))
    p = prâ‚‚ (e (f x)) (x , refl (f x))

    q : transport (Î» - â†’ f - â‰¡ f x) (ap prâ‚ p) (prâ‚‚ Ï†) â‰¡ refl (f x)
    q = (transport-ap (Î» - â†’ f - â‰¡ f x) prâ‚ p ((prâ‚‚ Ï†)))â»Â¹ âˆ™ apd prâ‚‚ p

equiv-invertible-hae-factorization : {X : ğ“¤ Ì‡ } {Y : ğ“¥ Ì‡ } (f : X â†’ Y)
                                   â†’ equivs-are-invertible f
                                   âˆ¼ haes-are-invertible f âˆ˜ equivs-are-haes f

equiv-invertible-hae-factorization f e = refl (equivs-are-invertible f e)

half-adjoint-condition : {X : ğ“¤ Ì‡ } {Y : ğ“¥ Ì‡ } (f : X â†’ Y) (e : is-equiv f) (x : X)
                       â†’ ap f (inverses-are-retractions f e x) â‰¡ inverses-are-sections f e (f x)

half-adjoint-condition f e = prâ‚‚ (prâ‚‚ (prâ‚‚ (equivs-are-haes f e)))

Î£-change-of-variable : {X : ğ“¤ Ì‡ } {Y : ğ“¥ Ì‡ } (A : Y â†’ ğ“¦ Ì‡ ) (f : X â†’ Y)
                     â†’ is-equiv f â†’ (Î£ y ê‰ Y , A y) â‰ƒ (Î£ x ê‰ X , A (f x))

Î£-change-of-variable {ğ“¤} {ğ“¥} {ğ“¦} {X} {Y} A f i = Î³
 where
  g = inverse f i
  Î· = inverses-are-retractions f i
  Îµ = inverses-are-sections f i
  Ï„ = half-adjoint-condition f i

  Ï† : Î£ A â†’ Î£ (A âˆ˜ f)
  Ï† (y , a) = (g y , transport A ((Îµ y)â»Â¹) a)

  Ïˆ : Î£ (A âˆ˜ f) â†’ Î£ A
  Ïˆ (x , a) = (f x , a)

  ÏˆÏ† : (z : Î£ A) â†’ Ïˆ (Ï† z) â‰¡ z
  ÏˆÏ† (y , a) = p
   where
    p : (f (g y) , transport A ((Îµ y)â»Â¹) a) â‰¡ (y , a)
    p = to-Î£-â‰¡ (Îµ y , transport-is-retraction A (Îµ y) a)

  Ï†Ïˆ : (t : Î£ (A âˆ˜ f)) â†’ Ï† (Ïˆ t) â‰¡ t
  Ï†Ïˆ (x , a) = p
   where
    a' : A (f (g (f x)))
    a' = transport A ((Îµ (f x))â»Â¹) a

    q = transport (A âˆ˜ f) (Î· x)  a' â‰¡âŸ¨ transport-ap A f (Î· x) a' âŸ©
        transport A (ap f (Î· x)) a' â‰¡âŸ¨ ap (Î» - â†’ transport A - a') (Ï„ x) âŸ©
        transport A (Îµ (f x))    a' â‰¡âŸ¨ transport-is-retraction A (Îµ (f x)) a âŸ©
        a                          âˆ

    p : (g (f x) , transport A ((Îµ (f x))â»Â¹) a) â‰¡ (x , a)
    p = to-Î£-â‰¡ (Î· x , q)

  Î³ : Î£ A â‰ƒ Î£ (A âˆ˜ f)
  Î³ = invertibility-gives-â‰ƒ Ï† (Ïˆ , ÏˆÏ† , Ï†Ïˆ)

~-naturality : {X : ğ“¤ Ì‡ } {A : ğ“¥ Ì‡ }
               (f g : X â†’ A) (H : f âˆ¼ g) {x y : X} {p : x â‰¡ y}
             â†’ H x âˆ™ ap g p â‰¡ ap f p âˆ™ H y

~-naturality f g H {x} {_} {refl a} = refl-left â»Â¹

~-naturality' : {X : ğ“¤ Ì‡ } {A : ğ“¥ Ì‡ }
                (f g : X â†’ A) (H : f âˆ¼ g) {x y : X} {p : x â‰¡ y}
              â†’ H x âˆ™ ap g p âˆ™ (H y)â»Â¹ â‰¡ ap f p

~-naturality' f g H {x} {x} {refl x} = â»Â¹-rightâˆ™ (H x)

~-id-naturality : {X : ğ“¤ Ì‡ }
                  (h : X â†’ X) (Î· : h âˆ¼ id) {x : X}
                â†’ Î· (h x) â‰¡ ap h (Î· x)

~-id-naturality h Î· {x} =

   Î· (h x)                         â‰¡âŸ¨ refl _ âŸ©
   Î· (h x) âˆ™ refl (h x)            â‰¡âŸ¨ i âŸ©
   Î· (h x) âˆ™ (Î· x âˆ™ (Î· x)â»Â¹)       â‰¡âŸ¨ ii âŸ©
   Î· (h x) âˆ™ Î· x âˆ™ (Î· x)â»Â¹         â‰¡âŸ¨ iii âŸ©
   Î· (h x) âˆ™ ap id (Î· x) âˆ™ (Î· x)â»Â¹ â‰¡âŸ¨ iv âŸ©
   ap h (Î· x)                      âˆ

 where
  i   = ap (Î·(h x) âˆ™_) ((â»Â¹-rightâˆ™ (Î· x))â»Â¹)
  ii  = (âˆ™assoc (Î· (h x)) (Î· x) (Î· x â»Â¹))â»Â¹
  iii = ap (Î» - â†’ Î· (h x) âˆ™ - âˆ™ Î· x â»Â¹) ((ap-id (Î· x))â»Â¹)
  iv  = ~-naturality' h id Î· {h x} {x} {Î· x}

invertibles-are-haes : {X : ğ“¤ Ì‡ } {Y : ğ“¥ Ì‡ } (f : X â†’ Y)
                     â†’ invertible f â†’ is-hae f

invertibles-are-haes f (g , Î· , Îµ) = g , Î· , Îµ' , Ï„
 where
  Îµ' = Î» y â†’ f (g y)         â‰¡âŸ¨ (Îµ (f (g y)))â»Â¹ âŸ©
             f (g (f (g y))) â‰¡âŸ¨ ap f (Î· (g y)) âŸ©
             f (g y)         â‰¡âŸ¨ Îµ y âŸ©
             y               âˆ

  module _ (x : domain f) where

   p = Î· (g (f x))       â‰¡âŸ¨ ~-id-naturality (g âˆ˜ f) Î· âŸ©
       ap (g âˆ˜ f) (Î· x)  â‰¡âŸ¨ ap-âˆ˜ f g (Î· x) âŸ©
       ap g (ap f (Î· x)) âˆ

   q = ap f (Î· (g (f x))) âˆ™ Îµ (f x)          â‰¡âŸ¨ by-p âŸ©
       ap f (ap g (ap f (Î· x))) âˆ™ Îµ (f x)    â‰¡âŸ¨ by-ap-âˆ˜ âŸ©
       ap (f âˆ˜ g) (ap f (Î· x))  âˆ™ Îµ (f x)    â‰¡âŸ¨ by-~-naturality âŸ©
       Îµ (f (g (f x))) âˆ™ ap id (ap f (Î· x))  â‰¡âŸ¨ by-ap-id âŸ©
       Îµ (f (g (f x))) âˆ™ ap f (Î· x)          âˆ
    where
     by-p            = ap (Î» - â†’ ap f - âˆ™ Îµ (f x)) p
     by-ap-âˆ˜         = ap (_âˆ™ Îµ (f x)) ((ap-âˆ˜ g f (ap f (Î· x)))â»Â¹)
     by-~-naturality = (~-naturality (f âˆ˜ g) id Îµ {f (g (f x))} {f x} {ap f (Î· x)})â»Â¹
     by-ap-id        = ap (Îµ (f (g (f x))) âˆ™_) (ap-id (ap f (Î· x)))

   Ï„ = ap f (Î· x)                                           â‰¡âŸ¨ refl-left â»Â¹ âŸ©
       refl (f (g (f x)))                     âˆ™ ap f (Î· x)  â‰¡âŸ¨ by-â»Â¹-leftâˆ™ âŸ©
       (Îµ (f (g (f x))))â»Â¹ âˆ™  Îµ (f (g (f x))) âˆ™ ap f (Î· x)  â‰¡âŸ¨ by-âˆ™assoc âŸ©
       (Îµ (f (g (f x))))â»Â¹ âˆ™ (Îµ (f (g (f x))) âˆ™ ap f (Î· x)) â‰¡âŸ¨ by-q âŸ©
       (Îµ (f (g (f x))))â»Â¹ âˆ™ (ap f (Î· (g (f x))) âˆ™ Îµ (f x)) â‰¡âŸ¨ refl _ âŸ©
       Îµ' (f x)                                             âˆ
    where
     by-â»Â¹-leftâˆ™ = ap (_âˆ™ ap f (Î· x)) ((â»Â¹-leftâˆ™ (Îµ (f (g (f x)))))â»Â¹)
     by-âˆ™assoc   = âˆ™assoc ((Îµ (f (g (f x))))â»Â¹) (Îµ (f (g (f x)))) (ap f (Î· x))
     by-q        = ap ((Îµ (f (g (f x))))â»Â¹ âˆ™_) (q â»Â¹)

\end{code}
