Martin Escardo, 21 March 2018

We prove the known (constructive) fact that

  X + ğŸ™ â‰ƒ Y + ğŸ™ â†’ X â‰ƒ Y.

The proof may be new (or not).

\begin{code}

{-# OPTIONS --without-K --exact-split #-}

open import SpartanMLTT
open import UF-Base
open import UF-Equiv
open import UF-FunExt
open import UF-Subsingletons-FunExt

module PlusOneLC (fe : âˆ€ U V â†’ funext U V) where

_âˆ–_ : âˆ€ {U} (X : U Ì‡) (a : X) â†’ U Ì‡
X âˆ– a = Î£ \(x : X) â†’ x â‰¢ a

add-and-remove-same-point : âˆ€ {U} {X : U Ì‡} â†’  X â‰ƒ (X + ğŸ™) âˆ– (inr *)
add-and-remove-same-point {U} {X} = f , ((g , fg) , (g , gf))
 where
  f : X â†’ (X + ğŸ™) âˆ– inr *
  f x = (inl x , Î» ())
  g : (X + ğŸ™) âˆ– inr * â†’ X
  g (inl x , u) = x
  g (inr * , u) = ğŸ˜-elim (u refl)
  fg : f âˆ˜ g âˆ¼ id
  fg (inl x , u) = to-Î£-â‰¡'' (refl , neg-is-prop (fe U Uâ‚€) _ _)
  fg (inr * , u) = ğŸ˜-elim (u refl)
  gf : g âˆ˜ f âˆ¼ id
  gf x = refl

remove-points : âˆ€ {U} {V} {X : U Ì‡} {Y : V Ì‡} (f : X â†’ Y) â†’ qinv f â†’ (a : X) â†’ X âˆ– a â‰ƒ Y âˆ– (f a)
remove-points {U} {V} {X} {Y} f (g , (gf , fg)) a = (f' , e')        
 where
  f' : X âˆ– a â†’ Y âˆ– (f a)
  f' (x , u) = (f x , Î»(p : f x â‰¡ f a) â†’ u ((gf x)â»Â¹ âˆ™ ap g p âˆ™ gf a))
  g' : Y âˆ– (f a) â†’ X âˆ– a
  g' (y , v) = (g y , Î»(p : g y â‰¡ a) â†’ v ((fg y) â»Â¹ âˆ™ ap f p))
  gf' : g' âˆ˜ f' âˆ¼ id
  gf' (x , _) = to-Î£-â‰¡'' (gf x , neg-is-prop (fe U Uâ‚€) _ _) 
  fg' : f' âˆ˜ g' âˆ¼ id
  fg' (y , _) = to-Î£-â‰¡'' (fg y , neg-is-prop (fe V Uâ‚€) _ _)
  e' : is-equiv f'
  e' = qinv-is-equiv f' (g' , gf' , fg')

open import DiscreteAndSeparated

add-one-and-remove-isolated-point : âˆ€ {V} {Y : V Ì‡} (z : Y + ğŸ™) â†’ isolated z â†’ ((Y + ğŸ™) âˆ– z) â‰ƒ Y
add-one-and-remove-isolated-point {V} {Y} (inl b) i = (f , qinv-is-equiv f (g , gf , fg))
 where
  f : (Y + ğŸ™) âˆ– (inl b) â†’ Y
  f (inl y , u) = y
  f (inr * , u) = b
  g' : (y : Y) â†’ decidable (inl b â‰¡ inl y) â†’ (Y + ğŸ™) âˆ– (inl b)
  g' y (inl p) = (inr * , Î» ())
  g' y (inr u) = (inl y , contrapositive (Î» p â†’ p â»Â¹) u)
  g : Y â†’ (Y + ğŸ™) âˆ– (inl b)
  g y = g' y (i (inl y))
  gf : g âˆ˜ f âˆ¼ id
  gf (inl y , u) = to-Î£-â‰¡'' (p , neg-is-prop (fe V Uâ‚€) _ _)
   where
    Ï† : (p : inl b â‰¡ inl y) (q : i (inl y) â‰¡ inl p) â†’ i (inl y) â‰¡ inr (â‰¢-sym u)
    Ï† p q = ğŸ˜-elim (u (p â»Â¹))
    Ïˆ : (v : inl b â‰¢ inl y) (q : i (inl y) â‰¡ inr v) â†’ i (inl y) â‰¡ inr (â‰¢-sym u)
    Ïˆ v q = q âˆ™ ap inr (neg-is-prop (fe V Uâ‚€) _ _)
    h : i (inl y) â‰¡ inr (â‰¢-sym u)
    h = equality-cases (i (inl y)) Ï† Ïˆ
    p : prâ‚(g' y (i (inl y))) â‰¡ inl y
    p = ap (prâ‚ âˆ˜ (g' y)) h
  gf (inr * , u) = equality-cases (i (inl b)) Ï† Ïˆ
   where
    Ï† : (p : inl b â‰¡ inl b) â†’ i (inl b) â‰¡ inl p â†’ g (f (inr * , u)) â‰¡ (inr * , u)
    Ï† p q = r âˆ™ to-Î£-â‰¡'' (refl , (neg-is-prop (fe V Uâ‚€) _ _))
     where
      r : g b â‰¡ (inr * , Î» ())
      r = ap (g' b) q 
    Ïˆ : (v : inl b â‰¢ inl b) â†’ i (inl b) â‰¡ inr v â†’ g (f (inr * , u)) â‰¡ (inr * , u)
    Ïˆ v q = ğŸ˜-elim (v refl)
  fg : f âˆ˜ g âˆ¼ id
  fg y = equality-cases (i (inl y)) Ï† Ïˆ
   where
    Ï† : (p : inl b â‰¡ inl y) â†’ i (inl y) â‰¡ inl p â†’ f (g' y (i (inl y))) â‰¡ y
    Ï† p q = ap (Î» d â†’ f (g' y d)) q âˆ™ inl-injective p
    Ïˆ : (u : inl b â‰¢ inl y) â†’ i (inl y) â‰¡ inr u â†’ f (g' y (i (inl y))) â‰¡ y
    Ïˆ _ = ap ((Î» d â†’ f (g' y d)))

add-one-and-remove-isolated-point {V} {Y} (inr *) _ = â‰ƒ-sym add-and-remove-same-point

+ğŸ™-cancellable : âˆ€ {U} {V} {X : U Ì‡} {Y : V Ì‡} â†’ (X + ğŸ™) â‰ƒ (Y + ğŸ™) â†’ X â‰ƒ Y
+ğŸ™-cancellable {U} {V} {X} {Y} (Ï† , e) =
   X                  â‰ƒâŸ¨ add-and-remove-same-point âŸ©
  (X + ğŸ™) âˆ– inr *     â‰ƒâŸ¨ remove-points Ï† (is-equiv-qinv Ï† e) (inr *) âŸ©
  (Y + ğŸ™) âˆ– Ï† (inr *) â‰ƒâŸ¨ add-one-and-remove-isolated-point
                              (Ï† (inr *))
                              (equivalences-preserve-isolatedness Ï† e (inr *) isolated-added-point) âŸ©
   Y â–  

\end{code}

\begin{code}

infix 2 _âˆ–_

\end{code}
