\begin{code}

{-# OPTIONS --without-K --exact-split --safe #-}

open import SpartanMLTT
open import UF-FunExt
open import Escardo-Simpson-LICS2001
open import UF-PropTrunc
open import OrderedIntervalObject

module RealisabilityMid
 (ğ“¤ : Universe)
 (fe : FunExt)
 (io : Interval-object fe ğ“¤)
 (hd : has-double fe ğ“¤ io)
 (pt : propositional-truncations-exist)
 (or : is-ordered fe pt io)
 where

open import UF-Base
-- open import GenericConvergentSequence
-- open import CoNaturals
-- open import Codistance fe
-- open import Ultracometrics fe
open import DiscreteAndSeparated
open import Sequence fe
-- open import NaturalsOrder renaming (_<_ to _<â„•_; _â‰¤_ to _â‰¤â„•_)
open import NaturalsAddition renaming (_+_ to _+â„•_)
open import UF-Subsingletons
-- open import UF-Subsingletons-FunExt

open basic-interval-object-development fe io hd

-- Define the code types

data ğŸ› : ğ“¤â‚€ Ì‡ where
  â‚ƒâ° â‚ƒâºÂ¹ â‚ƒâ»Â¹ : ğŸ›

ğŸ›á´º : ğ“¤â‚€ Ì‡
ğŸ›á´º = â„• â†’ ğŸ›

ğŸ›-is-discrete : is-discrete ğŸ›
ğŸ›-is-discrete â‚ƒâ°  â‚ƒâ°  = inl refl
ğŸ›-is-discrete â‚ƒâ°  â‚ƒâºÂ¹ = inr (Î» ())
ğŸ›-is-discrete â‚ƒâ°  â‚ƒâ»Â¹ = inr (Î» ())
ğŸ›-is-discrete â‚ƒâºÂ¹ â‚ƒâ°  = inr (Î» ())
ğŸ›-is-discrete â‚ƒâºÂ¹ â‚ƒâºÂ¹ = inl refl
ğŸ›-is-discrete â‚ƒâºÂ¹ â‚ƒâ»Â¹ = inr (Î» ())
ğŸ›-is-discrete â‚ƒâ»Â¹ â‚ƒâ°  = inr (Î» ())
ğŸ›-is-discrete â‚ƒâ»Â¹ â‚ƒâºÂ¹ = inr (Î» ())
ğŸ›-is-discrete â‚ƒâ»Â¹ â‚ƒâ»Â¹ = inl refl

-- Define the realisability map

q : ğŸ› â†’ ğ•€
q â‚ƒâ»Â¹ = âˆ’1
q â‚ƒâ°  =  O
q â‚ƒâºÂ¹ = +1

ğ•¢ : ğŸ›á´º â†’ ğ•€
ğ•¢ Î± = M (Î» n â†’ q (Î± n))

neg : ğŸ› â†’ ğŸ›
neg â‚ƒâ»Â¹ = â‚ƒâºÂ¹
neg  â‚ƒâ° = â‚ƒâ°
neg â‚ƒâºÂ¹ = â‚ƒâ»Â¹

zip : {X : ğ“¥ Ì‡ } {Y : ğ“¦ Ì‡ } â†’ (X â†’ Y) â†’ (â„• â†’ X) â†’ (â„• â†’ Y)
zip f Î± n = f (Î± n)

_realisesÂ²_ : (ğŸ›á´º â†’ ğŸ›á´º â†’ ğŸ›á´º) â†’ (ğ•€ â†’ ğ•€ â†’ ğ•€) â†’ ğ“¤ Ì‡
_*Â³_ realisesÂ² _*á´µ_ = Î  Î± ê‰ ğŸ›á´º , Î  Î² ê‰ ğŸ›á´º , (ğ•¢ (Î± *Â³ Î²) â‰¡ ğ•¢ Î± *á´µ ğ•¢ Î²)

_realisesÂ¹_ : (ğŸ›á´º â†’ ğŸ›á´º) â†’ (ğ•€ â†’ ğ•€) â†’ ğ“¤ Ì‡
fÂ³ realisesÂ¹ fá´µ = Î  Î± ê‰ ğŸ›á´º , (ğ•¢ (fÂ³ Î±) â‰¡ fá´µ (ğ•¢ Î±))

âˆ’-real' : (h : ğŸ›) â†’ q (neg h) â‰¡ âˆ’ q h
âˆ’-real' â‚ƒâ»Â¹ = âˆ’1-inverse â»Â¹
âˆ’-real' â‚ƒâ°  = O-inverse â»Â¹
âˆ’-real' â‚ƒâºÂ¹ = +1-inverse â»Â¹

ğ•¢-map : (fÂ³ : ğŸ› â†’ ğŸ›) (fá´µ : ğ•€ â†’ ğ•€)
      â†’ is-âŠ•-homomorphism fe ğ“˜ ğ“˜ fá´µ
      â†’ ((h : ğŸ›) â†’ q (fÂ³ h) â‰¡ fá´µ (q h))
      â†’ (zip fÂ³) realisesÂ¹ fá´µ
ğ•¢-map fÂ³ fá´µ h g Î± = ap M (dfunext (fe ğ“¤â‚€ ğ“¤) (Î» n â†’ g (Î± n)))
                  âˆ™ âŠ•-homs-are-M-homs fá´µ h (Î» n â†’ q (Î± n)) â»Â¹

âˆ’-real : (zip neg) realisesÂ¹ âˆ’_
âˆ’-real = ğ•¢-map neg âˆ’_ âˆ’-is-âŠ•-homomorphism âˆ’-real'

id-realises-id : id realisesÂ¹ id
id-realises-id Î± = refl

-- Show that midpoint and multiplication have realisers

-- mid-realisability : mid realisesÂ² _âŠ•_
-- mid-realisability Î± Î² = {!!}

data ğŸ : ğ“¤â‚€ Ì‡ where
 âˆ’2' âˆ’1' O' +1' +2' : ğŸ

ğŸá´º : ğ“¤â‚€ Ì‡
ğŸá´º = â„• â†’ ğŸ

add2' : ğŸ› â†’ ğŸ› â†’ ğŸ
add2' â‚ƒâ»Â¹ â‚ƒâ»Â¹ = âˆ’2'
add2' â‚ƒâ»Â¹ â‚ƒâ°  = âˆ’1'  
add2' â‚ƒâ»Â¹ â‚ƒâºÂ¹ = O'
add2' â‚ƒâ°  â‚ƒâ»Â¹ = âˆ’1'
add2' â‚ƒâºÂ¹ â‚ƒâ»Â¹ = O'
add2' â‚ƒâ°  â‚ƒâ°  = O'
add2' â‚ƒâ°  â‚ƒâºÂ¹ = +1'
add2' â‚ƒâºÂ¹ â‚ƒâ°  = +1'
add2' â‚ƒâºÂ¹ â‚ƒâºÂ¹ = +2'

add2 : ğŸ›á´º â†’ ğŸ›á´º â†’ ğŸá´º
add2 x y n = add2' (x n) (y n)

half : ğŸ â†’ ğ•€
half âˆ’2' = âˆ’1
half âˆ’1' = âˆ’1 /2
half  O' =  O
half +1' = +1 /2
half +2' = +1

half-real : Î  Î± ê‰ ğŸ›á´º , Î  Î² ê‰ ğŸ›á´º , (M (zip half (add2 Î± Î²)) â‰¡ ğ•¢ Î± âŠ• ğ•¢ Î²)
half-real Î± Î² = ap M (dfunext (fe ğ“¤â‚€ ğ“¤) (Î» i â†’ Î³ (Î± i) (Î² i)))
              âˆ™ M-hom (Î» n â†’ q (Î± n)) (Î» n â†’ q (Î² n)) â»Â¹
 where
   Î³ : (h h' : ğŸ›) â†’ half (add2' h h') â‰¡ (q h âŠ• q h')
   Î³ â‚ƒâ»Â¹ â‚ƒâ»Â¹ = âŠ•-idem â»Â¹
   Î³ â‚ƒâ»Â¹ â‚ƒâ°  = refl
   Î³ â‚ƒâ»Â¹ â‚ƒâºÂ¹ = refl
   Î³ â‚ƒâ°  â‚ƒâ»Â¹ = âŠ•-comm
   Î³ â‚ƒâºÂ¹ â‚ƒâ»Â¹ = âŠ•-comm
   Î³ â‚ƒâ°  â‚ƒâ°  = âŠ•-idem â»Â¹
   Î³ â‚ƒâ°  â‚ƒâºÂ¹ = âŠ•-comm
   Î³ â‚ƒâºÂ¹ â‚ƒâ°  = refl
   Î³ â‚ƒâºÂ¹ â‚ƒâºÂ¹ = âŠ•-idem â»Â¹

div2 : ğŸá´º â†’ ğŸ›á´º

Î´c : ğŸ â†’ ğŸá´º â†’ ğŸ›á´º
Î´c âˆ’2' Î± 0 = â‚ƒâ°
Î´c âˆ’2' Î± 1 = â‚ƒâ°
Î´c âˆ’2' Î± (succ (succ n)) = div2 (tail (tail Î±)) n
Î´c  O' Î± 0 = â‚ƒâ°
Î´c  O' Î± 1 = â‚ƒâºÂ¹
Î´c  O' Î± (succ (succ n)) = div2 (tail (tail Î±)) n
Î´c +2' Î± 0 = â‚ƒâºÂ¹
Î´c +2' Î± 1 = â‚ƒâ°
Î´c +2' Î± (succ (succ n)) = div2 (tail (tail Î±)) n
Î´c âˆ’1' Î± 0 = â‚ƒâ°
Î´c âˆ’1' Î± (succ n) = div2 (+1' âˆ¶âˆ¶ tail Î±) n
Î´c +1' Î± 0 = â‚ƒâºÂ¹
Î´c +1' Î± (succ n) = div2 (âˆ’1' âˆ¶âˆ¶ tail Î±) n    

Î´b : ğŸ â†’ ğŸá´º â†’ ğŸ›á´º
Î´b âˆ’2' _ 0 = â‚ƒâ»Â¹
Î´b âˆ’2' _ 1 = â‚ƒâ°
Î´b âˆ’2' Î± (succ (succ n)) = div2 (tail (tail Î±)) n
Î´b  O' _ 0 = â‚ƒâ°
Î´b  O' _ 1 = â‚ƒâ»Â¹
Î´b  O' Î± (succ (succ n)) = div2 (tail (tail Î±)) n
Î´b +2' _ 0 = â‚ƒâ°
Î´b +2' _ 1 = â‚ƒâ°
Î´b +2' Î± (succ (succ n)) = div2 (tail (tail Î±)) n
Î´b âˆ’1' _ 0 = â‚ƒâ»Â¹
Î´b âˆ’1' Î± (succ n) = div2 (+1' âˆ¶âˆ¶ tail Î±) n
Î´b +1' _ 0 = â‚ƒâ°
Î´b +1' Î± (succ n) = div2 (âˆ’1' âˆ¶âˆ¶ tail Î±) n

Î³a : ğŸ â†’ ğŸá´º â†’ ğŸ›á´º
Î³a âˆ’2' _ 0 = â‚ƒâ»Â¹
Î³a  O' _ 0 = â‚ƒâ°
Î³a +2' _ 0 = â‚ƒâºÂ¹
Î³a âˆ’2' Î± (succ n) = div2 (tail Î±) n
Î³a  O' Î± (succ n) = div2 (tail Î±) n
Î³a +2' Î± (succ n) = div2 (tail Î±) n
Î³a âˆ’1' Î± = Î´b (Î± 1) Î±
Î³a +1' Î± = Î´c (Î± 1) Î±

div2 Î± = Î³a (Î± 0) Î±
  
mid : ğŸ›á´º â†’ ğŸ›á´º â†’ ğŸ›á´º
mid Î± Î² = div2 (add2 Î± Î²)

{-
transportâ‚ : (h : ğŸ) (Î± : ğŸá´º) â†’ M (Î» n â†’ q (Î³a h Î± n)) â‰¡ M (Î» n â†’ q (Î³a h (Î± 0 âˆ¶âˆ¶ tail Î±) n))
transportâ‚ h Î± = ap (Î» - â†’ M (Î» n â†’ q (Î³a h - n))) (dfunext (fe ğ“¤â‚€ ğ“¤â‚€) Î³) where
  Î³ : Î± âˆ¼ (Î± 0 âˆ¶âˆ¶ tail Î±)
  Î³ 0 = refl
  Î³ (succ i) = refl

mid-div' : (h : ğŸ) (Î± : ğŸá´º) (i : â„•) â†’ M (Î» n â†’ q (Î³a h (h âˆ¶âˆ¶ Î±) (n +â„• i))) â‰¡ M (Î» n â†’ zip half (h âˆ¶âˆ¶ Î±) (n +â„• i))
mid-div' âˆ’2' Î± zero = M-propâ‚ (Î» n â†’ q (Î³a âˆ’2' (âˆ’2' âˆ¶âˆ¶ Î±) (n +â„• zero))) âˆ™ {!!} âˆ™ M-propâ‚ (Î» n â†’ zip half (âˆ’2' âˆ¶âˆ¶ Î±) (n +â„• zero)) â»Â¹
mid-div' âˆ’2' Î± (succ i) = {!!}
mid-div' âˆ’1' Î± i = {!!}
mid-div' O' Î± i = {!!}
mid-div' +1' Î± i = {!!}
mid-div' +2' Î± i = {!!}

mid-div : (h : ğŸ) (Î± : ğŸá´º) â†’ ğ•¢ (div2 Î±) â‰¡ M (zip half Î±) â†’ ğ•¢ (div2 (h âˆ¶âˆ¶ Î±)) â‰¡ M (zip half (h âˆ¶âˆ¶ Î±))
mid-div âˆ’2' Î± e = M-propâ‚ (Î» n â†’ q (div2 (âˆ’2' âˆ¶âˆ¶ Î±) n)) âˆ™ ap (u âŠ•_) e âˆ™ M-propâ‚ (zip half (âˆ’2' âˆ¶âˆ¶ Î±)) â»Â¹
mid-div âˆ’1' Î± e = {!!}
mid-div  O' Î± e = M-propâ‚ (Î» n â†’ q (div2 (O' âˆ¶âˆ¶ Î±) n)) âˆ™ ap (O âŠ•_) e âˆ™ M-propâ‚ (zip half (O' âˆ¶âˆ¶ Î±)) â»Â¹
mid-div +1' Î± e = {!!}
mid-div +2' Î± e = M-propâ‚ (Î» n â†’ q (div2 (+2' âˆ¶âˆ¶ Î±) n)) âˆ™ ap (v âŠ•_) e âˆ™ M-propâ‚ (zip half (+2' âˆ¶âˆ¶ Î±)) â»Â¹
-}

mid-realisability : mid realisesÂ² _âŠ•_
mid-realisability Î± Î² = Î³ (add2 Î± Î²) âˆ™ half-real Î± Î²
 where
  Î³ : (Î± : ğŸá´º) â†’ ğ•¢ (div2 Î±) â‰¡ M (zip half Î±)
  Î³ Î± = {!!}

data Vec (A : ğ“¥ Ì‡) : â„• â†’ ğ“¥ Ì‡ where
  [] : Vec A 0
  _âˆ·_ : âˆ€ {n} â†’ A â†’ Vec A n â†’ Vec A (succ n)

_++_ : {A : ğ“¥ Ì‡} {n : â„•} â†’ Vec A n â†’ (â„• â†’ A) â†’ â„• â†’ A
[] ++ s = s
(x âˆ· v) ++ s = x âˆ¶âˆ¶ (v ++ s)

first-_ : {A : ğ“¥ Ì‡ } (n : â„•) â†’ (â„• â†’ A) â†’ Vec A n
(first- 0) a = []
(first- succ n) a = head a âˆ· (first- n) (tail a)

affine-âŠ•-l : (x a b y : ğ•€) â†’ x âŠ• affine a b y â‰¡ affine (x âŠ• a) (x âŠ• b) y
affine-âŠ•-l x a b y = affine-uniquenessÂ· (Î» y â†’ x âŠ• affine a b y) (x âŠ• a) (x âŠ• b)
                         (ap (x âŠ•_) (affine-equation-l a b))
                         (ap (x âŠ•_) (affine-equation-r a b))
                         (Î» z y â†’
                           (ap (x âŠ•_) (affine-is-âŠ•-homomorphism a b z y))
                           âˆ™ ap (_âŠ• (affine a b z âŠ• affine a b y)) (âŠ•-idem â»Â¹)
                           âˆ™ âŠ•-tran)
                         y â»Â¹

open is-ordered or hiding (M)

ğ•€-induction : (P : ğ•€ â†’ ğ“¥ Ì‡ )
            â†’ ((x : ğ•€) â†’ is-prop (P x))
            â†’ P u
            â†’ ((a : â„• â†’ ğ•€) â†’ ((n : â„•) â†’ P (a n)) â†’ P (M a))
            â†’ P v
            â†’ (x : ğ•€) â†’ P x
             
â‰¤-affine : (a b i : ğ•€) â†’ a â‰¤ b â†’ a â‰¤ affine a b i Ã— affine a b i â‰¤ b
â‰¤-affine a b i aâ‰¤b = ğ•€-induction (Î» i â†’ a â‰¤ affine a b i) (Î» _ â†’ â‰¤-prop-valued)
                       (transport (a â‰¤_) (affine-equation-l a b â»Â¹) <-irreflexive)
                       (Î» Î± f â†’ transport (a â‰¤_)
                                  (âŠ•-homs-are-M-homs
                                    (affine a b) (affine-is-âŠ•-homomorphism a b) Î± â»Â¹)
                                (â‰¤-âŠ•â‚˜ f))
                       (transport (a â‰¤_) (affine-equation-r a b â»Â¹) aâ‰¤b)
                       i
                   , ğ•€-induction (Î» i â†’ affine a b i â‰¤ b) (Î» _ â†’ â‰¤-prop-valued)
                       (transport (_â‰¤ b) (affine-equation-l a b â»Â¹) aâ‰¤b)
                       (Î» Î± f â†’ transport (_â‰¤ b)
                                  (âŠ•-homs-are-M-homs
                                    (affine a b) (affine-is-âŠ•-homomorphism a b) Î± â»Â¹)
                                (â‰¤-âŠ•â‚˜' f))
                       (transport (_â‰¤ b) (affine-equation-r a b â»Â¹) <-irreflexive)
                       i
                       
M-seq-eq : (a b : ğ•€) â†’ a â‰¤ b
         â†’ (i : ğ•€) (Î± : â„• â†’ ğ•€)
         â†’ Î£ c ê‰ ğ•€ , Î£ d ê‰ ğ•€ ,
           (a â‰¤ c)
         Ã— (c â‰¤ d)
         Ã— (d â‰¤ b)
         Ã— (affine a b (M (i âˆ¶âˆ¶ Î±)) â‰¡ affine c d (M Î±))
M-seq-eq a b aâ‰¤b i Î± = c , d , aâ‰¤c , câ‰¤d , dâ‰¤b , Î³
 where
  c = affine a b i âŠ• a
  d = affine a b i âŠ• b
  aâ‰¤c : a â‰¤ c
  aâ‰¤c = transport (_â‰¤ c) âŠ•-idem (â‰¤-âŠ•â‚‚ (prâ‚ (â‰¤-affine a b i aâ‰¤b)) <-irreflexive)
  câ‰¤d = â‰¤-âŠ•â‚‚ <-irreflexive aâ‰¤b
  dâ‰¤b = transport (d â‰¤_) âŠ•-idem (â‰¤-âŠ•â‚‚ (prâ‚‚ (â‰¤-affine a b i aâ‰¤b)) <-irreflexive)
  Î³ = ap (affine a b) (M-propâ‚ (i âˆ¶âˆ¶ Î±))
    âˆ™ affine-is-âŠ•-homomorphism a b i (M Î±)
    âˆ™ affine-âŠ•-l (affine a b i) a b (M Î±)

tail-_ : {A : ğ“¥ Ì‡ } (n : â„•) â†’ (â„• â†’ A) â†’ (â„• â†’ A)
(tail- 0) Î± = Î±
(tail- succ n) Î± = (tail- n) (tail Î±)

increasing decreasing : (â„• â†’ ğ•€) â†’ ğ“¤â‚€ Ì‡
increasing Î± = (n : â„•) â†’ Î± n        â‰¤ Î± (succ n)
decreasing Î± = (n : â„•) â†’ Î± (succ n) â‰¤ Î± n


M-thing : (a b : ğ•€) â†’ a â‰¤ b â†’ {n : â„•}
          â†’ (v : Vec ğ•€ n) (Î± : â„• â†’ ğ•€)
          â†’ Î£ c ê‰ ğ•€ , Î£ d ê‰ ğ•€ ,
            (a â‰¤ c)
          Ã— (c â‰¤ d)
          Ã— (d â‰¤ b)
          Ã— (affine a b (M (v ++ Î±)) â‰¡ affine c d (M Î±))
M-thing a b aâ‰¤b [] Î± = a , b , â‰¤-reflexive , aâ‰¤b , â‰¤-reflexive , refl
M-thing a b aâ‰¤b (x âˆ· v) Î± = IHc , IHd , â‰¤-trans Haâ‰¤c IHaâ‰¤c , IHcâ‰¤d , â‰¤-trans IHdâ‰¤b Hdâ‰¤b
                            , (HÎ³ âˆ™ IHÎ³)
 where
  H = M-seq-eq a b aâ‰¤b x (v ++ Î±)
  Hc   = prâ‚ H
  Hd   = prâ‚ (prâ‚‚ H)
  Haâ‰¤c = prâ‚ (prâ‚‚ (prâ‚‚ H))
  Hcâ‰¤d = prâ‚ (prâ‚‚ (prâ‚‚ (prâ‚‚ H)))
  Hdâ‰¤b = prâ‚ (prâ‚‚ (prâ‚‚ (prâ‚‚ (prâ‚‚ H))))
  HÎ³ : affine a b (M (x âˆ¶âˆ¶ (v ++ Î±))) â‰¡
         affine (prâ‚ H) (prâ‚ (prâ‚‚ H)) (M (v ++ Î±))
  HÎ³   = prâ‚‚ (prâ‚‚ (prâ‚‚ (prâ‚‚ (prâ‚‚ H))))
  IH = M-thing Hc Hd Hcâ‰¤d v Î±
  IHc   = prâ‚ IH
  IHd   = prâ‚ (prâ‚‚ IH)
  IHaâ‰¤c = prâ‚ (prâ‚‚ (prâ‚‚ IH))
  IHcâ‰¤d = prâ‚ (prâ‚‚ (prâ‚‚ (prâ‚‚ IH)))
  IHdâ‰¤b = prâ‚ (prâ‚‚ (prâ‚‚ (prâ‚‚ (prâ‚‚ IH))))
  IHÎ³ : affine Hc Hd (M (v ++ Î±)) â‰¡ affine (prâ‚ IH) (prâ‚ (prâ‚‚ IH)) (M Î±)
  IHÎ³   = prâ‚‚ (prâ‚‚ (prâ‚‚ (prâ‚‚ (prâ‚‚ IH))))

first-tail-eq : {A : ğ“¥ Ì‡ } (n : â„•) (Î± : â„• â†’ A) â†’ ((first- n) Î± ++ (tail- n) Î±) â‰¡ Î±
first-tail-eq 0 Î± = refl
first-tail-eq {ğ“¥} (succ n) Î± = dfunext (fe ğ“¤â‚€ ğ“¥) Î³ where
  Î³ : ((first- succ n) Î± ++ (tail- succ n) Î±) âˆ¼ Î±
  Î³ 0 = refl
  Î³ (succ i) = happly (first-tail-eq n (tail Î±)) i 

M-seq-inf : (a b : ğ•€) â†’ a â‰¤ b
          â†’ (Î± : â„• â†’ ğ•€)
          â†’ Î£ cs ê‰ (â„• â†’ ğ•€) , Î£ ds ê‰ (â„• â†’ ğ•€) ,
            increasing cs Ã— decreasing ds
          Ã— ((n : â„•)
          â†’ affine a      b      (M Î±)
          â‰¡ affine (cs n) (ds n) (M ((tail- n) Î±)))
M-seq-inf a b aâ‰¤b Î± = cs , ds , csâ‰¤cs , dsâ‰¤ds , Î³ -- cs , ds , {!!} , {!!} , Î³
 where
  IH = Î» n â†’ M-thing a b aâ‰¤b ((first- n) Î±) ((tail- n) Î±) 
  cs = Î» n â†’ prâ‚ (IH n)
  ds = Î» n â†’ prâ‚ (prâ‚‚ (IH n))
  Î³ : (n : â„•) â†’ affine a b (M Î±) â‰¡ affine (cs n) (ds n) (M ((tail- n) Î±))
  Î³ n = transport
          (Î» - â†’ affine a b (M -) â‰¡ affine (cs n) (ds n) (M ((tail- n) Î±)))
          (first-tail-eq n Î±)
          (prâ‚‚ (prâ‚‚ (prâ‚‚ (prâ‚‚ (prâ‚‚ (IH n))))))
  csâ‰¤cs : increasing cs
  csâ‰¤cs n = {!!}
  dsâ‰¤ds : decreasing ds
  dsâ‰¤ds = {!!}
  IHâ‚‚ : (h : ğ•€) (n : â„•) â†’ affine (cs n) (ds n) (M ({!!} âˆ¶âˆ¶ (tail- n) Î±))
                â‰¡ affine (cs (succ n)) (ds (succ n)) (M ((tail- n) Î±))
  IHâ‚‚ n = {!!}
  
ğ•€-induction = {!!}
