Martin Escardo

The two-point type is defined, together with its induction principle,
in the module SpartanMLTT. Here we develop some general machinery.

\begin{code}

{-# OPTIONS --without-K --exact-split --safe #-}

module Two-Properties where

open import SpartanMLTT
open import Unit-Properties

ğŸš-Cases : {A : ğ“¤ Ì‡ } â†’ ğŸš â†’ A â†’ A â†’ A
ğŸš-Cases a b c = ğŸš-cases b c a

ğŸš-equality-cases : {A : ğ“¤ Ì‡ } {b : ğŸš} â†’ (b â‰¡ â‚€ â†’ A) â†’ (b â‰¡ â‚ â†’ A) â†’ A
ğŸš-equality-cases {ğ“¤} {A} {â‚€} fâ‚€ fâ‚ = fâ‚€ refl
ğŸš-equality-cases {ğ“¤} {A} {â‚} fâ‚€ fâ‚ = fâ‚ refl

ğŸš-equality-casesâ‚€ : {A : ğ“¤ Ì‡ } {b : ğŸš} {fâ‚€ : b â‰¡ â‚€ â†’ A} {fâ‚ : b â‰¡ â‚ â†’ A}
                  â†’ (p : b â‰¡ â‚€) â†’ ğŸš-equality-cases {ğ“¤} {A} {b} fâ‚€ fâ‚ â‰¡ fâ‚€ p
ğŸš-equality-casesâ‚€ {ğ“¤} {A} {.â‚€} refl = refl

ğŸš-equality-casesâ‚ : {A : ğ“¤ Ì‡ } {b : ğŸš} {fâ‚€ : b â‰¡ â‚€ â†’ A} {fâ‚ : b â‰¡ â‚ â†’ A}
                  â†’ (p : b â‰¡ â‚) â†’ ğŸš-equality-cases {ğ“¤} {A} {b} fâ‚€ fâ‚ â‰¡ fâ‚ p
ğŸš-equality-casesâ‚ {ğ“¤} {A} {.â‚} refl = refl

ğŸš-equality-cases' : {Aâ‚€ Aâ‚ : ğ“¤ Ì‡ } {b : ğŸš} â†’ (b â‰¡ â‚€ â†’ Aâ‚€) â†’ (b â‰¡ â‚ â†’ Aâ‚) â†’ Aâ‚€ + Aâ‚
ğŸš-equality-cases' {ğ“¤} {Aâ‚€} {Aâ‚} {â‚€} fâ‚€ fâ‚ = inl (fâ‚€ refl)
ğŸš-equality-cases' {ğ“¤} {Aâ‚€} {Aâ‚} {â‚} fâ‚€ fâ‚ = inr (fâ‚ refl)

ğŸš-possibilities : (b : ğŸš) â†’ (b â‰¡ â‚€) + (b â‰¡ â‚)
ğŸš-possibilities â‚€ = inl refl
ğŸš-possibilities â‚ = inr refl


ğŸš-excluded-third : (b : ğŸš) â†’ b â‰¢ â‚€ â†’ b â‰¢ â‚ â†’ ğŸ˜ {ğ“¤â‚€}
ğŸš-excluded-third â‚€ u v = u refl
ğŸš-excluded-third â‚ u v = v refl

ğŸš-things-distinct-from-a-third-are-equal : (x y z : ğŸš) â†’ x â‰¢ z â†’ y â‰¢ z â†’ x â‰¡ y
ğŸš-things-distinct-from-a-third-are-equal â‚€ â‚€ z u v = refl
ğŸš-things-distinct-from-a-third-are-equal â‚€ â‚ z u v = ğŸ˜-elim (ğŸš-excluded-third z (â‰¢-sym u) (â‰¢-sym v))
ğŸš-things-distinct-from-a-third-are-equal â‚ â‚€ z u v = ğŸ˜-elim (ğŸš-excluded-third z (â‰¢-sym v) (â‰¢-sym u))
ğŸš-things-distinct-from-a-third-are-equal â‚ â‚ z u v = refl

one-is-not-zero : â‚ â‰¢ â‚€
one-is-not-zero p = ğŸ™-is-not-ğŸ˜ q
 where
  f : ğŸš â†’ ğ“¤â‚€ Ì‡
  f â‚€ = ğŸ˜
  f â‚ = ğŸ™

  q : ğŸ™ â‰¡ ğŸ˜
  q = ap f p

zero-is-not-one : â‚€ â‰¢ â‚
zero-is-not-one p = one-is-not-zero (p â»Â¹)

equal-â‚-different-from-â‚€ : {b : ğŸš} â†’ b â‰¡ â‚ â†’ b â‰¢ â‚€
equal-â‚-different-from-â‚€ r s = zero-is-not-one (s â»Â¹ âˆ™ r)

different-from-â‚€-equal-â‚ : {b : ğŸš} â†’ b â‰¢ â‚€ â†’ b â‰¡ â‚
different-from-â‚€-equal-â‚ f = ğŸš-equality-cases (ğŸ˜-elim âˆ˜ f) (Î» r â†’ r)

different-from-â‚-equal-â‚€ : {b : ğŸš} â†’ b â‰¢ â‚ â†’ b â‰¡ â‚€
different-from-â‚-equal-â‚€ f = ğŸš-equality-cases (Î» r â†’ r) (ğŸ˜-elim âˆ˜ f)

equal-â‚€-different-from-â‚ : {b : ğŸš} â†’ b â‰¡ â‚€ â†’ b â‰¢ â‚
equal-â‚€-different-from-â‚ r s = zero-is-not-one (r â»Â¹ âˆ™ s)

[aâ‰¡â‚â†’bâ‰¡â‚]-gives-[bâ‰¡â‚€â†’aâ‰¡â‚€] : {a b : ğŸš} â†’ (a â‰¡ â‚ â†’ b â‰¡ â‚) â†’ b â‰¡ â‚€ â†’ a â‰¡ â‚€
[aâ‰¡â‚â†’bâ‰¡â‚]-gives-[bâ‰¡â‚€â†’aâ‰¡â‚€] f = different-from-â‚-equal-â‚€ âˆ˜ (contrapositive f) âˆ˜ equal-â‚€-different-from-â‚

[aâ‰¡â‚€â†’bâ‰¡â‚€]-gives-[bâ‰¡â‚â†’aâ‰¡â‚] : {a b : ğŸš} â†’ (a â‰¡ â‚€ â†’ b â‰¡ â‚€) â†’ b â‰¡ â‚ â†’ a â‰¡ â‚
[aâ‰¡â‚€â†’bâ‰¡â‚€]-gives-[bâ‰¡â‚â†’aâ‰¡â‚] f = different-from-â‚€-equal-â‚ âˆ˜ (contrapositive f) âˆ˜ equal-â‚-different-from-â‚€

\end{code}

ğŸš-Characteristic function of equality on ğŸš:

\begin{code}

complement : ğŸš â†’ ğŸš
complement â‚€ = â‚
complement â‚ = â‚€

complement-no-fp : (n : ğŸš) â†’ n â‰¡ complement n â†’ ğŸ˜ {ğ“¤}
complement-no-fp â‚€ p = ğŸ˜-elim (zero-is-not-one p)
complement-no-fp â‚ p = ğŸ˜-elim (one-is-not-zero p)

complement-involutive : (b : ğŸš) â†’ complement (complement b) â‰¡ b
complement-involutive â‚€ = refl
complement-involutive â‚ = refl

eqğŸš : ğŸš â†’ ğŸš â†’ ğŸš
eqğŸš â‚€ n = complement n
eqğŸš â‚ n = n

eqğŸš-equal : (m n : ğŸš) â†’ eqğŸš m n â‰¡ â‚ â†’ m â‰¡ n
eqğŸš-equal â‚€ n p = ap complement (p â»Â¹) âˆ™ complement-involutive n
eqğŸš-equal â‚ n p = p â»Â¹

equal-eqğŸš : (m n : ğŸš) â†’ m â‰¡ n â†’ eqğŸš m n â‰¡ â‚
equal-eqğŸš â‚€ â‚€ refl = refl
equal-eqğŸš â‚ â‚ refl = refl

\end{code}

Natural order of binary numbers:

\begin{code}

_<â‚‚_ : (a b : ğŸš) â†’ ğ“¤â‚€ Ì‡
a <â‚‚ b = (a â‰¡ â‚€) Ã— (b â‰¡ â‚)

_â‰¤â‚‚_ : (a b : ğŸš) â†’ ğ“¤â‚€ Ì‡
a â‰¤â‚‚ b = a â‰¡ â‚ â†’ b â‰¡ â‚

<â‚‚-gives-â‰¤â‚‚ : {a b : ğŸš} â†’ a <â‚‚ b â†’ a â‰¤â‚‚ b
<â‚‚-gives-â‰¤â‚‚ (refl , refl) _ = refl

â‚-top : {b : ğŸš} â†’ b â‰¤â‚‚ â‚
â‚-top r = refl

â‚€-bottom : {b : ğŸš} â†’ â‚€ â‰¤â‚‚ b
â‚€-bottom {b} p = ğŸ˜-elim (zero-is-not-one p)

_â‰¤â‚‚'_ : (a b : ğŸš) â†’ ğ“¤â‚€ Ì‡
a â‰¤â‚‚' b = b â‰¡ â‚€ â†’ a â‰¡ â‚€

â‰¤â‚‚-gives-â‰¤â‚‚' : {a b : ğŸš} â†’ a â‰¤â‚‚ b â†’ a â‰¤â‚‚' b
â‰¤â‚‚-gives-â‰¤â‚‚' {â‚€} {b} f p = refl
â‰¤â‚‚-gives-â‰¤â‚‚' {â‚} {â‚€} f p = (f refl)â»Â¹
â‰¤â‚‚-gives-â‰¤â‚‚' {â‚} {â‚} f p = p

â‰¤â‚‚'-gives-â‰¤â‚‚ : {a b : ğŸš} â†’ a â‰¤â‚‚' b â†’ a â‰¤â‚‚ b
â‰¤â‚‚'-gives-â‰¤â‚‚ {â‚€} {â‚€} f p = p
â‰¤â‚‚'-gives-â‰¤â‚‚ {â‚€} {â‚} f p = refl
â‰¤â‚‚'-gives-â‰¤â‚‚ {â‚} {â‚€} f p = (f refl)â»Â¹
â‰¤â‚‚'-gives-â‰¤â‚‚ {â‚} {â‚} f p = p

â‰¤â‚‚-anti : {a b : ğŸš} â†’ a â‰¤â‚‚ b â†’ b â‰¤â‚‚ a â†’ a â‰¡ b
â‰¤â‚‚-anti {â‚€} {â‚€} f g = refl
â‰¤â‚‚-anti {â‚€} {â‚} f g = g refl
â‰¤â‚‚-anti {â‚} {â‚€} f g = â‰¤â‚‚-gives-â‰¤â‚‚' f refl
â‰¤â‚‚-anti {â‚} {â‚} f g = refl

â‚-maximal : {b : ğŸš} â†’ â‚ â‰¤â‚‚ b â†’ b â‰¡ â‚
â‚-maximal = â‰¤â‚‚-anti â‚-top

_â‰¥â‚‚_ : (a b : ğŸš) â†’ ğ“¤â‚€ Ì‡
a â‰¥â‚‚ b = b â‰¤â‚‚ a

minğŸš : ğŸš â†’ ğŸš â†’ ğŸš
minğŸš â‚€ b = â‚€
minğŸš â‚ b = b

Lemma[minabâ‰¤â‚‚a] : {a b : ğŸš} â†’ minğŸš a b â‰¤â‚‚ a
Lemma[minabâ‰¤â‚‚a] {â‚€} {b} r = ğŸ˜-elim (equal-â‚-different-from-â‚€ r refl)
Lemma[minabâ‰¤â‚‚a] {â‚} {b} r = refl

Lemma[minabâ‰¤â‚‚b] : {a b : ğŸš} â†’ minğŸš a b â‰¤â‚‚ b
Lemma[minabâ‰¤â‚‚b] {â‚€} {b} r = ğŸ˜-elim (equal-â‚-different-from-â‚€ r refl)
Lemma[minabâ‰¤â‚‚b] {â‚} {b} r = r

Lemma[minğŸšabâ‰¡â‚â†’bâ‰¡â‚] : {a b : ğŸš} â†’ minğŸš a b â‰¡ â‚ â†’ b â‰¡ â‚
Lemma[minğŸšabâ‰¡â‚â†’bâ‰¡â‚] {â‚€} {â‚€} r = r
Lemma[minğŸšabâ‰¡â‚â†’bâ‰¡â‚] {â‚€} {â‚} r = refl
Lemma[minğŸšabâ‰¡â‚â†’bâ‰¡â‚] {â‚} {â‚€} r = r
Lemma[minğŸšabâ‰¡â‚â†’bâ‰¡â‚] {â‚} {â‚} r = refl

Lemma[minğŸšabâ‰¡â‚â†’aâ‰¡â‚]  : {a b : ğŸš} â†’ minğŸš a b â‰¡ â‚ â†’ a â‰¡ â‚
Lemma[minğŸšabâ‰¡â‚â†’aâ‰¡â‚] {â‚€} r = r
Lemma[minğŸšabâ‰¡â‚â†’aâ‰¡â‚] {â‚} r = refl

Lemma[aâ‰¡â‚â†’bâ‰¡â‚â†’minğŸšabâ‰¡â‚] : {a b : ğŸš} â†’ a â‰¡ â‚ â†’ b â‰¡ â‚ â†’ minğŸš a b â‰¡ â‚
Lemma[aâ‰¡â‚â†’bâ‰¡â‚â†’minğŸšabâ‰¡â‚] {â‚€} {â‚€} p q = q
Lemma[aâ‰¡â‚â†’bâ‰¡â‚â†’minğŸšabâ‰¡â‚] {â‚€} {â‚} p q = p
Lemma[aâ‰¡â‚â†’bâ‰¡â‚â†’minğŸšabâ‰¡â‚] {â‚} {â‚€} p q = q
Lemma[aâ‰¡â‚â†’bâ‰¡â‚â†’minğŸšabâ‰¡â‚] {â‚} {â‚} p q = refl

Lemma[aâ‰¤â‚‚bâ†’minğŸšabâ‰¡a] : {a b : ğŸš} â†’ a â‰¤â‚‚ b â†’ minğŸš a b â‰¡ a
Lemma[aâ‰¤â‚‚bâ†’minğŸšabâ‰¡a] {â‚€} {b} p = refl
Lemma[aâ‰¤â‚‚bâ†’minğŸšabâ‰¡a] {â‚} {b} p = p refl

Lemma[minğŸšabâ‰¡â‚€] : {a b : ğŸš} â†’ (a â‰¡ â‚€) + (b â‰¡ â‚€) â†’ minğŸš a b â‰¡ â‚€
Lemma[minğŸšabâ‰¡â‚€] {â‚€} {b} (inl p) = refl
Lemma[minğŸšabâ‰¡â‚€] {â‚€} {â‚€} (inr q) = refl
Lemma[minğŸšabâ‰¡â‚€] {â‚} {â‚€} (inr q) = refl

lemma[minğŸšabâ‰¡â‚€] : {a b : ğŸš} â†’ minğŸš a b â‰¡ â‚€ â†’ (a â‰¡ â‚€) + (b â‰¡ â‚€)
lemma[minğŸšabâ‰¡â‚€] {â‚€} {b} p = inl p
lemma[minğŸšabâ‰¡â‚€] {â‚} {b} p = inr p

maxğŸš : ğŸš â†’ ğŸš â†’ ğŸš
maxğŸš â‚€ b = b
maxğŸš â‚ b = â‚

maxğŸš-lemma : (a b : ğŸš) â†’ maxğŸš a b â‰¡ â‚ â†’ (a â‰¡ â‚) + (b â‰¡ â‚)
maxğŸš-lemma â‚€ b r = inr r
maxğŸš-lemma â‚ b r = inl refl

maxğŸš-lemma-converse : (a b : ğŸš) â†’ (a â‰¡ â‚) + (b â‰¡ â‚) â†’ maxğŸš a b â‰¡ â‚
maxğŸš-lemma-converse â‚€ b (inl r) = unique-from-ğŸ˜ (zero-is-not-one r)
maxğŸš-lemma-converse â‚€ b (inr r) = r
maxğŸš-lemma-converse â‚ b x = refl

\end{code}

Addition modulo 2:

\begin{code}

_âŠ•_ : ğŸš â†’ ğŸš â†’ ğŸš
â‚€ âŠ• x = x
â‚ âŠ• x = complement x

complement-of-eqğŸš-is-âŠ• : (m n : ğŸš) â†’ complement (eqğŸš m n) â‰¡ m âŠ• n
complement-of-eqğŸš-is-âŠ• â‚€ n = complement-involutive n
complement-of-eqğŸš-is-âŠ• â‚ n = refl

Lemma[bâŠ•bâ‰¡â‚€] : {b : ğŸš} â†’ b âŠ• b â‰¡ â‚€
Lemma[bâŠ•bâ‰¡â‚€] {â‚€} = refl
Lemma[bâŠ•bâ‰¡â‚€] {â‚} = refl

Lemma[bâ‰¡câ†’bâŠ•câ‰¡â‚€] : {b c : ğŸš} â†’ b â‰¡ c â†’ b âŠ• c â‰¡ â‚€
Lemma[bâ‰¡câ†’bâŠ•câ‰¡â‚€] {b} {c} r = ap (Î» - â†’ b âŠ• -) (r â»Â¹) âˆ™ (Lemma[bâŠ•bâ‰¡â‚€] {b})

Lemma[bâŠ•câ‰¡â‚€â†’bâ‰¡c] : {b c : ğŸš} â†’ b âŠ• c â‰¡ â‚€ â†’ b â‰¡ c
Lemma[bâŠ•câ‰¡â‚€â†’bâ‰¡c] {â‚€} {â‚€} r = refl
Lemma[bâŠ•câ‰¡â‚€â†’bâ‰¡c] {â‚€} {â‚} r = r â»Â¹
Lemma[bâŠ•câ‰¡â‚€â†’bâ‰¡c] {â‚} {â‚€} r = r
Lemma[bâŠ•câ‰¡â‚€â†’bâ‰¡c] {â‚} {â‚} r = refl

Lemma[bâ‰¢câ†’bâŠ•câ‰¡â‚] : {b c : ğŸš} â†’ b â‰¢ c â†’ b âŠ• c â‰¡ â‚
Lemma[bâ‰¢câ†’bâŠ•câ‰¡â‚] = different-from-â‚€-equal-â‚ âˆ˜ (contrapositive Lemma[bâŠ•câ‰¡â‚€â†’bâ‰¡c])

Lemma[bâŠ•câ‰¡â‚â†’bâ‰¢c] : {b c : ğŸš} â†’ b âŠ• c â‰¡ â‚ â†’ b â‰¢ c
Lemma[bâŠ•câ‰¡â‚â†’bâ‰¢c] = (contrapositive Lemma[bâ‰¡câ†’bâŠ•câ‰¡â‚€]) âˆ˜ equal-â‚-different-from-â‚€

\end{code}

Order and complements:

\begin{code}

complement-left : {b c : ğŸš} â†’ complement b â‰¤â‚‚ c â†’ complement c â‰¤â‚‚ b
complement-left {â‚€} {â‚€} f p = f p
complement-left {â‚€} {â‚} f p = p
complement-left {â‚} {c} f p = refl

complement-right : {b c : ğŸš} â†’ b â‰¤â‚‚ complement c â†’ c â‰¤â‚‚ complement b
complement-right {â‚€} {c} f p = refl
complement-right {â‚} {â‚€} f p = p
complement-right {â‚} {â‚} f p = f p

complement-both-left : {b c : ğŸš} â†’ complement b â‰¤â‚‚ complement c â†’ c â‰¤â‚‚ b
complement-both-left {â‚€} {â‚€} f p = p
complement-both-left {â‚€} {â‚} f p = f p
complement-both-left {â‚} {c} f p = refl

complement-both-right : {b c : ğŸš} â†’ b â‰¤â‚‚ c â†’ complement c â‰¤â‚‚ complement b
complement-both-right {â‚€} {c} f p = refl
complement-both-right {â‚} {â‚€} f p = f p
complement-both-right {â‚} {â‚} f p = p

\end{code}

Fixities and precedences:

\begin{code}

infixr 31 _âŠ•_

\end{code}
