\begin{code}

{-# OPTIONS --without-K --exact-split #-}

module UF-Embedding where

open import SpartanMLTT
open import UF-Base
open import UF-Subsingletons
open import UF-Subsingletons-Equiv
open import UF-Equiv
open import UF-EquivalenceExamples
open import UF-LeftCancellable
open import UF-Yoneda
open import UF-Retracts
open import UF-FunExt
open import UF-Subsingletons-FunExt
open import UF-Univalence
open import UF-UA-FunExt

is-embedding : {X : U Ì‡} {Y : V Ì‡} â†’ (X â†’ Y) â†’ U âŠ” V Ì‡
is-embedding f = âˆ€ y â†’ is-prop(fiber f y)

is-embedding-is-prop : funext V (U âŠ” V) â†’ funext (U âŠ” V) (U âŠ” V)
                     â†’ {X : U Ì‡} {Y : V Ì‡} (f : X â†’ Y)
                     â†’ is-prop(is-embedding f)
is-embedding-is-prop {U} {V} fe fe' f = Î -is-prop
                                          fe
                                          (Î» x â†’ is-prop-is-a-prop fe')

embedding-criterion : {X : U Ì‡} {Y : V Ì‡} (f : X â†’ Y)
                    â†’ ((x : X) â†’ is-prop (fiber f (f x)))
                    â†’ is-embedding f
embedding-criterion f Ï† .(f x) (x , refl) = Ï† x (x , refl)

is-equiv-is-embedding : {X : U Ì‡} {Y : V Ì‡} (f : X â†’ Y)
                      â†’ is-equiv f â†’ is-embedding f
is-equiv-is-embedding f e y = singletons-are-propositions (equivs-are-vv-equivs f e y)

_â†ª_ : U Ì‡ â†’ V Ì‡ â†’ U âŠ” V Ì‡
X â†ª Y = Î£ \(f : X â†’ Y) â†’ is-embedding f

etofun : {X : U Ì‡} {Y : V Ì‡} â†’ (X â†ª Y) â†’ X â†’ Y
etofun = prâ‚

is-embedding-etofun : {X : U Ì‡} {Y : V Ì‡}
                    â†’ (e : X â†ª Y) â†’ is-embedding(etofun e)
is-embedding-etofun = prâ‚‚

equiv-embedding : {X : U Ì‡} {Y : V Ì‡}
               â†’ X â‰ƒ Y â†’ X â†ª Y
equiv-embedding e = eqtofun e ,
                    is-equiv-is-embedding
                     (eqtofun e)
                     (eqtofun-is-an-equiv e)

embedding-lc : {X : U Ì‡} {Y : V Ì‡} (f : X â†’ Y)
             â†’ is-embedding f â†’ left-cancellable f
embedding-lc f e {x} {x'} p = ap prâ‚ (e (f x) (x , refl) (x' , (p â»Â¹)))

is-embedding' : {X : U Ì‡} {Y : V Ì‡} â†’ (X â†’ Y) â†’ U âŠ” V Ì‡
is-embedding' f = âˆ€ x x' â†’ is-equiv (ap f {x} {x'})

embedding-embedding' : {X : U Ì‡} {Y : V Ì‡} (f : X â†’ Y)
                     â†’ is-embedding f â†’ is-embedding' f
embedding-embedding' {U} {V} {X} {Y} f ise = g
 where
  b : (x : X) â†’ is-singleton(fiber f (f x))
  b x = (x , refl) , ise (f x) (x , refl)
  c : (x : X) â†’ is-singleton(fiber' f (f x))
  c x = retract-of-singleton (prâ‚ (fiber-lemma f (f x)) , prâ‚(prâ‚‚(fiber-lemma f (f x)))) (b x)
  g : (x x' : X) â†’ is-equiv(ap f {x} {x'})
  g x = universality-equiv x refl (unique-element-is-universal-element
                                         (Î» x' â†’ f x â‰¡ f x')
                                         (prâ‚(c x))
                                         (prâ‚‚(c x)))

embedding'-embedding : {X : U Ì‡} {Y : V Ì‡} (f : X â†’ Y) â†’ is-embedding' f â†’ is-embedding f
embedding'-embedding {U} {V} {X} {Y} f ise = g
 where
  e : (x x' : X) â†’ is-the-only-element (x , refl)
  e x x' = universal-element-is-the-only-element
             (x , refl)
             (equiv-universality x refl (ise x))
  h : (x : X) â†’ is-prop (fiber' f (f x))
  h x Ïƒ Ï„ = Ïƒ â‰¡âŸ¨ (e x (prâ‚ Ïƒ) Ïƒ)â»Â¹ âŸ© (x , refl) â‰¡âŸ¨ e x (prâ‚ Ï„) Ï„ âŸ© Ï„ âˆ
  g' : (y : Y) â†’ is-prop (fiber' f y)
  g' y (x , p) = transport (Î» - â†’ is-prop (Î£ \(x' : X) â†’ - â‰¡ f x')) (p â»Â¹) (h x) (x , p)
  g : (y : Y) â†’ is-prop (fiber f y)
  g y = left-cancellable-reflects-is-prop
            (prâ‚ (fiber-lemma f y))
            (section-lc _ (prâ‚‚ (prâ‚‚ (fiber-lemma f y)))) (g' y)

prâ‚-embedding : {X : U Ì‡} {Y : X â†’ V Ì‡}
              â†’ ((x : X) â†’ is-prop(Y x))
              â†’ is-embedding (prâ‚ {U} {V} {X} {Y})
prâ‚-embedding f x ((.x , y') , refl) ((.x , y'') , refl) = g
 where
  g : (x , y') , refl â‰¡ (x , y'') , refl
  g = ap (Î» - â†’ (x , -) , refl) (f x y' y'')

prâ‚-lc-bis : {X : U Ì‡} {Y : X â†’ V Ì‡} â†’ ({x : X} â†’ is-prop(Y x)) â†’ left-cancellable prâ‚
prâ‚-lc-bis f {u} {v} r = embedding-lc prâ‚ (prâ‚-embedding (Î» x â†’ f {x})) r

prâ‚-embedding-converse : {X : U Ì‡} {Y : X â†’ V Ì‡}
                       â†’ is-embedding (prâ‚ {U} {V} {X} {Y})
                       â†’ ((x : X) â†’ is-prop(Y x))
prâ‚-embedding-converse {U} {V} {X} {Y} ie x = h
  where
    e : Î£ Y â†’ X
    e = prâ‚ {U} {V} {X} {Y}
    isp : is-prop(fiber e x)
    isp = ie x
    s : Y x â†’ fiber e x
    s y = (x , y) , refl
    r : fiber e x â†’ Y x
    r ((x , y) , refl) = y
    rs : (y : Y x) â†’ r(s y) â‰¡ y
    rs y = refl
    h : is-prop(Y x)
    h = left-cancellable-reflects-is-prop s (section-lc s (r , rs)) isp

K-idtofun-lc : K (U âº) â†’ {X : U Ì‡} (x y : X) (A : X â†’ U Ì‡)
             â†’ left-cancellable(idtofun (Id x y) (A y))
K-idtofun-lc {U} k {X} x y A {p} {q} r = k (Set U) p q

lc-embedding :{X : U Ì‡} {Y : V Ì‡} (f : X â†’ Y)
             â†’ left-cancellable f
             â†’ is-set Y
             â†’ is-embedding f
lc-embedding {U} {V} {X} {Y} f f-lc iss y (x , p) (x' , p') = to-Î£-Id (r , q)
 where
   r : x â‰¡ x'
   r = f-lc (p âˆ™ (p' â»Â¹))
   q : yoneda-nat x (Î» x â†’ f x â‰¡ y) p x' r â‰¡ p'
   q = iss (yoneda-nat x (Î» x â†’ f x â‰¡ y) p x' r) p'

lc-embedding-with-K : {X : U Ì‡} {Y : V Ì‡} (f : X â†’ Y)
                    â†’ left-cancellable f â†’ K V â†’ is-embedding f
lc-embedding-with-K {U} {V} {X} {Y} f f-lc k = lc-embedding f f-lc (k Y)

id-is-embedding : {X : U Ì‡} â†’ is-embedding (id {U} {X})
id-is-embedding = identifications-to-is-prop

comp-embedding : {X : U Ì‡} {Y : V Ì‡} {Z : W Ì‡}
                {f : X â†’ Y} {g : Y â†’ Z}
               â†’ is-embedding f
               â†’ is-embedding g
               â†’ is-embedding (g âˆ˜ f)
comp-embedding {U} {V} {W} {X} {Y} {Z} {f} {g} e d = h
 where
  T : (z : Z) â†’ U âŠ” V âŠ” W Ì‡
  T z = Î£ \(w : fiber g z) â†’ fiber f (prâ‚ w)
  T-is-prop : (z : Z) â†’ is-prop (T z)
  T-is-prop z = subtype-of-prop-is-prop prâ‚ (prâ‚-lc (Î» {t} â†’ e (prâ‚ t))) (d z)
  Ï† : (z : Z) â†’ fiber (g âˆ˜ f) z â†’ T z
  Ï† z (x , p) = (f x , p) , x , refl
  Î³ : (z : Z) â†’ T z â†’ fiber (g âˆ˜ f) z
  Î³ z ((.(f x) , p) , x , refl) = x , p
  Î³Ï† : (z : Z) (t : fiber (g âˆ˜ f) z) â†’ Î³ z (Ï† z t) â‰¡ t
  Î³Ï† .(g (f x)) (x , refl) = refl
  h : (z : Z) â†’ is-prop (fiber (g âˆ˜ f) z)
  h z = subtype-of-prop-is-prop
         (Ï† z)
         (has-retraction-lc (Ï† z) (Î³ z , (Î³Ï† z)))
         (T-is-prop z)

disjoint-images : {X : U Ì‡} {Y : V Ì‡} {A : W Ì‡} â†’ (X â†’ A) â†’ (Y â†’ A) â†’ U âŠ” V âŠ” W Ì‡
disjoint-images f g = âˆ€ x y â†’ f x â‰¢ g y

disjoint-cases-embedding : {X : U Ì‡} {Y : V Ì‡} {A : W Ì‡} (f : X â†’ A) (g : Y â†’ A)
                         â†’ is-embedding f â†’ is-embedding g â†’ disjoint-images f g
                         â†’ is-embedding (cases f g)
disjoint-cases-embedding {U} {V} {W} {X} {Y} {A} f g ef eg d = go
  where
   go : (a : A) (Ïƒ Ï„ : Î£ \(z : X + Y) â†’ cases f g z â‰¡ a) â†’ Ïƒ â‰¡ Ï„
   go a (inl x , p) (inl x' , p') = r
     where
       q : x , p â‰¡ x' , p'
       q = ef a (x , p) (x' , p')
       h : fiber f a â†’ fiber (cases f g) a
       h (x , p) = inl x , p
       r : inl x , p â‰¡ inl x' , p'
       r = ap h q
   go a (inl x , p) (inr y  , q) = ğŸ˜-elim (d x y (p âˆ™ q â»Â¹))
   go a (inr y , q) (inl x  , p) = ğŸ˜-elim (d x y (p âˆ™ q â»Â¹))
   go a (inr y , q) (inr y' , q') = r
     where
       p : y , q â‰¡ y' , q'
       p = eg a (y , q) (y' , q')
       h : fiber g a â†’ fiber (cases f g) a
       h (y , q) = inr y , q
       r : inr y , q â‰¡ inr y' , q'
       r = ap h p

\end{code}

TODO.
  (1) f : X â†’ Y is an embedding iff fiber f (f x) is a singleton for every x : X.
  (2) f : X â†’ Y is an embedding iff its corestriction to its image is an equivalence.

This can be deduced directly from Yoneda.

\begin{code}

is-dense : {X : U Ì‡} {Y : V Ì‡} â†’ (X â†’ Y) â†’ U âŠ” V Ì‡
is-dense f = is-empty (Î£ \y â†’ Â¬ fiber f y)

id-is-dense : {X : U Ì‡} â†’ is-dense (id {U} {X})
id-is-dense (y , n) = n (y , refl)

comp-dense : {X : U Ì‡} {Y : V Ì‡} {Z : W Ì‡}
                {f : X â†’ Y} {g : Y â†’ Z}
           â†’ is-dense f
           â†’ is-dense g
           â†’ is-dense (g âˆ˜ f)
comp-dense {U} {V} {W} {X} {Y} {Z} {f} {g} e d = h
 where
  h : Â¬ Î£ \(z : Z) â†’ Â¬ fiber (g âˆ˜ f) z
  h (z , n) = d (z , k)
   where
    k : Â¬ fiber g z
    k (y , refl) = e (y , l)
     where
      l : Â¬ fiber f y
      l (x , refl) = n (x , refl)

\end{code}

We should find a better home for the above definition, which says that
the complement of the image of f is empty. Perhaps a better
terminology would be Â¬Â¬-dense.

\begin{code}

_â†ªáµˆ_ : U Ì‡ â†’ V Ì‡ â†’ U âŠ” V Ì‡
X â†ªáµˆ Y = Î£ \(f : X â†’ Y) â†’ is-embedding f Ã— is-dense f

module _ {U V} {X : U Ì‡} {Y : V Ì‡} where

 retraction-is-dense : (r : X â†’ Y) â†’ has-section r â†’ is-dense r
 retraction-is-dense r (s , rs) (y , n) = n (s y , rs y)

 is-equiv-is-dense : (f : X â†’ Y) â†’ is-equiv f â†’ is-dense f
 is-equiv-is-dense f e = retraction-is-dense f (is-equiv-has-section f e)

 equiv-dense-embedding : X â‰ƒ Y â†’ X â†ªáµˆ Y
 equiv-dense-embedding e = eqtofun e ,
                            is-equiv-is-embedding
                              (eqtofun e)
                              (eqtofun-is-an-equiv e),
                            is-equiv-is-dense
                              (eqtofun e)
                              (eqtofun-is-an-equiv e)

 detofun : (X â†ªáµˆ Y) â†’ X â†’ Y
 detofun = prâ‚

 is-embedding-detofun : (e : X â†ªáµˆ Y) â†’ is-embedding(detofun e)
 is-embedding-detofun e = prâ‚ (prâ‚‚ e)

 is-dense-detofun : (e : X â†ªáµˆ Y) â†’ is-dense(detofun e)
 is-dense-detofun e = prâ‚‚ (prâ‚‚ e)


module _ {U V W T}
         {X : U Ì‡}
         {A : X â†’ V Ì‡}
         {Y : W Ì‡}
         {B : Y â†’ T Ì‡}
         (f : X â†’ Y)
         (g : (x : X) â†’ A x â†’ B (f x))
       where

 pair-fun : Î£ A â†’ Î£ B
 pair-fun (x , a) = (f x , g x a)

 pair-fun-embedding : is-embedding f
                    â†’ ((x : X) â†’ is-embedding (g x))
                    â†’ is-embedding pair-fun
 pair-fun-embedding e d (y , b) = h
  where
   Z : U âŠ” V âŠ” W âŠ” T Ì‡
   Z = Î£ \(w : fiber f y) â†’ fiber (g (prâ‚ w)) (back-transport B (prâ‚‚ w) b)
   Z-is-prop : is-prop Z
   Z-is-prop = subtype-of-prop-is-prop
                prâ‚
                (prâ‚-lc (Î» {w} â†’ d (prâ‚ w) (back-transport B (prâ‚‚ w) b)))
                (e y)
   Ï† : fiber pair-fun (y , b) â†’ Z
   Ï† ((x , a) , refl) = (x , refl) , (a , refl)
   Î³ : Z â†’ fiber pair-fun (y , b)
   Î³ ((x , refl) , (a , refl)) = (x , a) , refl
   Î³Ï† : (t : fiber pair-fun (y , b)) â†’ Î³ (Ï† t) â‰¡ t
   Î³Ï† ((x , a) , refl) = refl
   h : is-prop (fiber pair-fun (y , b))
   h = subtype-of-prop-is-prop Ï† (has-retraction-lc Ï† (Î³ , Î³Ï†)) Z-is-prop

 pair-fun-dense : is-dense f
               â†’ ((x : X) â†’ is-dense (g x))
               â†’ is-dense pair-fun
 pair-fun-dense i j = contrapositive Î³ i
  where
   Î³ : (Î£ \(w : Î£ B) â†’ Â¬ fiber pair-fun w) â†’ Î£ \(y : Y) â†’ Â¬ fiber f y
   Î³ ((y , b) , n) = y , m
    where
     m : Â¬ fiber f y
     m (x , refl) = j x (b , l)
      where
       l : Â¬ fiber (g x) b
       l (a , refl) = n ((x , a) , refl)

inl-embedding : (X : U Ì‡) (Y : V Ì‡)
              â†’ is-embedding (inl {U} {V} {X} {Y})
inl-embedding {U} {V} X Y (inl a) (.a , refl) (.a , refl) = refl
inl-embedding {U} {V} X Y (inr b) (x , p) (x' , p') = ğŸ˜-elim (+disjoint p)

inr-embedding : (X : U Ì‡) (Y : V Ì‡)
              â†’ is-embedding (inr {U} {V} {X} {Y})
inr-embedding {U} {V} X Y (inl b) (x , p) (x' , p') = ğŸ˜-elim (+disjoint' p)
inr-embedding {U} {V} X Y (inr a) (.a , refl) (.a , refl) = refl

maps-of-props-are-embeddings : {P : U Ì‡} {Q : V Ì‡} (f : P â†’ Q)
                             â†’ is-prop P â†’ is-prop Q â†’ is-embedding f
maps-of-props-are-embeddings f i j q (p , s) (p' , s') = to-Î£-â‰¡ (i p p' ,
                                                                props-are-sets j _ s')

Ã—-embedding : âˆ€ {T} {X : U Ì‡} {Y : VÂ Ì‡} {A : W Ì‡} {B : T Ì‡}
                (f : X â†’ A ) (g : Y â†’ B)
            â†’ is-embedding f
            â†’ is-embedding g
            â†’ is-embedding (Î» (z : X Ã— Y) â†’ (f (prâ‚ z) , g (prâ‚‚ z)))
Ã—-embedding f g i j (a , b) = retract-of-subsingleton (r , (s , rs))
                                                      (Ã—-is-prop (i a) (j b))
 where
  r : fiber f a Ã— fiber g b â†’ fiber (Î» z â†’ f (prâ‚ z) , g (prâ‚‚ z)) (a , b)
  r ((x , s) , (y , t)) = (x , y) , to-Ã—-â‰¡ s t
  s : fiber (Î» z â†’ f (prâ‚ z) , g (prâ‚‚ z)) (a , b) â†’ fiber f a Ã— fiber g b
  s ((x , y) , p) = (x , ap prâ‚ p) , (y , ap prâ‚‚ p)
  rs : (Ï† : fiber (Î» z â†’ f (prâ‚ z) , g (prâ‚‚ z)) (a , b)) â†’ r (s Ï†) â‰¡ Ï†
  rs ((x , y) , refl) = refl

NatÎ£-is-embedding : {X : U Ì‡} (A : X â†’ V Ì‡) (B : X â†’ W Ì‡) (Î¶ : Nat A B)
                  â†’ ((x : X) â†’ is-embedding(Î¶ x)) â†’ is-embedding(NatÎ£ Î¶)
NatÎ£-is-embedding A B Î¶ i (x , b) = equiv-to-subsingleton
                                     (â‰ƒ-sym (NatÎ£-fiber-equiv A B Î¶ x b))
                                     (i x b)

NatÎ£-is-embedding-converse : {X : U Ì‡} (A : X â†’ V Ì‡) (B : X â†’ W Ì‡) (Î¶ : Nat A B)
                           â†’ is-embedding(NatÎ£ Î¶) â†’ ((x : X) â†’ is-embedding(Î¶ x))
NatÎ£-is-embedding-converse A B Î¶ e x b = equiv-to-subsingleton
                                          (NatÎ£-fiber-equiv A B Î¶ x b)
                                          (e (x , b))

NatÎ -is-embedding : {X : U Ì‡} (A : X â†’ V Ì‡) (B : X â†’ W Ì‡) (Î¶ : Nat A B)
                  â†’ funext U W â†’ funext U (V âŠ” W)
                  â†’ ((x : X) â†’ is-embedding(Î¶ x)) â†’ is-embedding(NatÎ  Î¶)
NatÎ -is-embedding A B Î¶ fe fe' i g = equiv-to-subsingleton
                                      (â‰ƒ-sym (NatÎ -fiber-equiv A B Î¶ fe g))
                                      (Î -is-prop fe' (Î» x â†’ i x (g x)))

\end{code}
