In univalent logic, as opposed to Curry-Howard logic, a proposition is
a subsingleton or a type such that any two of its elements are
identified.

https://www.newton.ac.uk/files/seminar/20170711100011001-1009756.pdf
https://unimath.github.io/bham2017/uf.pdf

About (sub)singletons using function extensionality.

\begin{code}

{-# OPTIONS --without-K --exact-split #-}

module UF-Subsingletons-FunExt where

open import SpartanMLTT
open import UF-Base
open import UF-Subsingletons
open import UF-FunExt
open import UF-LeftCancellable

Î -is-prop : funext U V â†’ {X : U Ì‡} {A : X â†’ V Ì‡}
          â†’ ((x : X) â†’ is-prop (A x)) â†’ is-prop (Î  A)
Î -is-prop fe i f g = dfunext fe (Î» x â†’ i x (f x) (g x))

Î -is-singleton : funext U V â†’ {X : U Ì‡} {A : X â†’ V Ì‡}
               â†’ ((x : X) â†’ is-singleton (A x)) â†’ is-singleton (Î  A)
Î -is-singleton fe i = (Î» x â†’ prâ‚ (i x)) , (Î» f â†’ dfunext fe (Î» x â†’ prâ‚‚ (i x) (f x)))

being-a-prop-is-a-prop : {X : U Ì‡} â†’ funext U U â†’ is-prop (is-prop X)
being-a-prop-is-a-prop {U} {X} fe f g = câ‚
 where
  l : is-set X
  l = props-are-sets f
  c : (x y : X) â†’ f x y â‰¡ g x y
  c x y = l (f x y) (g x y)
  câ‚€ : (x : X) â†’ f x â‰¡ g x
  câ‚€ x = dfunext fe (c x)
  câ‚ : f â‰¡ g
  câ‚  = dfunext fe câ‚€

identifications-of-props-are-props : propext U â†’ funext U U
                      â†’ (P : U Ì‡) â†’ is-prop P
                      â†’ (X : U Ì‡) â†’ is-prop (X â‰¡ P)
identifications-of-props-are-props {U} pe fe P i = local-hedberg' P (Î» X â†’ g X âˆ˜ f X , k X)
 where
  f : (X : U Ì‡) â†’ X â‰¡ P â†’ is-prop X Ã— (X â‡” P)
  f X refl = i , (id , id)
  g : (X : U Ì‡) â†’ is-prop X Ã— (X â‡” P) â†’ X â‰¡ P
  g X (l , Ï† , Î³) = pe l i Ï† Î³
  j : (X : U Ì‡) â†’ is-prop (is-prop X Ã— (X â‡” P))
  j X = Ã—-prop-criterion ((Î» _ â†’ being-a-prop-is-a-prop fe) ,
                          (Î» l â†’ Ã—-is-prop (Î -is-prop fe (Î» x â†’ i))
                                            (Î -is-prop fe (Î» p â†’ l))))
  k : (X : U Ì‡) â†’ constant (g X âˆ˜ f X)
  k X p q = ap (g X) (j X (f X p) (f X q))

is-singleton-is-a-prop : {X : U Ì‡} â†’ funext U U â†’ is-prop(is-singleton X)
is-singleton-is-a-prop {U} {X} fe (x , Ï†) (y , Î³) = to-Î£-â‰¡ (Ï† y , dfunext fe Î» z â†’ iss {y} {z} _ _)
 where
  isp : is-prop X
  isp = singletons-are-propositions (y , Î³)
  iss : is-set X
  iss = props-are-sets isp

Î -is-set : funext U V â†’ {X : U Ì‡} {A : X â†’ V Ì‡}
         â†’ ((x : X) â†’ is-set(A x)) â†’ is-set(Î  A)
Î -is-set {U} {V} fe {X} {A} isa {f} {g} = b
 where
  a : is-prop (f âˆ¼ g)
  a p q = dfunext fe Î» x â†’ isa x (p x) (q x)
  b : is-prop(f â‰¡ g)
  b = left-cancellable-reflects-is-prop happly (section-lc happly (prâ‚‚ (fe f g))) a

\end{code}

The meat of the following proof is being-set-is-a-prop'. The rest of the
code is to deal with implicit arguments in conjunction with function
extensionality. The solution is not ideal. Ideally, functions with
implicit parameters should be the same as their versions with explicit
parameters.

\begin{code}

being-set-is-a-prop : {X : U Ì‡} â†’ funext U U â†’ is-prop (is-set X)
being-set-is-a-prop {U} {X} fe = h
 where
  is-set' : U Ì‡ â†’ U Ì‡
  is-set' X = (x y : X) â†’ is-prop(x â‰¡ y)

  being-set-is-a-prop' : {X : U Ì‡} â†’ funext U U â†’ is-prop (is-set' X)
  being-set-is-a-prop' fe = Î -is-prop fe
                         (Î» x â†’ Î -is-prop fe
                         (Î» y â†’ being-a-prop-is-a-prop fe))

  f : {X : U Ì‡} â†’ is-set' X â†’ is-set X
  f s {x} {y} = s x y

  g : {X : U Ì‡} â†’ is-set X â†’ is-set' X
  g s x y = s {x} {y}

  h : is-prop (is-set X)
  h = subtype-of-prop-is-a-prop g (ap f) (being-set-is-a-prop' fe)

\end{code}

\begin{code}

decidable-types-are-props : {P : U Ì‡} â†’ funext U Uâ‚€ â†’ is-prop P â†’ is-prop(P + Â¬ P)
decidable-types-are-props feâ‚€ isp = sum-of-contradictory-props
                             isp
                             (Î -is-prop feâ‚€ Î» _ â†’ ğŸ˜-is-prop)
                             (Î» p u â†’ u p)

PropExt : funext U U â†’ propext U â†’ {p q : Î© U}
        â†’ (p holds â†’ q holds) â†’ (q holds â†’ p holds) â†’ p â‰¡ q
PropExt {U} fe pe {p} {q} f g =
 to-Î£-â‰¡ ((pe (holds-is-prop p) (holds-is-prop q) f g) , being-a-prop-is-a-prop fe _ _)

Î©-is-a-set : funext U U â†’ propext U â†’ is-set (Î© U)
Î©-is-a-set {U} fe pe = Id-collapsibles-are-sets pc
 where
  A : (p q : Î© U) â†’ U Ì‡
  A p q = (p holds â†’ q holds) Ã— (q holds â†’ p holds)
  A-is-prop : (p q : Î© U) â†’ is-prop(A p q)
  A-is-prop p q = Î£-is-prop (Î -is-prop fe
                                   (Î» _ â†’ holds-is-prop q))
                                   (Î» _ â†’ Î -is-prop fe (Î» _ â†’ holds-is-prop p))
  g : (p q : Î© U) â†’ p â‰¡ q â†’ A p q
  g p q e = (b , c)
   where
    a : p holds â‰¡ q holds
    a = ap _holds e
    b : p holds â†’ q holds
    b = transport (Î» X â†’ X) a
    c : q holds â†’ p holds
    c = transport (Î» X â†’ X) (a â»Â¹)
  h  : (p q : Î© U) â†’ A p q â†’ p â‰¡ q
  h p q (u , v) = PropExt fe pe u v
  f  : (p q : Î© U) â†’ p â‰¡ q â†’ p â‰¡ q
  f p q e = h p q (g p q e)
  constant-f : (p q : Î© U) (d e : p â‰¡ q) â†’ f p q d â‰¡ f p q e
  constant-f p q d e = ap (h p q) (A-is-prop p q (g p q d) (g p q e))
  pc : {p q : Î© U} â†’ Î£ \(f : p â‰¡ q â†’ p â‰¡ q) â†’ constant f
  pc {p} {q} = (f p q , constant-f p q)

powersets-are-sets : {A : U Ì‡} â†’ funext U (V âº) â†’ funext V V â†’ propext V
                â†’ is-set (A â†’ Î© V)
powersets-are-sets {U} fe fe' pe = Î -is-set fe (Î» x â†’ Î©-is-a-set fe' pe)

negations-are-props : {X : U Ì‡} â†’ funext U Uâ‚€ â†’ is-prop(Â¬ X)
negations-are-props fe = Î -is-prop fe (Î» x â†’ ğŸ˜-is-prop)

not : funext U Uâ‚€ â†’ Î© U â†’ Î© U
not fe (P , i) = (Â¬ P , negations-are-props fe)

\end{code}

For the moment we work with Uâ‚€ here because ğŸ™ and âŠ¤ live in Uâ‚€:

\begin{code}

equal-âŠ¤-is-true : (P : U Ì‡) (i : is-prop P)
               â†’ (P , i) â‰¡ âŠ¤ â†’ P
equal-âŠ¤-is-true P hp r = f *
 where
  s : ğŸ™ â‰¡ P
  s = (ap prâ‚ r)â»Â¹
  f : ğŸ™ â†’ P
  f = transport id s

true-is-equal-âŠ¤ : propext U â†’ funext U U â†’ (P : U Ì‡) (i : is-prop P)
                â†’ P â†’ (P , i) â‰¡ âŠ¤
true-is-equal-âŠ¤ pe fe P i x = to-Î£-â‰¡ (pe i ğŸ™-is-prop unique-to-ğŸ™ (Î» _ â†’ x) ,
                                        being-a-prop-is-a-prop fe _ _)

Î©-ext : propext U â†’ funext U U â†’ {p q : Î© U}
      â†’ (p â‰¡ âŠ¤ â†’ q â‰¡ âŠ¤) â†’ (q â‰¡ âŠ¤ â†’ p â‰¡ âŠ¤) â†’ p â‰¡ q
Î©-ext pe fe {(P , i)} {(Q , j)} f g = to-Î£-â‰¡ (pe i j I II ,
                                              being-a-prop-is-a-prop fe _ _ )
 where
  I : P â†’ Q
  I x = equal-âŠ¤-is-true Q j (f (true-is-equal-âŠ¤ pe fe P i x))
  II : Q â†’ P
  II y = equal-âŠ¤-is-true P i (g (true-is-equal-âŠ¤ pe fe Q j y))

\end{code}

Without excluded middle, we have that:

\begin{code}

no-truth-values-other-than-âŠ¥-or-âŠ¤ : funext U U â†’ propext U
                                   â†’ Â¬ Î£ \(p : Î© U) â†’ (p â‰¢ âŠ¥) Ã— (p â‰¢ âŠ¤)
no-truth-values-other-than-âŠ¥-or-âŠ¤ fe pe ((P , isp) , (f , g)) = Ï† u
 where
   u : Â¬ P
   u p = g l
     where
       l : (P , isp) â‰¡ âŠ¤
       l = PropExt fe pe unique-to-ğŸ™ (Î» _ â†’ p)
   Ï† : Â¬Â¬ P
   Ï† u = f l
     where
       l : (P , isp) â‰¡ âŠ¥
       l = PropExt fe pe (Î» p â†’ ğŸ˜-elim (u p)) unique-from-ğŸ˜

\end{code}

The above and following ğŸ˜-elim is used to coerce from ğŸ˜ {U} to ğŸ˜ {Uâ‚€}
as this is where negations take values in.

\begin{code}

âŠ¥-is-not-âŠ¤ : Â¬(âŠ¥ {U} â‰¡ âŠ¤ {U})
âŠ¥-is-not-âŠ¤ b = ğŸ˜-elim(ğŸ˜-is-not-ğŸ™ (ap _holds b))

\end{code}
