Martin Escardo, 14th January 2022.

An isomorphic copy of ℕ∞ defined in CoNaturals.GenericConvergentSequence.
The isomorphism is proved in CoNaturals.Equivalence.

\begin{code}

{-# OPTIONS --safe --without-K #-}

module CoNaturals.GenericConvergentSequence2 where

open import MLTT.Spartan
open import MLTT.Two-Properties
open import Naturals.Order hiding (max)
open import Naturals.Properties
open import Notation.CanonicalMap
open import Notation.Order
open import TypeTopology.Cantor
open import UF.DiscreteAndSeparated
open import UF.FunExt
open import UF.NotNotStablePropositions
open import UF.Sets
open import UF.Subsingletons
open import UF.Subsingletons-FunExt

T-cantor : (ℕ → 𝟚) → 𝓤₀ ̇
T-cantor α = Σ n ꞉ ℕ , α n ＝ ₁

private
 T = T-cantor

has-at-most-one-₁ : (ℕ → 𝟚) → 𝓤₀ ̇
has-at-most-one-₁ α = is-prop (T α)

has-at-most-one-₁-is-prop : funext₀ → (α : ℕ → 𝟚) → is-prop (has-at-most-one-₁ α)
has-at-most-one-₁-is-prop fe α = being-prop-is-prop fe

ℕ∞' : 𝓤₀ ̇
ℕ∞' = Σ α ꞉ (ℕ → 𝟚) , has-at-most-one-₁ α

ℕ∞'-to-ℕ→𝟚 : ℕ∞' → (ℕ → 𝟚)
ℕ∞'-to-ℕ→𝟚 = pr₁

ℕ∞'-to-ℕ→𝟚-lc : funext₀ → left-cancellable ℕ∞'-to-ℕ→𝟚
ℕ∞'-to-ℕ→𝟚-lc fe = pr₁-lc (being-prop-is-prop fe)

ℕ∞'-is-¬¬-separated : funext₀ → is-¬¬-separated ℕ∞'
ℕ∞'-is-¬¬-separated fe = subtype-is-¬¬-separated
                         pr₁
                         (ℕ∞'-to-ℕ→𝟚-lc fe)
                         (Cantor-is-¬¬-separated fe)

ℕ∞'-is-set : funext₀ → is-set ℕ∞'
ℕ∞'-is-set fe = ¬¬-separated-types-are-sets fe (ℕ∞'-is-¬¬-separated fe)

private
 ¬T : (ℕ → 𝟚) → 𝓤₀ ̇
 ¬T α = (n : ℕ) → α n ＝ ₀

not-T-gives-¬T : {α : ℕ → 𝟚} → ¬ (T α) → ¬T α
not-T-gives-¬T {α} ϕ n = different-from-₁-equal-₀ (λ (e : α n ＝ ₁) → ϕ (n , e))

¬T-gives-not-T : {α : ℕ → 𝟚} → ¬T α → ¬ (T α)
¬T-gives-not-T {α} ψ (n , e) = zero-is-not-one ((ψ n)⁻¹ ∙ e)

to-T-＝ : {α : ℕ → 𝟚}
          {n n' : ℕ}
        → n ＝ n'
        → {e : α n ＝ ₁} {e' : α n' ＝ ₁}
        → (n , e) ＝[ T α ] (n' , e')
to-T-＝ p = to-subtype-＝ (λ - → 𝟚-is-set) p

from-T-＝ : {α : ℕ → 𝟚}
          {n n' : ℕ}
        → {e : α n ＝ ₁} {e' : α n' ＝ ₁}
        → (n , e) ＝[ T α ] (n' , e')
        → n ＝ n'
from-T-＝ p = ap pr₁ p

index-uniqueness : (α : ℕ → 𝟚)
                 → is-prop (T α)
                 → {n n' : ℕ} → α n ＝ ₁ → α n' ＝ ₁ → n ＝ n'
index-uniqueness α i {n} {n'} e e' = from-T-＝ (i (n , e) (n' , e'))

index-uniqueness-converse : (α : ℕ → 𝟚)
                          → ({n n' : ℕ} → α n ＝ ₁ → α n' ＝ ₁ → n ＝ n')
                          → is-prop (T α)
index-uniqueness-converse α ϕ (n , e) (n' , e') = to-T-＝ (ϕ e e')

private
 instance
  canonical-map-ℕ∞'-ℕ→𝟚 : Canonical-Map ℕ∞' (ℕ → 𝟚)
  ι {{canonical-map-ℕ∞'-ℕ→𝟚}} = ℕ∞'-to-ℕ→𝟚

ℕ∞'-to-ℕ→𝟚-at-most-one-₁ : (u : ℕ∞') → is-prop (T (ℕ∞'-to-ℕ→𝟚 u))
ℕ∞'-to-ℕ→𝟚-at-most-one-₁ = pr₂

ℕ∞'-index-uniqueness : (u : ℕ∞')
                     → {n n' : ℕ} → ι u n ＝ ₁ → ι u n' ＝ ₁ → n ＝ n'
ℕ∞'-index-uniqueness (α , i) = index-uniqueness α i

Zero' : ℕ∞'
Zero' = α , h
 where
  α : ℕ → 𝟚
  α 0        = ₁
  α (succ n) = ₀

  i : is-prop (T α)
  i (0 , e) (0 , e') = to-T-＝ refl

  h : has-at-most-one-₁ α
  h (n , e) (n' , e') = to-T-＝ (index-uniqueness α i e e')

Succ' : ℕ∞' → ℕ∞'
Succ' (α , h) = cons ₀ α , h'
 where
  h' : has-at-most-one-₁ (cons ₀ α)
  h' (succ n , e) (succ n' , e') = to-T-＝ (ap succ (index-uniqueness α h e e'))

ℕ-to-ℕ∞' : ℕ → ℕ∞'
ℕ-to-ℕ∞' 0        = Zero'
ℕ-to-ℕ∞' (succ n) = Succ' (ℕ-to-ℕ∞' n)

private
 instance
  Canonical-Map-ℕ-ℕ∞' : Canonical-Map ℕ ℕ∞'
  ι {{Canonical-Map-ℕ-ℕ∞'}} = ℕ-to-ℕ∞'

is-finite' : ℕ∞' → 𝓤₀ ̇
is-finite' u@(α , a) = T α

being-finite'-is-prop : funext₀ → (u : ℕ∞') → is-prop (is-finite' u)
being-finite'-is-prop fe₀ u@(α , a) = a

size' : {u : ℕ∞'} → is-finite' u → ℕ
size' (n , e) = n

size'-property : {u : ℕ∞'} (φ : is-finite' u) → ℕ∞'-to-ℕ→𝟚 u (size' {u} φ) ＝ ₁
size'-property (n , e) = e

Zero'-is-finite : is-finite' Zero'
Zero'-is-finite = 0 , refl

is-finite'-up : (u : ℕ∞')
              → is-finite' u
              → is-finite' (Succ' u)
is-finite'-up _ (n , e) = succ n , e

is-finite'-down : (u : ℕ∞')
                → is-finite' (Succ' u)
                → is-finite' u
is-finite'-down _ (succ n , e) = n , e

ℕ-to-ℕ∞'-is-finite' : (n : ℕ) → is-finite' (ι n)
ℕ-to-ℕ∞'-is-finite' 0        = Zero'-is-finite
ℕ-to-ℕ∞'-is-finite' (succ n) = is-finite'-up (ι n)
                                (ℕ-to-ℕ∞'-is-finite' n)

∞' : ℕ∞'
∞' = (λ _ → ₀) , (λ (n , e) (n' , e') → 𝟘-elim (zero-is-not-one e))

not-finite'-is-∞' : funext₀ → (u : ℕ∞') → ¬ is-finite' u → u ＝ ∞'
not-finite'-is-∞' fe u ν = ℕ∞'-to-ℕ→𝟚-lc fe
                            (dfunext fe
                              (λ i → different-from-₁-equal-₀
                                      (λ (e : ℕ∞'-to-ℕ→𝟚 u i ＝ ₁) → ν (i , e))))

not-T-is-∞' : funext₀ → (u : ℕ∞') → ¬ T (ι u) → u ＝ ∞'
not-T-is-∞' fe u ν = ℕ∞'-to-ℕ→𝟚-lc fe (dfunext fe (not-T-gives-¬T ν))

is-infinite-∞' : ¬ is-finite' ∞'
is-infinite-∞' (n , e) = zero-is-not-one e

\end{code}
